Cleanup till end of safety

type_system/subtyping_lemmas.v
@@ -10,18 +10,20 @@ Require Export declarational wf_lemmas.
 (* ==================== Sig and Eqs Properties ==================== *)
 
 Lemma sig_subtype_get_Some Σ Σ' op A B :
-  sig_subtype Σ Σ' -> get_op_type Σ op = Some (A, B) -> exists A' B', 
-  get_op_type Σ' op = Some (A', B') /\ vsubtype A A' /\ vsubtype B' B.
+  sig_subtype Σ Σ' -> get_op_type Σ op = Some (A, B) -> 
+  exists A' B', 
+    get_op_type Σ' op = Some (A', B') /\ 
+    vsubtype A A' /\ vsubtype B' B.
 Proof.
 intros sty gets. induction sty; simpl in gets. discriminate.
-destruct (op == op0).
-- inv gets. exists A'. exists B'. auto.
-- apply IHsty in gets. assumption.
+destruct (op == op0); eauto.
+inv gets. exists A', B'. auto.
 Qed.
 
 
 Lemma sig_subtype_extend Σ Σ' op A B :
-  sig_subtype Σ Σ' -> wf_sig (SigU Σ' op A B) -> sig_subtype Σ (SigU Σ' op A B).
+  sig_subtype Σ Σ' -> wf_sig (SigU Σ' op A B) -> 
+  sig_subtype Σ (SigU Σ' op A B).
 Proof.
 intros. induction H.
 + apply SubtypeSigØ.
@@ -33,7 +35,8 @@ Qed.
 Lemma sig_subtype_empty Σ : 
   sig_subtype Σ SigØ -> Σ = SigØ.
 Proof.
-intro subty. inv subty. reflexivity. simpl in *. discriminate.
+intro subty. inv subty.
+auto. simpl in *. discriminate.
 Qed.
 
 
@@ -43,7 +46,7 @@ Lemma eqs_subtype_extend E E' Σ Γ Z T1 T2 :
 Proof.
 intros. induction H.
 + apply SubtypeEqsØ.
-+ eapply SubtypeEqsU. auto. simpl. right. assumption.
++ eapply SubtypeEqsU. auto. simpl. right. auto.
 Qed.
 
 
@@ -52,13 +55,14 @@ Lemma eqs_subtype_contains E E' Γ Z T1 T2 :
   has_eq E' Γ Z T1 T2.
 Proof.
 intros sty gets. induction sty; simpl in gets; destruct gets; auto.
-destruct H0 as [a [b [c ]]]. subst. assumption.
+destruct H0 as [a [b [c d]]]. subst. assumption.
 Qed.
 
 Lemma eqs_subtype_empty E E': 
   eqs_subtype E E' -> E' = EqsØ -> E = EqsØ.
 Proof.
-intros subty eq. induction subty. auto. subst. simpl in H. destruct H.
+intros subty eq. induction subty.
+auto. subst. simpl in H. destruct H.
 Qed.
 
 (* ==================== Reflexivity and Transitivity ==================== *)
@@ -100,119 +104,130 @@ apply SubtypeCtxU; inv H; auto.
 Qed.
 
 
-Fixpoint eqs_subtype_trans E1 E2 E3 (E12 : eqs_subtype E1 E2) {struct E12} : 
-  eqs_subtype E2 E3 -> eqs_subtype E1 E3.
+Fixpoint eqs_subtype_trans E1 E2 E3 
+  (E12 : eqs_subtype E1 E2) {struct E12} :  eqs_subtype E2 E3 -> 
+  eqs_subtype E1 E3.
 Proof.
 intros E23. destruct E12.
-apply SubtypeEqsØ.
-eapply SubtypeEqsU; eauto; eapply eqs_subtype_contains; eauto.
++ apply SubtypeEqsØ.
++ eapply SubtypeEqsU; eauto; eapply eqs_subtype_contains; eauto.
 Qed.
 
-
-(* Weird notation for SPEED! *)
+(* Use all lemmas explicitly, in order to ensure termination. The 'rev' lemmas
+   are used for precisely that reason. *)
 Fixpoint vsubtype_trans A1 A2 A3 
   (A12 : vsubtype A1 A2) {struct A12} : vsubtype A2 A3 -> 
   vsubtype A1 A3
+
 with vsubtype_trans_rev A1 A2 A3
   (A21 : vsubtype A2 A1) {struct A21} : vsubtype A3 A2 -> 
   vsubtype A3 A1
+
 with csubtype_trans C1 C2 C3
   (C12 : csubtype C1 C2) {struct C12} : csubtype C2 C3 -> 
   csubtype C1 C3
+
 with csubtype_trans_rev C1 C2 C3 
   (C21 : csubtype C2 C1) {struct C21} : csubtype C3 C2 -> 
   csubtype C3 C1
+
 with sig_subtype_trans Σ1 Σ2 Σ3 
   (S12 : sig_subtype Σ1 Σ2) {struct S12} : sig_subtype Σ2 Σ3 -> 
   sig_subtype Σ1 Σ3
+
 with sig_subtype_trans_rev Σ1 Σ2 Σ3
   (S21 : sig_subtype Σ2 Σ1) {struct S21} : sig_subtype Σ3 Σ2 -> 
   sig_subtype Σ3 Σ1
+
 with get_op_trans op A' A B B' Σ1 Σ2 (S12 : sig_subtype Σ1 Σ2) {struct S12} :
-  get_op_type Σ1 op = Some (A', B') -> vsubtype A A' -> vsubtype B' B ->
+  get_op_type Σ1 op = Some (A', B') ->
+  vsubtype A A' -> vsubtype B' B ->
   exists A'' B'', 
-  get_op_type Σ2 op = Some (A'', B'') /\ vsubtype A A'' /\ vsubtype B'' B.
+    get_op_type Σ2 op = Some (A'', B'') /\ 
+    vsubtype A A'' /\ vsubtype B'' B.
+
 Proof.
+all: rename vsubtype_trans into VT; rename vsubtype_trans_rev into VTR.
+all: rename csubtype_trans into CT; rename csubtype_trans_rev into CTR.
+all: rename sig_subtype_trans into ST; rename sig_subtype_trans_rev into STR.
+all: rename get_op_trans into GOPT.
 {
-clear sig_subtype_trans sig_subtype_trans_rev get_op_trans.
+clear ST STR GOPT.
 intros A23; destruct A12; try assumption; inv A23. 
 + apply SubtypeTyΣ; eauto.
 + apply SubtypeTyΠ; eauto.
 + apply SubtypeTyList; eauto.
 + apply SubtypeTyFun.
-  - eapply vsubtype_trans_rev; eauto. 
-  - eapply csubtype_trans; eauto.
+  - eapply VTR; eauto. 
+  - eapply CT; eauto.
 + apply SubtypeTyHandler.
-  - eapply csubtype_trans_rev; eauto. 
-  - eapply csubtype_trans; eauto.
+  - eapply CTR; eauto. 
+  - eapply CT; eauto.
 }{
-clear sig_subtype_trans sig_subtype_trans_rev get_op_trans.
+clear ST STR GOPT.
 intros A32; destruct A21; try assumption; inv A32. 
-+ apply SubtypeTyΣ; eapply vsubtype_trans_rev; eauto.
-+ apply SubtypeTyΠ; eapply vsubtype_trans_rev; eauto.
-+ apply SubtypeTyList; eapply vsubtype_trans_rev; eauto.
++ apply SubtypeTyΣ; eapply VTR; eauto.
++ apply SubtypeTyΠ; eapply VTR; eauto.
++ apply SubtypeTyList; eapply VTR; eauto.
 + apply SubtypeTyFun.
-  - eapply vsubtype_trans; eauto.
-  - eapply csubtype_trans_rev; eauto.
+  - eapply VT; eauto.
+  - eapply CTR; eauto.
 + apply SubtypeTyHandler.
-  - eapply csubtype_trans; eauto.
-  - eapply csubtype_trans_rev; eauto.
+  - eapply CT; eauto.
+  - eapply CTR; eauto.
 }{
-clear vsubtype_trans_rev csubtype_trans csubtype_trans_rev.
-clear sig_subtype_trans_rev get_op_trans.
+clear VTR CT CTR STR GOPT.
 intros C23; destruct C12. inv C23. apply SubtypeCTy.
-- eapply vsubtype_trans; eauto.
-- eapply sig_subtype_trans; eauto.
+- eapply VT; eauto.
+- eapply ST; eauto.
 - eapply eqs_subtype_trans; eauto.
 }{
-clear vsubtype_trans csubtype_trans csubtype_trans.
-clear sig_subtype_trans get_op_trans.
+clear VT CT CTR ST GOPT.
 intros C32; destruct C21. inv C32. apply SubtypeCTy.
-- eapply vsubtype_trans_rev; eauto.
-- eapply sig_subtype_trans_rev; eauto.
+- eapply VTR; eauto.
+- eapply STR; eauto.
 - eapply eqs_subtype_trans; eauto.
 }{
-clear csubtype_trans csubtype_trans_rev sig_subtype_trans_rev.
+clear CT CTR STR.
 intros S23. destruct S12.
-{ apply SubtypeSigØ. }
+apply SubtypeSigØ.
 apply (sig_subtype_get_Some Σ' Σ3) in H as H'.
-destruct H' as [A'' [B'' [g]]]. eapply SubtypeSigU.
+destruct H' as [A'' [B'' [g [stya' styb']]]].
+eapply SubtypeSigU.
 2 : exact g. all: try assumption.
-+ eapply sig_subtype_trans; eauto.
-+ clear sig_subtype_trans vsubtype_trans_rev.
-  destruct H2. eapply vsubtype_trans; eauto.
-+ clear sig_subtype_trans vsubtype_trans.
-  destruct H2. eapply vsubtype_trans_rev; eauto.
++ eapply ST; eauto.
++ eapply VT; eauto.
++ eapply VTR; eauto.
 }{
-clear csubtype_trans csubtype_trans_rev sig_subtype_trans.
+clear CT CTR ST.
 intros S32. destruct S21.
 { apply sig_subtype_empty in S32. subst. apply SubtypeSigØ. }
 induction Σ3.
 { apply SubtypeSigØ. }
 inv S32. simpl in *. destruct (o==op).
 + inv H8. eapply SubtypeSigU. auto. eauto.
-  - eapply vsubtype_trans_rev; eauto.
-  - eapply vsubtype_trans; eauto.
-+ eapply get_op_trans in H8 as gets'.
-  2:exact S21. 2:exact H9. 2:exact H10.
-  destruct gets' as [A'' [B'' [gets' [styA'']]]].
+  - eapply VTR; eauto.
+  - eapply VT; eauto.
++ eapply GOPT in H8 as gets'. all: eauto.
+  destruct gets' as [A'' [B'' [gets' [styA'' styB'']]]].
   eapply SubtypeSigU; eauto.
 }{
-clear csubtype_trans csubtype_trans_rev.
-clear sig_subtype_trans sig_subtype_trans_rev get_op_trans.
+clear CT CTR ST STR GOPT.
 intros. revert H. induction S12; intros gets; simpl in *. discriminate.
 destruct (op==op0). 2: auto. inv gets.
-exists A'0. exists B'0. aconstructor. constructor.
-- eapply vsubtype_trans_rev; eauto.
-- eapply vsubtype_trans; eauto.
+exists A'0, B'0. aconstructor. constructor.
+- eapply VTR; eauto.
+- eapply VT; eauto.
 }
 Qed.
 
 
 Fixpoint ctx_subtype_trans Γ Γ' Γ'':
-  ctx_subtype Γ Γ' -> ctx_subtype Γ' Γ'' -> ctx_subtype Γ Γ''.
+  ctx_subtype Γ Γ' -> ctx_subtype Γ' Γ'' -> 
+  ctx_subtype Γ Γ''.
 Proof.
-destruct Γ; destruct Γ'; destruct Γ''; intros sty sty'. all: inv sty; inv sty'.
+destruct Γ; destruct Γ'; destruct Γ''; intros sty sty'. 
+all: inv sty; inv sty'.
 - apply SubtypeCtxØ.
 - apply SubtypeCtxU. eauto. eapply vsubtype_trans; eauto.
 Qed.
@@ -221,23 +236,25 @@ Qed.
 
 Fixpoint ctx_subtype_get Γ Γ' A num (csty : ctx_subtype Γ Γ') {struct csty}:
   get_vtype Γ num = Some A -> 
-  exists A', get_vtype Γ' num = Some A' /\ vsubtype A A'.
+  exists A', 
+    get_vtype Γ' num = Some A' /\ vsubtype A A'.
 Proof.
 revert num. induction csty. clear ctx_subtype_get.
 + intros num H. simpl in H. discriminate.
 + intros num get. destruct num; eauto.
-  clear IHcsty. simpl in *. inv get. exists A'. auto.
+  simpl in *. inv get. exists A'. auto.
 Qed.
 
 
 Fixpoint ctx_subtype_get_rev Γ Γ' A num (csty : ctx_subtype Γ' Γ) {struct csty}:
   get_vtype Γ num = Some A -> 
-  exists A', get_vtype Γ' num = Some A' /\ vsubtype A' A.
+  exists A', 
+    get_vtype Γ' num = Some A' /\ vsubtype A' A.
 Proof.
 revert num. induction csty. clear ctx_subtype_get_rev.
 + intros num H. simpl in H. discriminate.
 + intros num get. destruct num; eauto.
-  clear IHcsty. simpl in *. inv get. exists A0. auto.
+  simpl in *. inv get. exists A0. auto.
 Qed.
 
 
@@ -248,13 +265,15 @@ Proof.
 intros sty1 sty2. induction sty2; auto. apply SubtypeCtxU; assumption. 
 Qed.
 
+
 Lemma ctx_subtype_tctx_to_ctx Z C C':
   wf_tctx Z -> csubtype C C' -> 
   ctx_subtype (tctx_to_ctx Z C) (tctx_to_ctx Z C').
 Proof.
-intros wfz sty. induction Z; simpl. apply SubtypeCtxØ. 
-apply SubtypeCtxU. inv wfz. auto. apply SubtypeTyFun.
-apply vsubtype_refl. inv wfz. auto. auto. 
+intros wfz sty. induction Z; simpl.
++ apply SubtypeCtxØ. 
++ apply SubtypeCtxU. inv wfz. auto.
+  apply SubtypeTyFun. apply vsubtype_refl. inv wfz. auto. auto.
 Qed.
 
 
@@ -265,33 +284,9 @@ intro sty. induction sty; simpl; auto.
 Qed. 
 
 
-Lemma ctx_subtype_insert Γ A Γ' i: 
-  wf_ctx Γ' -> wf_ctx Γ -> wf_vtype A -> ctx_subtype Γ' (ctx_insert Γ A i) ->
-  exists Γ'' A', Γ' = ctx_insert Γ'' A' i /\ vsubtype A' A 
-    /\ wf_vtype A' /\ ctx_subtype Γ'' Γ.
-Proof.
-revert Γ A i. induction Γ'; intros Γ A i wfg' wfg wfA sty. 
-* inv sty. exists Γ. exists A. aconstructor. constructor.
-  apply vsubtype_refl. assumption. destruct Γ. aconstructor. apply SubtypeCtxØ.
-  simpl in H. destruct i; discriminate.
-* inv sty. destruct i.
-  + assert (forall Γ A, ctx_insert Γ A 0 = CtxU Γ A).
-    {intros. destruct Γ0; simpl; auto. }
-    rewrite H in H1. inv H1. exists Γ'. exists v. inv wfg'. auto.
-  + destruct Γ. simpl in *. discriminate.
-    assert (forall Γ A A', 
-      ctx_insert (CtxU Γ A') A (S i) = CtxU (ctx_insert Γ A i) A').
-    {intros. destruct Γ0; simpl; auto. }
-    rewrite H in H1. inv H1. inv wfg'. inv wfg. 
-    apply IHΓ' in H2; auto. destruct H2 as [Γ''[A'[ins[sty]]]].
-    exists (CtxU Γ'' v). exists A'. constructor. rewrite H. f_equal. auto.
-    aconstructor. destruct H0. aconstructor. apply SubtypeCtxU; auto.
-Qed.
-
-
-Fixpoint ctx_subtype_insert_rev Γ Γ' A A' n:
+Fixpoint ctx_subtype_insert Γ Γ' A A' n:
   ctx_subtype Γ Γ' -> vsubtype A A' ->
-  ctx_subtype (ctx_insert Γ A n) (ctx_insert Γ' A' n).
+  ctx_subtype (ctx_insert Γ n A) (ctx_insert Γ' n A').
 Proof.
 intros. destruct H; simpl in *; destruct n.
 + apply SubtypeCtxU. apply SubtypeCtxØ. auto.
@@ -299,25 +294,6 @@ intros. destruct H; simpl in *; destruct n.
 + apply SubtypeCtxU. apply SubtypeCtxU. all: auto.
 + apply SubtypeCtxU; auto.
 Qed.
-
-
-Lemma ctx_subtype_remove Γ Γ' i: 
-  wf_ctx Γ' -> wf_ctx Γ ->
-  ctx_subtype Γ' (ctx_remove Γ i) ->
-  exists Γ'', Γ' = ctx_remove Γ'' i /\ ctx_subtype Γ'' Γ /\ wf_ctx Γ''.
-Proof.
-revert Γ' i. induction Γ; intros Γ' i wfg' wfg sty.
-+  simpl in sty. destruct i; inv sty; exists CtxØ;
-   aconstructor; constructor; apply SubtypeCtxØ || apply WfCtxØ. 
-+ simpl in sty. destruct i.
-  - exists (CtxU Γ' v). aconstructor. constructor. apply SubtypeCtxU. auto.
-    all: inv wfg. apply vsubtype_refl. assumption. apply WfCtxU; auto.
-  - inv sty. apply IHΓ in H2. all: try (inv wfg; inv wfg'; assumption).
-    destruct H2 as [Γ''[eq[wf]]]. subst. exists (CtxU Γ'' A).
-    aconstructor. constructor. apply SubtypeCtxU; auto.
-    apply WfCtxU. assumption. inv wfg'. assumption.
-Qed.
-
 
 
 Fixpoint ctx_subtype_vtype Γ Γ' v A (types : has_vtype Γ v A) {struct types}:
@@ -345,108 +321,112 @@ with ctx_subtype_wf_inst Γ Γ' I Γi (wf : wf_inst Γ I Γi) {struct wf}:
   wf_ctx Γ' -> ctx_subtype Γ' Γ -> wf_inst Γ' I Γi.
 
 Proof.
+all: rename ctx_subtype_vtype into VL.
+all: rename ctx_subtype_ctype into CL.
+all: rename ctx_subtype_htype into HL.
+all: rename ctx_subtype_respects into RL.
+all: rename ctx_subtype_veq into VEL.
+all: rename ctx_subtype_ceq into CEL.
+all: rename ctx_subtype_heq into HEL.
+all: rename ctx_subtype_wf_inst into WFL.
 {
-clear ctx_subtype_veq ctx_subtype_ceq ctx_subtype_heq ctx_subtype_wf_inst.
+clear VEL CEL HEL WFL.
 intros wf ctxsty.
-destruct types. induction H1; apply TypeV; try assumption.
+destruct types. induction H1; apply TypeV; eauto.
 + apply TypeUnit.
 + apply TypeInt.
-+ apply (ctx_subtype_get_rev _ _ A n) in ctxsty.
-  destruct ctxsty as [A' [gets]]. 2: assumption. 
-  eapply TypeVSubtype. 2: eauto.
-  apply TypeV. assumption. apply get_vtype_wf in gets as wfA'; eauto.
-  apply TypeVar. assumption.
-+ apply TypePair; apply (ctx_subtype_vtype Γ Γ'); assumption.
-+ apply TypeInl. apply (ctx_subtype_vtype Γ Γ'); assumption.
-+ apply TypeInr. apply (ctx_subtype_vtype Γ Γ'); assumption.
++ apply (ctx_subtype_get_rev _ _ A n) in ctxsty; auto.
+  destruct ctxsty as [A' [gets stya]].
+  eapply TypeVSubtype; eauto.
+  apply TypeV; eauto. apply get_vtype_wf in gets as wfA'; eauto.
+  apply TypeVar. auto.
++ apply TypePair; eauto.
++ apply TypeInl; eauto.
++ apply TypeInr; eauto.
 + apply TypeListNil.
-+ apply TypeListCons; apply (ctx_subtype_vtype Γ Γ'); assumption.
-+ apply TypeFun. eapply ctx_subtype_ctype; inv H0. eauto.
-  - apply WfCtxU; assumption.
-  - apply SubtypeCtxU. assumption. apply vsubtype_refl. assumption.
-+ apply TypeHandler. eapply ctx_subtype_ctype; inv H0; inv H6. eauto.
-  - apply WfCtxU; assumption.
-  - apply SubtypeCtxU. assumption. apply vsubtype_refl. assumption.
-  - eapply (ctx_subtype_htype Γ Γ'); assumption.
-  - eapply ctx_subtype_respects; eauto.
-+ eapply TypeVSubtype. 2 : eauto.
-  eapply (ctx_subtype_vtype Γ Γ'); assumption.
++ apply TypeListCons; eauto.
++ apply TypeFun. eapply CL; inv H0. eauto.
+  - apply WfCtxU; auto.
+  - apply SubtypeCtxU. auto. apply vsubtype_refl. auto.
++ apply TypeHandler; eauto. eapply CL; inv H0; inv H6; eauto.
+  - apply WfCtxU; auto.
+  - apply SubtypeCtxU. auto. apply vsubtype_refl. auto.
++ eapply TypeVSubtype; eauto.
 }{
-clear ctx_subtype_wf_inst ctx_subtype_respects.
-clear ctx_subtype_veq ctx_subtype_ceq ctx_subtype_heq.
+clear WFL RL VEL CEL HEL.
 intros wf ctxsty.
-destruct types. induction H1; apply TypeC; try assumption.
+destruct types. induction H1; apply TypeC; eauto.
 + apply TypeRet. eauto.
 + apply TypeAbsurd. eauto.
-+ eapply TypeΠMatch.
-  - eapply (ctx_subtype_vtype Γ Γ'); eauto.
-  - eapply ctx_subtype_ctype. exact H2. all: inv H2; inv H3; inv H7.
-    * apply WfCtxU. apply WfCtxU. all: assumption.
-    * apply SubtypeCtxU. apply SubtypeCtxU. assumption.
-      all: apply vsubtype_refl; assumption.
-+ eapply TypeΣMatch. eauto.
-  - eapply ctx_subtype_ctype. exact H2. all: inv H2; inv H4. 
-    * apply WfCtxU; assumption.
-    * apply SubtypeCtxU. exact ctxsty. apply vsubtype_refl. assumption.
-  - eapply ctx_subtype_ctype. exact H3. all: inv H3; inv H4. 
-    * apply WfCtxU; assumption.
-    * apply SubtypeCtxU. exact ctxsty. apply vsubtype_refl. assumption.
++ eapply TypeΠMatch; eauto.
+  eapply CL. eauto.
+  all: inv H2; inv H3; inv H7.
+  * apply WfCtxU. apply WfCtxU. all: auto.
+  * apply SubtypeCtxU. apply SubtypeCtxU. auto.
+    all: apply vsubtype_refl; auto.
++ eapply TypeΣMatch; eauto.
+  - eapply CL. eauto.
+    all: inv H2; inv H4. 
+    * apply WfCtxU; auto.
+    * apply SubtypeCtxU. exact ctxsty. apply vsubtype_refl. auto.
+  - eapply CL; eauto.
+    all: inv H3; inv H4. 
+    * apply WfCtxU; auto.
+    * apply SubtypeCtxU. exact ctxsty. apply vsubtype_refl. auto.
 + eapply TypeListMatch; eauto.
-  eapply ctx_subtype_ctype. eauto. all: inv H3; inv H4; inv H8.
+  eapply CL. eauto.
+  all: inv H3; inv H4; inv H8.
   * apply WfCtxU. apply WfCtxU. all: auto.
   * apply SubtypeCtxU. apply SubtypeCtxU. auto.
     all: apply vsubtype_refl; auto. 
-+ eapply TypeDoBind.
-  - eapply ctx_subtype_ctype; eauto.
-  - inv H1. inv H4. eapply ctx_subtype_ctype. eauto.
-    * apply WfCtxU; assumption.
-    * apply SubtypeCtxU. exact ctxsty. apply vsubtype_refl. assumption.
++ eapply TypeDoBind; eauto.
+  inv H1. inv H4. eapply CL. eauto.
+  * apply WfCtxU; auto.
+  * apply SubtypeCtxU. exact ctxsty. apply vsubtype_refl. auto.
 + eapply TypeApp; eauto.
 + eapply TypeHandle; eauto.
 + eapply TypeLetRec.
-  - eapply ctx_subtype_ctype. eauto. all: inv H2; inv H3.
+  - eapply CL. eauto.
+    all: inv H2; inv H3.
     * apply WfCtxU. apply WfCtxU. eauto. inv H8. all: eauto.
-    * apply SubtypeCtxU. apply SubtypeCtxU. exact ctxsty.
-      apply vsubtype_refl. inv H8. assumption. apply vsubtype_refl. assumption.
-  - eapply ctx_subtype_ctype. eauto. all: inv H2; inv H3.
-    * apply WfCtxU; assumption.
-    * apply SubtypeCtxU. exact ctxsty. apply vsubtype_refl. assumption.
-+ eapply TypeOp. eauto. eapply ctx_subtype_vtype; eauto.
-  eapply ctx_subtype_ctype. exact H3. all: inv H3; inv H4.
-  - apply WfCtxU; assumption.
-  - apply SubtypeCtxU. assumption. apply vsubtype_refl. assumption.
-+ eapply TypeCSubtype. 2: exact H2.
-  eapply ctx_subtype_ctype. all: eauto.
+    * apply SubtypeCtxU. apply SubtypeCtxU. eauto.
+      apply vsubtype_refl. inv H8. auto. apply vsubtype_refl. auto.
+  - eapply CL. eauto. all: inv H2; inv H3.
+    * apply WfCtxU; auto.
+    * apply SubtypeCtxU. eauto. apply vsubtype_refl. auto.
++ eapply TypeOp; eauto.
+  eapply CL. eauto. all: inv H3; inv H4.
+  - apply WfCtxU; auto.
+  - apply SubtypeCtxU. auto. apply vsubtype_refl. auto.
++ eapply TypeCSubtype; eauto.
 }{
-clear ctx_subtype_vtype ctx_subtype_respects ctx_subtype_veq.
-clear ctx_subtype_ceq ctx_subtype_heq ctx_subtype_wf_inst.
+clear VL RL VEL CEL HEL WFL.
 intros wf ctxsty.
-destruct types. induction H2; apply TypeH; try assumption.
+destruct types. induction H2; apply TypeH; eauto.
 + eapply TypeCasesØ.
-+ eapply TypeCasesU. assumption.
-  eapply ctx_subtype_htype. all: eauto.
-  eapply ctx_subtype_ctype. eauto.
++ eapply TypeCasesU. auto.
+  eapply HL. all: eauto.
+  eapply CL. eauto.
   all: inv H4; inv H5; inv H9.
-  - apply WfCtxU. apply WfCtxU. all: assumption.
-  - apply SubtypeCtxU. apply SubtypeCtxU. assumption.
-    all: apply vsubtype_refl; assumption.
+  - apply WfCtxU. apply WfCtxU. all: auto.
+  - apply SubtypeCtxU. apply SubtypeCtxU. auto.
+    all: apply vsubtype_refl; auto.
 }{
-clear ctx_subtype_vtype ctx_subtype_ctype ctx_subtype_htype.
-clear ctx_subtype_veq ctx_subtype_heq.
+clear VL CL HL VEL HEL.
 intros wf ctxsty.
 inv r. eapply Respects; auto. destruct H3.
 + eapply RespectEqsØ.
 + eapply RespectEqsU; eauto.
-  eapply ctx_subtype_ceq. eauto.
-  apply wf_join_ctxs. apply wf_join_ctxs. all: inv H2; auto.
-  apply wf_tctx_to_ctx; auto.   
-  apply ctx_subtype_join_ctxs. apply ctx_subtype_join_ctxs. 
-  all: auto; apply ctx_subtype_refl.
-  apply wf_tctx_to_ctx; auto. auto.
+  eapply CEL; eauto; inv H2.
+  - apply wf_join_ctxs. apply wf_join_ctxs. auto.
+    apply wf_tctx_to_ctx. all: auto.
+  - apply ctx_subtype_join_ctxs. apply ctx_subtype_join_ctxs. 
+    all: auto; apply ctx_subtype_refl.
+    apply wf_tctx_to_ctx; auto. auto.
 }{
 intros wf ctxsty.
 inv equals. destruct H1; apply Veq; eauto.
-all: clear ctx_subtype_vtype ctx_subtype_ctype ctx_subtype_htype.
+all: clear VL CL HL.
 + apply VeqSym. eauto.
 + eapply VeqTrans; eauto.
 + eapply ctx_subtype_get_rev in ctxsty as cget; eauto.
@@ -459,10 +439,12 @@ all: clear ctx_subtype_vtype ctx_subtype_ctype ctx_subtype_htype.
 + eapply VeqInr; eauto.
 + eapply VeqListNil.
 + eapply VeqListCons; eauto.
-+ eapply VeqFun. eapply ctx_subtype_ceq. eauto. all: inv H; inv H3.
++ eapply VeqFun. eapply CEL. eauto.
+  all: inv H; inv H3.
   - apply WfCtxU; auto.
   - apply SubtypeCtxU. auto. apply vsubtype_refl. auto.
-+ eapply VeqHandler. eapply ctx_subtype_ceq; inv H; inv H5; inv H8. all: eauto.
++ eapply VeqHandler. eapply CEL;
+  inv H; inv H5; inv H8. all: eauto.
   - apply WfCtxU; auto.
   - apply SubtypeCtxU. auto. apply vsubtype_refl. auto.
 + apply ηUnit.
@@ -470,45 +452,49 @@ all: clear ctx_subtype_vtype ctx_subtype_ctype ctx_subtype_htype.
 }{
 intros wf ctxsty.
 inv equals. destruct H1; apply Ceq; eauto.
-all: clear ctx_subtype_htype ctx_subtype_heq.
+all: clear HL HEL.
 + apply CeqSym. eauto.
 + eapply CeqTrans; eauto.
 + eapply CeqRet; eauto.
 + eapply CeqAbsurd; eauto.
 + eapply CeqΠMatch; eauto.
-  eapply ctx_subtype_ceq. eauto. all: inv H1; inv H3; inv H6.
-  - apply WfCtxU. apply WfCtxU. all: assumption.
-  - apply SubtypeCtxU. apply SubtypeCtxU. assumption.
-    all: apply vsubtype_refl; assumption.
-+ eapply CeqΣMatch; eauto; 
-  eapply ctx_subtype_ceq; eauto; inv H1; inv H4; inv H7.
-  - apply WfCtxU; assumption.
-  - apply SubtypeCtxU. assumption. apply vsubtype_refl. assumption.
-  - apply WfCtxU; assumption.
-  - apply SubtypeCtxU. assumption. apply vsubtype_refl. assumption.
-+ eapply CeqListMatch; eauto. 
-  eapply ctx_subtype_ceq; eauto; inv H1; inv H4.
-  - apply WfCtxU. apply WfCtxU. all: try assumption. inv H7. assumption.
-  - apply SubtypeCtxU. apply SubtypeCtxU. assumption.
-    all: apply vsubtype_refl. inv H7. all: assumption.
-+ eapply CeqDoBind; eauto. eapply ctx_subtype_ceq; eauto.
+  eapply CEL. eauto.
   all: inv H1; inv H3; inv H6.
-  - apply WfCtxU; assumption.
-  - apply SubtypeCtxU. assumption. apply vsubtype_refl. assumption.
+  - apply WfCtxU. apply WfCtxU. all: auto.
+  - apply SubtypeCtxU. apply SubtypeCtxU. auto.
+    all: apply vsubtype_refl; auto.
++ eapply CeqΣMatch; eauto; 
+  eapply CEL; eauto.
+  all: inv H1; inv H4; inv H7.
+  all: apply WfCtxU || apply SubtypeCtxU; auto.
+  all: apply vsubtype_refl; auto.
++ eapply CeqListMatch; eauto.
+  eapply CEL; eauto. 
+  all: inv H1; inv H4.
+  - apply WfCtxU. apply WfCtxU. all: auto. inv H7. auto.
+  - apply SubtypeCtxU. apply SubtypeCtxU. auto.
+    all: apply vsubtype_refl. inv H7. all: auto.
++ eapply CeqDoBind; eauto. eapply CEL; eauto.
+  all: inv H1; inv H3; inv H6.
+  - apply WfCtxU; auto.
+  - apply SubtypeCtxU. auto. apply vsubtype_refl. auto.
 + eapply CeqApp; eauto.
 + eapply CeqHandle; eauto.
 + eapply CeqLetRec.
-  - eapply ctx_subtype_ceq; eauto; inv H2; inv H4; inv H2.
+  - eapply CEL; eauto.
+    all: inv H2; inv H4; inv H2.
     * apply WfCtxU. apply WfCtxU. 2: inv H10. all: eauto.
-    * apply SubtypeCtxU. apply SubtypeCtxU. assumption.
+    * apply SubtypeCtxU. apply SubtypeCtxU. auto.
       all: apply vsubtype_refl. inv H10. all: auto.
-  - eapply ctx_subtype_ceq; eauto; inv H2; inv H4; inv H2.
-    * apply WfCtxU; assumption.
-    * apply SubtypeCtxU. assumption. apply vsubtype_refl. assumption.
+  - eapply CEL; eauto.
+    all: inv H2; inv H4; inv H2.
+    * apply WfCtxU; auto.
+    * apply SubtypeCtxU. auto. apply vsubtype_refl. auto.
 + eapply CeqOp; eauto.
-  eapply ctx_subtype_ceq; eauto; inv H3; inv H5; inv H3.
-  - apply WfCtxU; assumption.
-  - apply SubtypeCtxU. assumption. apply vsubtype_refl. assumption.
+  eapply CEL; eauto.
+  all: inv H3; inv H5; inv H3.
+  - apply WfCtxU; auto.
+  - apply SubtypeCtxU. auto. apply vsubtype_refl. auto.
 + eapply OOTB; eauto.
 + eapply βΠMatch.
 + eapply βΣMatch_Inl.
@@ -525,31 +511,33 @@ all: clear ctx_subtype_htype ctx_subtype_heq.
   apply ctx_subtype_len in ctxsty. omega.
   assert (wf_vtype (TyΠ A B)). 
   { inv H2. apply wf_ctx_insert_vtype in H3; auto. }
-  eapply ctx_subtype_ctype; eauto. apply wf_ctx_insert; eauto.
-  eapply ctx_subtype_insert_rev. 
-  auto. apply vsubtype_refl. auto.
+  eapply CL; eauto. 
+  - apply wf_ctx_insert; eauto.
+  - eapply ctx_subtype_insert. auto.
+    apply vsubtype_refl. auto.
 + eapply ηSum. apply ctx_subtype_len in ctxsty. omega.
   assert (wf_vtype (TyΣ A B)). 
   { inv H2. apply wf_ctx_insert_vtype in H3; auto. }
-  eapply ctx_subtype_ctype; eauto. apply wf_ctx_insert; eauto.
-  eapply ctx_subtype_insert_rev. 
-  auto. apply vsubtype_refl. auto.
+  eapply CL; eauto.
+  - apply wf_ctx_insert; eauto.
+  - eapply ctx_subtype_insert. auto.
+    apply vsubtype_refl. auto.
 + eapply ηDoBind.
 }{
 intros wf ctxsty.
 inv equals. destruct H4.
-all: clear ctx_subtype_vtype ctx_subtype_ctype.
-all: clear ctx_subtype_veq ctx_subtype_wf_inst.
+all: clear VL CL.
+all: clear VEL WFL.
 + eapply Heq. auto. exact H0. exact H1. all: eauto. eapply HeqSigØ.
 + eapply Heq. exact H. exact H0. all: eauto.
   eapply HeqSigU; eauto.
-  eapply ctx_subtype_ceq; eauto; inv H6; inv H8; inv H6; inv H14.
+  eapply CEL; eauto; inv H6; inv H8; inv H6; inv H14.
   - apply WfCtxU. apply WfCtxU. all: assumption.
   - apply SubtypeCtxU. apply SubtypeCtxU. assumption.
     all: apply vsubtype_refl; assumption.
 }{
-clear ctx_subtype_htype ctx_subtype_ctype ctx_subtype_veq ctx_subtype_ceq.
-clear ctx_subtype_respects ctx_subtype_heq.
+clear HL CL VEL CEL.
+clear RL HEL.
 intros wfc ctxsty.
 destruct wf.
 + eapply WfInstØ. auto.
@@ -565,10 +553,10 @@ Lemma wf_inst_subtype Γcheck I Γ Γ':
   wf_ctx Γ' -> ctx_subtype Γ Γ' -> wf_inst Γcheck I Γ ->
   wf_inst Γcheck I Γ'.
 Proof.
-intros wfc csty orig. revert Γ' wfc csty. 
-induction orig; intros Γ' wfc csty.
-+ inv csty. apply WfInstØ. auto.
-+ inv csty. apply WfInstU.
+intros wfc csty orig. revert Γ' wfc csty.
+induction orig; intros Γ' wfc csty; inv csty.
++ apply WfInstØ. auto.
++ apply WfInstU.
   - apply TypeV. inv H. auto. inv wfc. auto.
     eapply TypeVSubtype; eauto.
   - apply IHorig. inv wfc. auto. auto.
@@ -597,113 +585,139 @@ Proof.
 intro sty. inv sty. reflexivity.
 Qed. 
 
+
 Lemma subtype_shape_prod A B C : vsubtype C (TyΠ A B) -> 
-  exists A' B', C = (TyΠ A' B') /\ vsubtype A' A /\ vsubtype B' B.
+  exists A' B',
+    C = (TyΠ A' B') /\ vsubtype A' A /\ vsubtype B' B.
 Proof.
-intro orig. inv orig. exists A0. exists B0. auto.
+intro orig. inv orig. exists A0, B0. auto.
 Qed.
+
 
 Lemma subtype_shape_prod_rev A B C : vsubtype (TyΠ A B) C -> 
-  exists A' B', C = (TyΠ A' B') /\ vsubtype A A' /\ vsubtype B B'.
+  exists A' B',
+    C = (TyΠ A' B') /\ vsubtype A A' /\ vsubtype B B'.
 Proof.
-intro orig. inv orig. exists A'. exists B'. auto.
+intro orig. inv orig. exists A', B'. auto.
 Qed.
+
 
 Lemma subtype_shape_sum A B C : vsubtype C (TyΣ A B) -> 
-  exists A' B', C = (TyΣ A' B') /\ vsubtype A' A /\ vsubtype B' B.
+  exists A' B',
+    C = (TyΣ A' B') /\ vsubtype A' A /\ vsubtype B' B.
 Proof.
-intro orig. inv orig. exists A0. exists B0. auto.
+intro orig. inv orig. exists A0, B0. auto.
 Qed.
+
 
 Lemma subtype_shape_sum_rev A B C : vsubtype (TyΣ A B) C -> 
-  exists A' B', C = (TyΣ A' B') /\ vsubtype A A' /\ vsubtype B B'.
+  exists A' B',
+    C = (TyΣ A' B') /\ vsubtype A A' /\ vsubtype B B'.
 Proof.
-intro orig. inv orig. exists A'. exists B'. auto.
+intro orig. inv orig. exists A', B'. auto.
 Qed.
+
 
 Lemma subtype_shape_fun A B C : vsubtype C (TyFun A B) -> 
-  exists A' B', C = (TyFun A' B') /\ vsubtype A A' /\ csubtype B' B.
+  exists A' B',
+    C = (TyFun A' B') /\ vsubtype A A' /\ csubtype B' B.
 Proof.
-intro orig. inv orig. exists A0. exists C0. auto.
+intro orig. inv orig. exists A0, C0. auto.
 Qed.
 
+
 Lemma subtype_shape_list A B : vsubtype B (TyList A) -> 
-  exists A', B = (TyList A') /\ vsubtype A' A.
+  exists A',
+    B = (TyList A') /\ vsubtype A' A.
 Proof.
 intro orig. inv orig. exists A0. auto.
 Qed.
 
+
 Lemma subtype_shape_list_rev A B : vsubtype (TyList A) B -> 
-  exists A', B = (TyList A') /\ vsubtype A A'.
+  exists A',
+    B = (TyList A') /\ vsubtype A A'.
 Proof.
 intro orig. inv orig. exists A'. auto.
 Qed.
 
+
 Lemma subtype_shape_fun_rev A B C : vsubtype (TyFun A B) C -> 
-  exists A' B', C = (TyFun A' B') /\ vsubtype A' A /\ csubtype B B'.
+  exists A' B',
+    C = (TyFun A' B') /\ vsubtype A' A /\ csubtype B B'.
 Proof.
-intro orig. inv orig. exists A'. exists C'. auto.
+intro orig. inv orig. exists A', C'. auto.
 Qed.
+
 
 Lemma subtype_shape_handler A B C : vsubtype C (TyHandler A B) -> 
-  exists A' B', C = (TyHandler A' B') /\ csubtype A A' /\ csubtype B' B.
+  exists A' B',
+    C = (TyHandler A' B') /\ csubtype A A' /\ csubtype B' B.
 Proof.
-intro orig. inv orig. exists C0. exists D. auto.
+intro orig. inv orig. exists C0, D. auto.
 Qed.
 
+
 Lemma subtype_shape_handler_rev A B C : vsubtype (TyHandler A B) C -> 
-  exists A' B', C = (TyHandler A' B') /\ csubtype A' A /\ csubtype B B'.
+  exists A' B',
+    C = (TyHandler A' B') /\ csubtype A' A /\ csubtype B B'.
 Proof.
-intro orig. inv orig. exists C'. exists D'. auto.
+intro orig. inv orig. exists C', D'. auto.
 Qed.
+
 
 Lemma subtype_shape_cty A Σ E C : csubtype C (CTy A Σ E) ->
   exists A' Σ' E', 
     C = CTy A' Σ' E' /\ vsubtype A' A /\ sig_subtype Σ' Σ /\ eqs_subtype E' E.
 Proof.
-intro orig. inv orig. exists A0. exists Σ0. exists E0. auto.
+intro orig. inv orig. exists A0, Σ0, E0. auto.
 Qed.
   
 Lemma subtype_shape_cty_rev A Σ E C : csubtype (CTy A Σ E) C ->
-  exists A' Σ' E', C = 
-    CTy A' Σ' E' /\ vsubtype A A' /\ sig_subtype Σ Σ' /\ eqs_subtype E E'.
+  exists A' Σ' E', 
+    C = CTy A' Σ' E' /\ vsubtype A A' /\ sig_subtype Σ Σ' /\ eqs_subtype E E'.
 Proof.
-intro orig. inv orig. exists A'. exists Σ'. exists E'. auto.
+intro orig. inv orig. exists A', Σ', E'. auto.
 Qed.
 
 (* ==================== Template WF Subtyping ==================== *)
 
 Lemma wf_t_subtype_sig Γ Γ' Z T Σ Σ':
-  wf_t Γ Z T Σ -> sig_subtype Σ Σ' -> 
-  ctx_subtype Γ' Γ -> wf_sig Σ' -> wf_ctx Γ' ->
+  wf_t Γ Z T Σ ->
+  sig_subtype Σ Σ' -> ctx_subtype Γ' Γ ->
+  wf_sig Σ' -> wf_ctx Γ' ->
   wf_t Γ' Z T Σ'.
 Proof.
 intros orig. revert Γ'. induction orig; intros Γ' sty cty wfs wfc.
-+ eapply WfTApp. eapply ctx_subtype_vtype; eauto. assumption.
++ eapply WfTApp. eapply ctx_subtype_vtype; eauto. auto.
 + eapply WfTAbsurd. eapply ctx_subtype_vtype; eauto.
 + eapply WfTΠMatch. eapply ctx_subtype_vtype; eauto. inv H. inv H1.
   apply IHorig; auto. apply SubtypeCtxU. 
   apply SubtypeCtxU. 4: apply WfCtxU. 4: apply WfCtxU.
-  all: assumption || apply vsubtype_refl; auto.
-+ eapply WfTΣMatch. eapply ctx_subtype_vtype; eauto.  all: inv H; inv H1.
-  apply IHorig1; auto. 3: apply IHorig2; auto.
-  1: apply SubtypeCtxU. 4: apply SubtypeCtxU. 3: apply WfCtxU. 7: apply WfCtxU.
-  all: assumption || apply vsubtype_refl; auto.
-+ eapply WfTListMatch. eapply ctx_subtype_vtype; eauto. all: inv H.
-  apply IHorig1; auto. apply IHorig2; auto.
-  apply SubtypeCtxU. apply SubtypeCtxU. 4: apply WfCtxU. 4: apply WfCtxU.
+  all: try apply vsubtype_refl; auto.
++ eapply WfTΣMatch. eapply ctx_subtype_vtype; eauto. 
+  all: inv H; inv H1.
+  all: apply IHorig1 || apply IHorig2; auto.
+  all: apply SubtypeCtxU || apply WfCtxU; auto.
+  all: apply vsubtype_refl; auto.
++ eapply WfTListMatch. eapply ctx_subtype_vtype; eauto.
+  all: inv H.
+  all: apply IHorig1 || apply IHorig2; auto.
+  all: do 2 (try (apply SubtypeCtxU || apply WfCtxU)); auto.
   all: try apply vsubtype_refl; auto || inv H1; auto.
 + eapply sig_subtype_get_Some in H. 2: exact sty.
-  destruct H as [A'[B'[gets'[Asty]]]].
+  destruct H as [A'[B'[gets'[Asty Bsty]]]].
   eapply WfTOp. eauto.
   - eapply ctx_subtype_vtype; eauto. apply TypeV.
-    * inv H0. assumption.
-    * apply get_op_type_wf in gets'. inv gets'. all: assumption.
+    * inv H0. auto.
+    * apply get_op_type_wf in gets'. inv gets'. all: auto.
     * eapply TypeVSubtype; eauto.
   - apply IHorig; auto.
     * apply SubtypeCtxU; auto.
-    * apply get_op_type_wf in gets'. inv gets'. apply WfCtxU. all: assumption.
+    * apply get_op_type_wf in gets'. inv gets'.
+      apply WfCtxU. all: auto.
 Qed.
+
 
 Lemma wf_eqs_sig_subtype E Σ Σ':
   wf_eqs E Σ -> sig_subtype Σ Σ' -> wf_sig Σ' -> wf_eqs E Σ'.
@@ -742,21 +756,23 @@ Qed.
 (* Var *)
 Fixpoint shape_var_full Γ v n A (orig : has_vtype Γ v A) {struct orig} :
   v = Var n -> 
-  (exists A', get_vtype Γ n = Some A' /\ vsubtype A' A).
+  exists A', 
+    get_vtype Γ n = Some A' /\ vsubtype A' A.
 Proof.
 intros same.
 destruct orig. destruct H1; try discriminate.
 + clear shape_var_full.
-  exists A. inv same. aconstructor. apply vsubtype_refl. assumption.
-+ subst. eapply shape_var_full in H1. clear shape_var_full. 2: reflexivity.
-  destruct H1 as [A'' [gets]].
+  exists A. inv same. aconstructor. apply vsubtype_refl. auto.
++ subst. eapply shape_var_full in H1; eauto.
+  destruct H1 as [A'' [gets stya]].
   exists A''. aconstructor. eapply vsubtype_trans; eauto.
 Qed.
 
 
 Lemma shape_var Γ n A:
   has_vtype Γ (Var n) A -> 
-  (exists A', get_vtype Γ n = Some A' /\ vsubtype A' A).
+  exists A',
+    get_vtype Γ n = Some A' /\ vsubtype A' A.
 Proof.
 intro orig. apply (shape_var_full _ _ n A) in orig as shape; eauto.
 Qed.
@@ -766,14 +782,14 @@ Lemma shape_var_ctx_empty n A:
   has_vtype CtxØ (Var n) A -> False.
 Proof.
 intro orig.
-apply (shape_var_full _ _ n A) in orig as shape. 
-2: reflexivity. destruct shape as [A'[gets]]. simpl in gets. discriminate.
+apply (shape_var_full _ _ n A) in orig as shape; eauto.
+destruct shape as [A'[gets]]. simpl in gets. discriminate.
 Qed.
 
 
 (* Empty *)
 Fixpoint shape_empty_full Γ v A (orig : has_vtype Γ v A) {struct orig} :
-  A = TyØ -> (exists n, v = Var n).
+  A = TyØ -> exists n, v = Var n.
 Proof.
 intros samety.
 destruct orig. destruct H1; try discriminate. eauto.
@@ -782,7 +798,7 @@ Qed.
 
 
 Lemma shape_empty Γ v:
-  has_vtype Γ v TyØ -> (exists n, v = Var n).
+  has_vtype Γ v TyØ -> exists n, v = Var n.
 Proof.
 intro orig. apply (shape_empty_full _ _) in orig as shape; auto.
 Qed.
@@ -792,35 +808,40 @@ Qed.
 Fixpoint shape_prod_full Γ v A B ty (orig : has_vtype Γ v ty) {struct orig} :
   ty = TyΠ A B ->
   (exists n, v = Var n) \/
-  (exists v1 v2, v = Pair v1 v2 /\ has_vtype Γ v1 A /\ has_vtype Γ v2 B).
+  (exists v1 v2, 
+    v = Pair v1 v2 /\ has_vtype Γ v1 A /\ has_vtype Γ v2 B).
 Proof.
 intros same.
 destruct orig. destruct H1; try discriminate.
 + left. eauto.
 + right. inv same. eauto.
 + rewrite same in H2. apply subtype_shape_prod in H2. 
-  destruct H2 as [A'' [B'' [pity]]]. subst.
-  apply (shape_prod_full _ _ A'' B'') in H1. clear shape_prod_full. 
-  2: reflexivity. destruct H1. auto.
-  right. destruct H1 as [v1 [v2]].
-  exists v1. exists v2. destruct H1 as [s[vty1]]. destruct H2.
+  destruct H2 as [A'' [B'' [samety]]]. subst.
+  apply (shape_prod_full _ _ A'' B'') in H1; eauto. clear shape_prod_full. 
+  destruct H1. auto.
+  right. destruct H1 as [v1[v2[s[vty1]]]].
+  exists v1, v2. destruct H2.
   aconstructor. inv H0. constructor; apply TypeV.
-  all: assumption || eapply TypeVSubtype; eauto.
+  all: try eapply TypeVSubtype; eauto.
 Qed.
 
 
 Fixpoint shape_pair_full Γ v v1 v2 ty (orig : has_vtype Γ v ty) {struct orig} :
   v = Pair v1 v2 ->
-  (exists A B, ty = TyΠ A B /\ has_vtype Γ v1 A /\ has_vtype Γ v2 B).
+  exists A B, 
+    ty = TyΠ A B /\ has_vtype Γ v1 A /\ has_vtype Γ v2 B.
 Proof.
 intros same.
 destruct orig. destruct H1; try discriminate.
-+ clear shape_pair_full. exists A. exists B. inv same. auto.
-+ subst. apply (shape_pair_full _ _ v1 v2) in H1. clear shape_pair_full. 
-  2: reflexivity. destruct H1 as [A''[B''[ty[tyv1]]]]. subst.
-  apply subtype_shape_prod_rev in H2. destruct H2 as [A'''[B'''[s[sty1]]]].
-  exists A'''. exists B'''. subst. inv H0. aconstructor. constructor;
-  apply TypeV; try assumption; eapply TypeVSubtype; eauto.
++ clear shape_pair_full. exists A, B. inv same. auto.
++ subst. apply (shape_pair_full _ _ v1 v2) in H1; eauto.
+  clear shape_pair_full. 
+  destruct H1 as [A''[B''[ty[tyv1 tyv2]]]]. subst.
+  apply subtype_shape_prod_rev in H2.
+  destruct H2 as [A'''[B'''[s[stya styb]]]].
+  exists A''', B'''. aconstructor. 
+  subst. inv H0. constructor; apply TypeV; auto.
+  all: eapply TypeVSubtype; eauto.
 Qed.
 
 
@@ -849,57 +870,62 @@ destruct orig. destruct H1; try discriminate.
 + right. left. inv same. eauto.
 + right. right. inv same. eauto.
 + rewrite same in H2. apply subtype_shape_sum in H2. 
-  destruct H2 as [A'' [B'' [sigty]]]. subst. inv H0. destruct H2. 
+  destruct H2 as [A'' [B'' [sigty[stya styb]]]]. subst. inv H0. 
   apply (shape_sum_full _ _ A'' B'') in H1. clear shape_sum_full. 
-  2: reflexivity. destruct H1. auto. right. do 3 destruct H1; subst.
+  2: reflexivity. destruct H1. auto. right. do 3 destruct H0; subst.
   * left. exists x. aconstructor.
-    apply TypeV; try assumption. eapply TypeVSubtype; eauto.
+    apply TypeV; auto. eapply TypeVSubtype; eauto.
   * right. exists x. aconstructor.
-    apply TypeV; try assumption. eapply TypeVSubtype; eauto.
+    apply TypeV; auto. eapply TypeVSubtype; eauto.
 Qed.
 
 
 Fixpoint shape_inl_full Γ v A v' (orig : has_vtype Γ v A) {struct orig} :
   v = Inl v' ->
-  (exists A' B', A = TyΣ A' B' /\ has_vtype Γ v' A').
+  exists A' B',
+    A = TyΣ A' B' /\ has_vtype Γ v' A'.
 Proof.
 intros same. destruct orig. destruct H1; try discriminate.
 + inv same. eauto.
 + inv same. eapply shape_inl_full in H1. 2: reflexivity.
   destruct H1 as [A''[B''[tysum]]]. subst. 
-  apply subtype_shape_sum_rev in H2. destruct H2 as [A'''[B'''[tysum]]]. subst.
-  exists A'''. exists B'''. aconstructor. inv H0. destruct H2.
+  apply subtype_shape_sum_rev in H2.
+  destruct H2 as [A'''[B'''[tysum]]]. subst.
+  exists A''', B'''. aconstructor. inv H0. destruct H2.
   apply TypeV; auto. eapply TypeVSubtype; eauto.
 Qed.
 
+
 Fixpoint shape_inr_full Γ v A v' (orig : has_vtype Γ v A) {struct orig} :
   v = Inr v' ->
-  (exists A' B', A = TyΣ A' B' /\ has_vtype Γ v' B').
+  exists A' B',
+    A = TyΣ A' B' /\ has_vtype Γ v' B'.
 Proof.
 intros same. destruct orig. destruct H1; try discriminate.
 + inv same. eauto.
 + inv same. eapply shape_inr_full in H1. 2: reflexivity.
   destruct H1 as [A''[B''[tysum]]]. subst.
-  apply subtype_shape_sum_rev in H2. destruct H2 as [A'''[B'''[tysum]]]. subst.
-  exists A'''. exists B'''. aconstructor. inv H0. destruct H2.
+  apply subtype_shape_sum_rev in H2.
+  destruct H2 as [A'''[B'''[tysum]]]. subst.
+  exists A''', B'''. aconstructor. inv H0. destruct H2.
   apply TypeV; auto. eapply TypeVSubtype; eauto.
 Qed.
 
 
-Lemma shape_sum_inl Γ v A B :
+Lemma shape_inl Γ v A B :
   has_vtype Γ (Inl v) (TyΣ A B) -> has_vtype Γ v A.
 Proof.
-intro orig. apply (shape_sum_full _ _ A B) in orig as shape. 2: reflexivity.
+intro orig. apply (shape_sum_full _ _ A B) in orig as shape; eauto.
 destruct shape.
 + destruct H as [n same]. discriminate.
 + destruct H; destruct H; destruct H; inv H. auto.
 Qed.
 
 
-Lemma shape_sum_inr Γ v A B :
+Lemma shape_inr Γ v A B :
   has_vtype Γ (Inr v) (TyΣ A B) -> has_vtype Γ v B.
 Proof.
-intro orig. apply (shape_sum_full _ _ A B) in orig as shape. 2: reflexivity.
+intro orig. apply (shape_sum_full _ _ A B) in orig as shape; eauto.
 destruct shape.
 + destruct H as [n same]. discriminate.
 + destruct H; destruct H; destruct H; inv H. auto.
@@ -920,8 +946,8 @@ destruct orig. destruct H1; try discriminate.
 + right. right. inv same. eauto.
 + rewrite same in H2. apply subtype_shape_list in H2.
   destruct H2 as [A'' [sigty]]. subst. 
-  apply (shape_list_full _ _ A'') in H1. clear shape_list_full.
-  2: reflexivity. destruct H1. auto. right. destruct H1. auto.
+  apply (shape_list_full _ _ A'') in H1; eauto. clear shape_list_full.
+  destruct H1. auto. right. destruct H1. auto.
   destruct H1 as [w[ws[shape[tys1 tys2]]]].
   right. exists w, ws. aconstructor. constructor.
   all: apply TypeV; try assumption. inv H0. auto.
@@ -931,24 +957,26 @@ Qed.
 
 Fixpoint shape_list_cons_full Γ v A w ws (orig: has_vtype Γ v A) {struct orig}:
   v = ListCons w ws ->
-  (exists A', A = TyList A' /\ has_vtype Γ w A' /\ has_vtype Γ ws (TyList A')).
+  exists A',
+    A = TyList A' /\ has_vtype Γ w A' /\ has_vtype Γ ws (TyList A').
 Proof.
 intros same. destruct orig. destruct H1; try discriminate.
 + inv same. eauto.
 + inv same. eapply shape_list_cons_full in H1. 2: reflexivity.
   destruct H1 as [A''[same[tys1 tys2]]]. subst. 
-  apply subtype_shape_list_rev in H2. destruct H2 as [A'''[tyl]]. subst.
+  apply subtype_shape_list_rev in H2.
+  destruct H2 as [A'''[tyl]]. subst.
   exists A'''. aconstructor. constructor.
   all: apply TypeV; auto. inv H0. auto. 
   all: eapply TypeVSubtype; eauto. apply SubtypeTyList. auto.
 Qed.
 
 
-Lemma shape_list_cons Γ v vs A :
+Lemma shape_cons Γ v vs A :
   has_vtype Γ (ListCons v vs) (TyList A) -> 
   has_vtype Γ v A /\ has_vtype Γ vs (TyList A).
 Proof.
-intro orig. eapply (shape_list_cons_full) in orig as shape. 2: reflexivity.
+intro orig. eapply (shape_list_cons_full) in orig as shape; eauto.
 destruct shape as [A'[same[tys1 tys2]]]. inv same. auto.
 Qed.
 
@@ -956,20 +984,23 @@ Qed.
 (* Function *)
 Fixpoint shape_fun_full Γ v c ty (orig : has_vtype Γ v ty) {struct orig} :
   v = Fun c ->
-  (exists A C, ty = TyFun A C /\ has_ctype (CtxU Γ A) c C).
+  exists A C,
+    ty = TyFun A C /\ has_ctype (CtxU Γ A) c C.
 Proof.
 intros same. destruct orig. destruct H1; try discriminate.
 + inv same. eauto.
-+ subst. apply (shape_fun_full _ _ c) in H1. clear shape_fun_full. 
-  2: reflexivity. destruct H1 as [A''[C''[s]]]. subst.
-  apply subtype_shape_fun_rev in H2. destruct H2 as [A'''[C'''[s[vty1]]]].
-  exists A'''. exists C'''. aconstructor. subst. inv H0.
++ subst. apply (shape_fun_full _ _ c) in H1; eauto. clear shape_fun_full. 
+  destruct H1 as [A''[C''[s]]]. subst.
+  apply subtype_shape_fun_rev in H2.
+  destruct H2 as [A'''[C'''[s[vty1]]]].
+  exists A''', C'''. aconstructor. subst. inv H0.
   apply TypeC; auto.
-  * apply WfCtxU; assumption.
+  * apply WfCtxU; auto.
   * eapply TypeCSubtype. 2: eauto.
-    eapply ctx_subtype_ctype. eauto. apply WfCtxU; assumption.
-    apply SubtypeCtxU. apply ctx_subtype_refl. all: assumption.
+    eapply ctx_subtype_ctype. eauto. apply WfCtxU; auto.
+    apply SubtypeCtxU. apply ctx_subtype_refl. all: auto.
 Qed.
+
 
 Fixpoint shape_tyfun_full Γ v A C ty (orig : has_vtype Γ v ty) {struct orig} :
   ty = TyFun A C ->
@@ -980,21 +1011,21 @@ intros same. destruct orig. destruct H1; try discriminate. eauto.
 + inv same. eauto. 
 + rewrite same in H2. apply subtype_shape_fun in H2. 
   destruct H2 as [A'' [C'' [funty]]]. subst. 
-  apply (shape_tyfun_full _ _ A'' C'') in H1. clear shape_tyfun_full. 
-  2: reflexivity. destruct H1. auto.
-  right. destruct H1 as [c']. 
+  apply (shape_tyfun_full _ _ A'' C'') in H1; eauto. clear shape_tyfun_full. 
+  destruct H1. auto. right. destruct H1 as [c']. 
   exists c'.
   destruct H1. aconstructor. apply TypeC; inv H0; auto.
-  * apply WfCtxU; assumption.
+  * apply WfCtxU; auto.
   * destruct H2. eapply TypeCSubtype. 2: eauto.
-    eapply ctx_subtype_ctype. eauto. apply WfCtxU; assumption.
-    apply SubtypeCtxU. apply ctx_subtype_refl. all: assumption.
+    eapply ctx_subtype_ctype. eauto. apply WfCtxU; auto.
+    apply SubtypeCtxU. apply ctx_subtype_refl. all: auto.
 Qed.
+
 
 Lemma shape_fun Γ c A C :
   has_vtype Γ (Fun c) (TyFun A C) -> has_ctype (CtxU Γ A) c C.
 Proof.
-intro orig. apply (shape_tyfun_full _ _ A C) in orig as shape. 2: reflexivity.
+intro orig. apply (shape_tyfun_full _ _ A C) in orig as shape; eauto.
 destruct shape.
 + destruct H. discriminate.
 + destruct H as [c'[same tys]]. inv same. auto.
@@ -1005,33 +1036,34 @@ Qed.
 Fixpoint shape_handler_full Γ v c_r h ty
   (orig : has_vtype Γ v ty) {struct orig} :
   v = Handler c_r h ->
-  (exists A Σ E D Σ' D', ty = TyHandler (CTy A Σ E) D /\ 
-    has_ctype (CtxU Γ A) c_r D /\ has_htype Γ h Σ' D' /\ respects Γ h Σ' D' E
-    /\ sig_subtype Σ Σ' /\ csubtype D' D).
+  exists A Σ E D Σ' D',
+    ty = TyHandler (CTy A Σ E) D /\ 
+    has_ctype (CtxU Γ A) c_r D /\ has_htype Γ h Σ' D' /\ 
+    respects Γ h Σ' D' E /\ sig_subtype Σ Σ' /\ csubtype D' D.
 Proof.
 intros same. destruct orig. destruct H1; try discriminate.
-+ clear shape_handler_full. exists A. exists Σ. exists E. exists D.
-  exists Σ. exists D. inv same. do 3 aconstructor.
++ clear shape_handler_full. exists A, Σ, E, D, Σ, D.
+  inv same. do 3 aconstructor.
   inv H0. inv H6. aconstructor. constructor.
   apply sig_subtype_refl. auto. apply csubtype_refl. auto.
-+ subst. apply (shape_handler_full _ _ c_r h) in H1.
-  clear shape_handler_full. 2: reflexivity.
++ subst. apply (shape_handler_full _ _ c_r h) in H1; eauto.
+  clear shape_handler_full.
   destruct H1 as [A''[Σ[E[D[Σ'[D'[same[cty[hty[r[sty]]]]]]]]]]]. subst.
-  apply subtype_shape_handler_rev in H2. destruct H2 as [C' [D''[same[sty']]]].
-  subst. apply subtype_shape_cty in sty'.
+  apply subtype_shape_handler_rev in H2.
+  destruct H2 as [C' [D''[same[sty']]]]. subst.
+  apply subtype_shape_cty in sty'.
   destruct sty' as [A'''[Σ'''[E'''[same]]]]. subst.
-  exists A'''. exists Σ'''. exists E'''. exists D''. exists Σ'. exists D'.
-  aconstructor. constructor. 2: constructor. 3: constructor. 4: constructor.
-  - eapply ctx_subtype_ctype. 
-    3 : apply SubtypeCtxU. 3: apply ctx_subtype_refl. 3: assumption.
-    3 : destruct H3; eauto.
-    * apply TypeC. inv cty. assumption. inv H0. assumption.
+  exists A''', Σ''', E''', D'', Σ', D'.
+  aconstructor. aconstructor. 2: aconstructor. 2: constructor. 3: constructor.
+  - eapply ctx_subtype_ctype.
+    3 : apply SubtypeCtxU; apply ctx_subtype_refl || destruct H3; eauto.
+    * apply TypeC. inv cty. auto. inv H0. auto.
       eapply TypeCSubtype; eauto.
-    * inv H0. inv H6. apply WfCtxU; assumption.
-  - assumption.
+    * inv H0. inv H6. apply WfCtxU; auto.
   - eapply respects_eqs_subtype; destruct H3 as [_[e]]; eauto. 
-    inv H0. inv H6. eapply wf_eqs_sig_subtype; eauto.
-    eapply sig_subtype_trans; eauto. inv hty. assumption.
+    inv H0. inv H6.
+    eapply wf_eqs_sig_subtype; eauto.
+    eapply sig_subtype_trans; eauto. inv hty. auto.
   - destruct H3 as [_[a]]. eapply sig_subtype_trans; eauto.
   - eapply csubtype_trans; eauto.
 Qed.
@@ -1041,45 +1073,52 @@ Fixpoint shape_tyhandler_full Γ v A Σ E D ty
   (orig : has_vtype Γ v ty) {struct orig} :
   ty = TyHandler (CTy A Σ E) D ->
   (exists n, v = Var n) \/
-  (exists c_r h Σ' D', v = Handler c_r h /\ has_ctype (CtxU Γ A) c_r D' 
-    /\ has_htype Γ h Σ' D' /\ respects Γ h Σ' D' E
-    /\ sig_subtype Σ Σ' /\ csubtype D' D).
+  (exists c_r h Σ' D', 
+    v = Handler c_r h /\ has_ctype (CtxU Γ A) c_r D' /\ 
+    has_htype Γ h Σ' D' /\ respects Γ h Σ' D' E /\
+    sig_subtype Σ Σ' /\ csubtype D' D).
 Proof.
 intros same. destruct orig. destruct H1; try discriminate. eauto.
 + clear shape_tyhandler_full. right.
-  exists c_ret. exists h. exists Σ. exists D.
+  exists cr, h, Σ, D.
   inv same. do 4 aconstructor. constructor; inv H2.
-  apply sig_subtype_refl. assumption. apply csubtype_refl. assumption.
+  apply sig_subtype_refl. auto. apply csubtype_refl. auto.
 + rewrite same in *. apply subtype_shape_handler in H2. 
-  destruct H2 as [C' [D' [hty]]]. destruct H2. subst.
+  destruct H2 as [C' [D' [hty[csty dsty]]]]. subst.
   destruct C' as [A' Σ' E'].
-  apply (shape_tyhandler_full _ _ A' Σ' E' D') in H1.
-  clear shape_tyhandler_full. 2: reflexivity. destruct H1. auto.
+  apply (shape_tyhandler_full _ _ A' Σ' E' D') in H1; eauto. 
+  destruct H1. auto.
   right. destruct H1 as [cr[h[Σ''[D''[same[cty[hty[r]]]]]]]].
-  exists cr. exists h. exists Σ''. exists D''.
+  exists cr, h, Σ'', D''.
   aconstructor. constructor; destruct H1.
   - eapply ctx_subtype_ctype. eauto.
-    inv H0. inv H7. apply WfCtxU; assumption.
-    apply SubtypeCtxU. apply ctx_subtype_refl. all: inv H2; assumption.
-  - inv H2. aconstructor. constructor.  eapply respects_eqs_subtype; eauto. 
-    inv H0. inv H6. eapply wf_eqs_sig_subtype; eauto.
-    eapply sig_subtype_trans; eauto. inv hty. assumption. constructor.
-    eapply sig_subtype_trans; eauto. eapply csubtype_trans; eauto.
+    inv H0. inv H5.
+    apply WfCtxU; auto.
+    apply SubtypeCtxU. apply ctx_subtype_refl.
+    all: inv csty; auto.
+  - inv csty. aconstructor. constructor. 
+    * eapply respects_eqs_subtype; eauto.
+      inv H0. inv H5. eapply wf_eqs_sig_subtype; eauto.
+      eapply sig_subtype_trans; eauto. inv hty. auto.
+    * constructor. eapply sig_subtype_trans; eauto.
+      eapply csubtype_trans; eauto.
 Qed.
+
 
 Lemma shape_handler Γ c_r h A Σ E D:
   has_vtype Γ (Handler c_r h) (TyHandler (CTy A Σ E) D) ->
-    (exists Σ' D', has_ctype (CtxU Γ A) c_r D' /\ has_htype Γ h Σ' D'
-      /\ respects Γ h Σ' D' E /\ sig_subtype Σ Σ' /\ csubtype D' D).
+  exists Σ' D',
+    has_ctype (CtxU Γ A) c_r D' /\ has_htype Γ h Σ' D' /\
+    respects Γ h Σ' D' E /\ sig_subtype Σ Σ' /\ csubtype D' D.
 Proof.
 intro orig.
-apply (shape_tyhandler_full _ _ A Σ E D) in orig as shape. 2: reflexivity.
+apply (shape_tyhandler_full _ _ A Σ E D) in orig as shape; eauto.
 destruct shape.
 + destruct H as [n]. discriminate.
 + do 5 (destruct H). inv H. eauto.
 Qed.
 
-(* ========================= Handler Cases Shapes ========================= *)
+(* ==================== Handler Cases Shapes ==================== *)
 
 Lemma h_has_case Γ h Σ D op A_op B_op:
   has_htype Γ h Σ D ->
@@ -1091,29 +1130,31 @@ revert Γ Σ. induction h; intros Γ Σ typed gets; inv typed; inv H2.
 + simpl in *. destruct (op==o); eauto.
 Qed.
 
-Lemma case_has_type Γ h Σ D op Aop Bop c_op:
-  has_htype Γ h Σ D -> get_op_type Σ op = Some (Aop, Bop) ->
-  get_case h op = Some c_op ->
-  has_ctype (CtxU (CtxU Γ (TyFun Bop D)) Aop) c_op D.
+Lemma case_has_type Γ h Σ D op A B c:
+  has_htype Γ h Σ D -> get_op_type Σ op = Some (A, B) ->
+  get_case h op = Some c ->
+  has_ctype (CtxU (CtxU Γ (TyFun B D)) A) c D.
 Proof.
 revert Σ. induction h; intros Σ tys gets finds.
 simpl in finds. discriminate.
 simpl in *. destruct (op==o).
-- inv tys. inv H2. simpl in *. destruct (o==o). 2: (destruct n; reflexivity).
-  inv finds. inv gets. assumption.
+- inv tys. inv H2. simpl in *. destruct (o==o).
+  + inv finds. inv gets. auto.
+  + destruct n; auto.
 - inv tys. inv H2. eapply IHh; eauto.
-  simpl in gets. destruct (op==o); eauto. rewrite e in n. destruct n. auto.
+  simpl in gets. destruct (op==o); eauto.
+  rewrite e in n. destruct n. auto.
 Qed. 
 
 (* ==================== Computation Shapes ==================== *)
 
 (* Return *)
 Fixpoint shape_ret_full Γ c C v A Σ E (orig : has_ctype Γ c C) {struct orig} :
-  c = (Ret v) -> C = (CTy A Σ E) -> 
+  c = Ret v -> C = CTy A Σ E -> 
   has_vtype Γ v A.
 Proof.  
 intros same samety. destruct orig. destruct H1; try discriminate.
-+ clear shape_ret_full. inv same. inv samety. assumption.
++ clear shape_ret_full. inv same. inv samety. auto.
 + destruct C as (A', Σ', E').
   apply (shape_ret_full _ _ (CTy A' Σ' E') v A' Σ' E') in H1;
   clear shape_ret_full; auto. subst.
@@ -1130,9 +1171,10 @@ Qed.
 
 (* Return *)
 Fixpoint shape_absurd_full Γ c C v (orig : has_ctype Γ c C) {struct orig} :
-  c = (Absurd v) -> has_vtype Γ v TyØ.
+  c = Absurd v -> has_vtype Γ v TyØ.
 Proof.  
-intros same. destruct orig. destruct H1; try discriminate; inv same; auto.
+intros same. destruct orig. 
+destruct H1; try discriminate; inv same; auto.
 apply (shape_absurd_full _ _ _ v) in H1; auto.
 Qed.
 
@@ -1147,21 +1189,23 @@ Qed.
 (* ΠMatch *)
 Fixpoint shape_prodmatch_full Γ c v c' C
   (orig : has_ctype Γ c C) {struct orig} :
-  c = (ΠMatch v c') ->
-  (exists A B, has_vtype Γ v (TyΠ A B) /\ has_ctype (CtxU (CtxU Γ A) B) c' C).
+  c = ΠMatch v c' ->
+  exists A B,
+    has_vtype Γ v (TyΠ A B) /\ has_ctype (CtxU (CtxU Γ A) B) c' C.
 Proof.  
 intros same. destruct orig. destruct H1; try discriminate; inv same.
-+ clear shape_prodmatch_full. exists A. exists B. auto.
-+ apply (shape_prodmatch_full _ _ v c') in H1; clear shape_prodmatch_full. 
-  2: reflexivity. destruct H1 as [A' [B' [vty]]].
-  exists A'. exists B'. aconstructor.
++ clear shape_prodmatch_full. exists A, B. auto.
++ apply (shape_prodmatch_full _ _ v c') in H1; eauto.
+  destruct H1 as [A' [B' [vty]]].
+  exists A', B'. aconstructor.
   apply TypeC; try (inv H1; assumption). eapply TypeCSubtype; eauto.
 Qed.
 
 
 Fixpoint shape_prodmatch Γ v c C :
   has_ctype Γ (ΠMatch v c) C ->
-  (exists A B, has_vtype Γ v (TyΠ A B) /\  has_ctype (CtxU (CtxU Γ A) B) c C).
+  exists A B,
+    has_vtype Γ v (TyΠ A B) /\  has_ctype (CtxU (CtxU Γ A) B) c C.
 Proof.
 intro orig. apply (shape_prodmatch_full _ _ v c) in orig; auto.
 Qed.
@@ -1170,16 +1214,16 @@ Qed.
 (* ΣMatch *)
 Fixpoint shape_summatch_full Γ c v c1 c2 C
   (orig : has_ctype Γ c C) {struct orig} :
-  c = (ΣMatch v c1 c2) ->
-  (exists A B, has_vtype Γ v (TyΣ A B) /\
-    has_ctype (CtxU Γ A) c1 C /\ has_ctype (CtxU Γ B) c2 C).
+  c = ΣMatch v c1 c2 ->
+  exists A B,
+    has_vtype Γ v (TyΣ A B) /\
+    has_ctype (CtxU Γ A) c1 C /\ has_ctype (CtxU Γ B) c2 C.
 Proof.  
 intros same. destruct orig. destruct H1; try discriminate.
-+ clear shape_summatch_full. inv same. exists A. exists B. auto.
-+ apply (shape_summatch_full _ _ v c1 c2) in H1;
-  clear shape_summatch_full. 2: assumption.
++ clear shape_summatch_full. inv same. exists A, B. auto.
++ apply (shape_summatch_full _ _ v c1 c2) in H1; eauto.
   destruct H1 as [A' [B' [vty]]].
-  exists A'. exists B'. aconstructor.
+  exists A', B'. aconstructor.
   inv H1. constructor; apply TypeC; auto.
   all: (eapply TypeCSubtype; eauto) || (inv H3; inv H4; assumption).
 Qed.
@@ -1187,8 +1231,9 @@ Qed.
 
 Fixpoint shape_summatch Γ v c1 c2 C :
   has_ctype Γ (ΣMatch v c1 c2) C ->
-  (exists A B, has_vtype Γ v (TyΣ A B) /\
-    has_ctype (CtxU Γ A) c1 C /\ has_ctype (CtxU Γ B) c2 C).
+  exists A B,
+    has_vtype Γ v (TyΣ A B) /\
+    has_ctype (CtxU Γ A) c1 C /\ has_ctype (CtxU Γ B) c2 C.
 Proof.
 intro orig. apply (shape_summatch_full _ _ v c1 c2) in orig; auto.
 Qed.
@@ -1197,14 +1242,14 @@ Qed.
 (* ListMatch *)
 Fixpoint shape_listmatch_full Γ c v c1 c2 C
   (orig : has_ctype Γ c C) {struct orig} :
-  c = (ListMatch v c1 c2) ->
-  (exists A, has_vtype Γ v (TyList A) /\
-    has_ctype Γ c1 C /\ has_ctype (CtxU (CtxU Γ A) (TyList A)) c2 C).
+  c = ListMatch v c1 c2 ->
+  exists A,
+    has_vtype Γ v (TyList A) /\
+    has_ctype Γ c1 C /\ has_ctype (CtxU (CtxU Γ A) (TyList A)) c2 C.
 Proof.
 intros same. destruct orig. destruct H1; try discriminate.
 + clear shape_listmatch_full. inv same. exists A. auto.
-+ apply (shape_listmatch_full _ _ v c1 c2) in H1;
-  clear shape_listmatch_full. 2: assumption.
++ apply (shape_listmatch_full _ _ v c1 c2) in H1; eauto.
   destruct H1 as [A' [vty[ty1 ty2]]].
   exists A'. aconstructor. constructor; apply TypeC; auto.
   all: (eapply TypeCSubtype || inv ty2); eauto.
@@ -1213,57 +1258,60 @@ Qed.
 
 Fixpoint shape_listmatch Γ v c1 c2 C:
   has_ctype Γ (ListMatch v c1 c2) C ->
-  (exists A, has_vtype Γ v (TyList A) /\
-    has_ctype Γ c1 C /\ has_ctype (CtxU (CtxU Γ A) (TyList A)) c2 C).
+  exists A,
+    has_vtype Γ v (TyList A) /\
+    has_ctype Γ c1 C /\ has_ctype (CtxU (CtxU Γ A) (TyList A)) c2 C.
 Proof.
 intro orig. eapply shape_listmatch_full in orig; eauto.
 Qed.
 
+
 (* App *)
 Fixpoint shape_app_full Γ c v1 v2 C (orig : has_ctype Γ c C) {struct orig} :
-  c = (App v1 v2) ->
-  (exists A, has_vtype Γ v1 (TyFun A C) /\ has_vtype Γ v2 A).
+  c = App v1 v2 ->
+  exists A,
+    has_vtype Γ v1 (TyFun A C) /\ has_vtype Γ v2 A.
 Proof.  
 intros same. destruct orig. destruct H1; try discriminate.
 + clear shape_app_full. inv same. exists A. auto.
-+ apply (shape_app_full _ _ v1 v2) in H1;
-  clear shape_app_full. 2: assumption.
++ apply (shape_app_full _ _ v1 v2) in H1; eauto.
   destruct H1 as [A' [fty]].
   exists A'. aconstructor. apply TypeV. auto.
-  - inv fty. inv H4. apply WfTyFun; assumption.
+  - inv fty. inv H4. apply WfTyFun; auto.
   - eapply TypeVSubtype. exact fty. apply SubtypeTyFun.
-    apply vsubtype_refl. inv fty. inv H4. all: assumption.
+    apply vsubtype_refl. inv fty. inv H4. all: auto.
 Qed.
 
 
 Fixpoint shape_app Γ c v C :
   has_ctype Γ (App (Fun c) v) C ->
-  (exists A, has_ctype (CtxU Γ A) c C /\ has_vtype Γ v A).
+  exists A, has_ctype (CtxU Γ A) c C /\ has_vtype Γ v A.
 Proof.
-intro orig. eapply (shape_app_full _ _ (Fun c) v C) in orig.
-2: reflexivity. destruct orig as [A [fty]]. apply shape_fun in fty. eauto.
+intro orig. eapply (shape_app_full _ _ (Fun c) v C) in orig; eauto.
+destruct orig as [A [fty]]. apply shape_fun in fty. eauto.
 Qed.
 
 
 (* Handle *)
 Fixpoint shape_handle_full Γ c v c' C (orig : has_ctype Γ c C) {struct orig} :
-  c = (Handle v c') ->
-  (exists C', has_vtype Γ v (TyHandler C' C) /\ has_ctype Γ c' C').
+  c = Handle v c' ->
+  exists C',
+    has_vtype Γ v (TyHandler C' C) /\ has_ctype Γ c' C'.
 Proof.  
 intros same. destruct orig. destruct H1; try discriminate.
 + clear shape_handle_full. inv same. exists C. auto.
 + apply (shape_handle_full _ _ v c') in H1; auto.
   destruct H1 as [D [vty]].
   exists D. aconstructor. inv H1.
-  apply TypeV. assumption. apply WfTyHandler; auto.
+  apply TypeV. auto. apply WfTyHandler; auto.
   eapply TypeVSubtype. exact vty.
-  apply SubtypeTyHandler. apply csubtype_refl. all: assumption.
+  apply SubtypeTyHandler. apply csubtype_refl. all: auto.
 Qed.
 
 
 Fixpoint shape_handle Γ v c D :
   has_ctype Γ (Handle v c) D ->
-  (exists C, has_vtype Γ v (TyHandler C D) /\ has_ctype Γ c C).
+  exists C, has_vtype Γ v (TyHandler C D) /\ has_ctype Γ c C.
 Proof.
 intro orig. eapply (shape_handle_full _ _ v c D) in orig; auto.
 Qed.
@@ -1272,24 +1320,25 @@ Qed.
 (* LetRec *)
 Fixpoint shape_letrec_full Γ c c1 c2 D
   (orig : has_ctype Γ c D) {struct orig} :
-  c = (LetRec c1 c2) ->
-  (exists A C, has_ctype (CtxU (CtxU Γ A) (TyFun A C)) c1 C /\ 
-    has_ctype (CtxU Γ (TyFun A C)) c2 D).
+  c = LetRec c1 c2 ->
+  exists A C,
+    has_ctype (CtxU (CtxU Γ A) (TyFun A C)) c1 C /\ 
+    has_ctype (CtxU Γ (TyFun A C)) c2 D.
 Proof.  
 intros same. destruct orig. destruct H1; try discriminate.
-+ clear shape_letrec_full. inv same. exists A. exists C. auto.
-+ apply (shape_letrec_full _ _ c1 c2) in H1;
-  clear shape_letrec_full. 2: assumption.
++ clear shape_letrec_full. inv same. exists A, C. auto.
++ apply (shape_letrec_full _ _ c1 c2) in H1; eauto.
   destruct H1 as [A' [C'' [cty]]]. inv H1.
-  exists A'. exists C''. aconstructor. apply TypeC; auto.
+  exists A', C''. aconstructor. apply TypeC; auto.
   eapply TypeCSubtype. 2: eauto. apply TypeC; assumption.
 Qed.
 
 
 Fixpoint shape_letrec Γ c1 c2 D :
   has_ctype Γ (LetRec c1 c2) D ->
-  (exists A C, has_ctype (CtxU (CtxU Γ A) (TyFun A C)) c1 C /\ 
-    has_ctype (CtxU Γ (TyFun A C)) c2 D).
+  exists A C, 
+    has_ctype (CtxU (CtxU Γ A) (TyFun A C)) c1 C /\ 
+    has_ctype (CtxU Γ (TyFun A C)) c2 D.
 Proof.
 intro orig. eapply (shape_letrec_full _ _ c1 c2 D) in orig; auto.
 Qed.
@@ -1298,17 +1347,18 @@ Qed.
 (* DoBind *)
 Fixpoint shape_dobind_full Γ c C c1 c2 A Σ E
   (orig : has_ctype Γ c C) {struct orig} :
-  c = (DoBind c1 c2) -> C = (CTy A Σ E) ->
-  (exists A', has_ctype Γ c1 (CTy A' Σ E) /\ has_ctype (CtxU Γ A') c2 C).
+  c = DoBind c1 c2 -> C = CTy A Σ E ->
+  exists A',
+    has_ctype Γ c1 (CTy A' Σ E) /\ has_ctype (CtxU Γ A') c2 C.
 Proof.  
 intros same samety. destruct orig. destruct H1; try discriminate; inv same.
 + inv samety. clear shape_dobind_full. exists A0. auto.
 + destruct C as (A', Σ', E').
-  apply (shape_dobind_full _ _ (CTy A' Σ' E') c1 c2 A' Σ' E') in H1;
-  clear shape_dobind_full; auto. destruct H1 as [A'' [cty]].
+  apply (shape_dobind_full _ _ (CTy A' Σ' E') c1 c2 A' Σ' E') in H1; eauto.
+  destruct H1 as [A'' [cty]].
   exists A''. constructor.
-  - apply TypeC. assumption. inv cty. inv H0. inv H4.
-    apply WfCTy; assumption. eapply TypeCSubtype. exact cty.
+  - apply TypeC. auto. inv cty. inv H0. inv H4.
+    apply WfCTy; auto. eapply TypeCSubtype. exact cty.
     inv H2. inv cty. inv H3. apply SubtypeCTy; auto. apply vsubtype_refl; auto.
   - apply TypeC. inv H1. 3: eapply TypeCSubtype. all: eauto.
 Qed.
@@ -1316,8 +1366,9 @@ Qed.
 
 Fixpoint shape_dobind Γ c1 c2 A Σ E :
   has_ctype Γ (DoBind c1 c2) (CTy A Σ E) ->
-  (exists A', has_ctype Γ c1 (CTy A' Σ E) /\ 
-    has_ctype (CtxU Γ A') c2 (CTy A Σ E)).
+  exists A',
+    has_ctype Γ c1 (CTy A' Σ E) /\ 
+    has_ctype (CtxU Γ A') c2 (CTy A Σ E).
 Proof.  
 intro orig. eapply (shape_dobind_full _ _ _ c1 c2 A Σ E) in orig; auto.
 Qed.
@@ -1326,32 +1377,35 @@ Qed.
 (* Op *)
 Fixpoint shape_op_full Γ c C op v c' A Σ E
   (orig : has_ctype Γ c C) {struct orig} :
-  c = (Op op v c') -> C = (CTy A Σ E) ->
-  (exists Aop Bop, get_op_type Σ op = Some (Aop, Bop) /\
-    has_vtype Γ v Aop /\  has_ctype (CtxU Γ Bop) c' C).
+  c = Op op v c' -> C = CTy A Σ E ->
+  exists Aop Bop,
+    get_op_type Σ op = Some (Aop, Bop) /\
+    has_vtype Γ v Aop /\  has_ctype (CtxU Γ Bop) c' C.
 Proof.  
 intros same samety. destruct orig. destruct H1; try discriminate; inv same.
 + inv samety. eauto.
 + destruct C as (A', Σ', E').
-  apply (shape_op_full _ _ (CTy A' Σ' E') op v c' A' Σ' E') in H1;
-  clear shape_op_full; eauto. destruct H1 as [A'' [B'' [g [vty]]]]. inv H2.
-  eapply sig_subtype_get_Some in g; eauto. destruct g as [A'''[B'''[g'[s']]]].
-  exists A'''. exists B'''. aconstructor. constructor.
-  - apply TypeV. assumption. apply get_op_type_wf in g'. destruct g'.
-    assumption. inv H0. assumption. eapply TypeVSubtype; eauto.
+  apply (shape_op_full _ _ (CTy A' Σ' E') op v c' A' Σ' E') in H1; eauto.
+  destruct H1 as [A'' [B'' [g [vty]]]]. inv H2.
+  eapply sig_subtype_get_Some in g; eauto.
+  destruct g as [A'''[B'''[g'[s']]]].
+  exists A''', B'''. aconstructor. constructor.
+  - apply TypeV. auto. apply get_op_type_wf in g'. destruct g'.
+    auto. inv H0. auto. eapply TypeVSubtype; eauto.
   - eapply (ctx_subtype_ctype (CtxU Γ B'') (CtxU Γ B''')).
-    * apply TypeC. inv H1. assumption. assumption.
-      eapply TypeCSubtype. eauto. apply SubtypeCTy; assumption.
-    * apply WfCtxU. assumption. apply get_op_type_wf in g'. destruct g'.
-      all: inv H0; assumption.
-    * apply SubtypeCtxU. apply ctx_subtype_refl. all: assumption.
+    * apply TypeC. inv H1. auto. auto.
+      eapply TypeCSubtype. eauto. apply SubtypeCTy; auto.
+    * apply WfCtxU. auto. apply get_op_type_wf in g'. destruct g'.
+      all: inv H0; auto.
+    * apply SubtypeCtxU. apply ctx_subtype_refl. all: auto.
 Qed.
 
 
 Fixpoint shape_op Γ op v c A Σ E :
   has_ctype Γ (Op op v c) (CTy A Σ E) -> 
-  (exists Aop Bop, get_op_type Σ op = Some (Aop, Bop) /\
-    has_vtype Γ v Aop /\  has_ctype (CtxU Γ Bop) c (CTy A Σ E)).
+  exists Aop Bop,
+    get_op_type Σ op = Some (Aop, Bop) /\
+    has_vtype Γ v Aop /\  has_ctype (CtxU Γ Bop) c (CTy A Σ E).
 Proof.  
 intro orig. eapply (shape_op_full _ _ _ op v c A Σ E) in orig; auto.
 Qed.
