substitution/substitution_lemmas.v
@@ -1,10 +1,9 @@
-(* Add LoadPath "C:\Users\Ziga\Documents\Ziga_podatki\repositories\eeff-formalization\substitution". *)
-(* Add LoadPath "C:\Users\Ziga\Documents\Ziga_podatki\repositories\eeff-formalization\syntax". *)
-Add LoadPath "E:\Ziga_Podatki\faks\eeff-formalization\substitution".
-Add LoadPath "E:\Ziga_Podatki\faks\eeff-formalization\syntax".
+Add LoadPath "C:\Users\Ziga\Documents\Ziga_podatki\repositories\eeff-formalization\substitution".
+Add LoadPath "C:\Users\Ziga\Documents\Ziga_podatki\repositories\eeff-formalization\syntax".
+(* Add LoadPath "E:\Ziga_Podatki\faks\eeff-formalization\substitution". *)
+(* Add LoadPath "E:\Ziga_Podatki\faks\eeff-formalization\syntax". *)
 Require Export substitution syntax_lemmas.
-Require Import Le Compare_dec Arith.
-Require Import Omega.
+Require Import Le Arith.
 
 (* ==================== Effects on getters ==================== *)
 
