type_system/type_aux_lemmas.v
@@ -7,11 +7,7 @@ Add LoadPath "C:\Users\Ziga\Documents\Ziga_podatki\repositories\eeff-formalizati
 (* Add LoadPath "E:\Ziga_Podatki\faks\eeff-formalization\substitution". *)
 (* Add LoadPath "E:\Ziga_Podatki\faks\eeff-formalization\logic". *)
 
-Require Export syntax_lemmas substitution_lemmas subtyping_lemmas
-  logic_aux_lemmas.
-Open Scope string_scope.
-
-Ltac inv H := inversion H; clear H; subst.
+Require Export subtyping_lemmas substitution_lemmas logic_aux_lemmas.
 
 (* ==================== Typing and No/Under Var ==================== *)
 
@@ -34,7 +30,7 @@ all: assert (forall A Γ, S(ctx_len Γ) = ctx_len (CtxU Γ A)) as ext by auto.
 all: erewrite ext; eauto; erewrite ext; eauto.
 }{
 intro types. destruct types. destruct H2; simpl. auto. constructor; eauto.
-assert (S(S(ctx_len Γ)) = ctx_len(CtxU(CtxU Γ (TyFun B_op D)) A_op)) by auto.
+assert (S(S(ctx_len Γ)) = ctx_len(CtxU(CtxU Γ (TyFun Bop D)) Aop)) by auto.
 rewrite H5. eauto.
 }
 Qed.
@@ -68,7 +64,8 @@ Qed.
 
 Lemma handle_t_no_var h i Γ Z T Σ:
   h_no_var h i -> wf_t Γ Z T Σ ->
-  c_no_var (handle_t (ctx_len Γ) (tctx_len Z) h T) 
+  c_no_var 
+    (handle_t (ctx_len Γ) (tctx_len Z) h T)
     (i + tctx_len Z + ctx_len Γ).
 Proof.
 revert h Γ i. induction T; intros; simpl.
@@ -77,32 +74,32 @@ all: assert (forall A Γ, S(ctx_len Γ)=ctx_len (CtxU Γ A)) as sctx by
 all: assert (forall x, S(i+tctx_len Z+x) = i+tctx_len Z+S x) as slen by
   (intros; omega).
 + constructor.
-  all: apply wf_is_under_ctx_tctx in H0; destruct H0; simpl in *. 
-  omega. eapply v_under_var_no_var. eauto. omega.
+  all: apply wf_is_under_ctx_tctx in H0; destruct H0; simpl in *.
+  omega. eapply v_under_var_no_var; eaomega.
 + apply wf_is_under_ctx_tctx in H0. destruct H0.
-  eapply v_under_var_no_var. eauto. omega.
+  eapply v_under_var_no_var; eaomega.
 + constructor; inv H0.
-  - eapply v_under_var_no_var. eapply has_vtype_is_under_ctx. eauto. omega.
+  - eapply v_under_var_no_var. eapply has_vtype_is_under_ctx. all: eaomega.
   - rewrite slen, slen, (sctx A), (sctx B). eauto.
 + inv H0. constructor. 2: constructor.
-  - eapply v_under_var_no_var. eapply has_vtype_is_under_ctx. eauto. omega.
+  - eapply v_under_var_no_var. eapply has_vtype_is_under_ctx. all: eaomega.
   - rewrite slen, (sctx A). auto. 
   - rewrite slen, (sctx B). auto. 
-+ inv H0. constructor. 2: constructor.
-  - eapply v_under_var_no_var. eapply has_vtype_is_under_ctx. eauto. omega.
-  - auto. 
++ inv H0. constructor. 2: aconstructor.
+  - eapply v_under_var_no_var. eapply has_vtype_is_under_ctx. all: eaomega.
   - rewrite slen, slen, (sctx A), (sctx (TyList A)). auto. 
 + destruct (get_case h o) eqn:finds; inv H0.
-  - apply c_no_var_subs. apply c_no_var_subs. all: omega || simpl.
+  - unfold c_subs2_out. unfold c_subs_out. 
+    apply c_no_var_subs. apply c_no_var_subs. all: omega || simpl.
     * eapply get_case_no_var in finds; eauto.
-      assert (S(S(i+tctx_len Z+ctx_len Γ))=(ctx_len Γ+tctx_len Z)+(2+i)) by omega.
-      rewrite H0. apply c_no_var_shift. eauto. omega.
+      assert (S(S(i+tctx_len Z+ctx_len Γ))=(ctx_len Γ+tctx_len Z)+(2+i)).
+      omega. rewrite H0. apply c_no_var_shift; eaomega.
     * apply v_no_var_shift. eapply v_under_var_no_var.
-      eapply has_vtype_is_under_ctx. eauto. all: omega.
-    * rewrite slen, (sctx B_op). eauto.
+      eapply has_vtype_is_under_ctx. all: eaomega.
+    * rewrite slen, (sctx Bop). eauto.
   - simpl. constructor.
-    * eapply v_under_var_no_var. eapply has_vtype_is_under_ctx. eauto. omega.
-    * rewrite slen, (sctx B_op). eauto.
+    * eapply v_under_var_no_var. eapply has_vtype_is_under_ctx. all: eaomega.
+    * rewrite slen, (sctx Bop). eauto.
 Qed.
 
 Lemma handle_t_under_var h i Γ Z T Σ:
@@ -117,9 +114,9 @@ all: assert (forall x, S(i+tctx_len Z+x) = i+tctx_len Z+S x) as slen by
   (intros; omega).
 + constructor.
   all: apply wf_is_under_ctx_tctx in H0; destruct H0; simpl in *. 
-  omega. eapply v_under_var_weaken. eauto. omega.
+  omega. eapply v_under_var_weaken; eaomega.
 + apply wf_is_under_ctx_tctx in H0. destruct H0.
-  eapply v_under_var_weaken. eauto. omega.
+  eapply v_under_var_weaken; eaomega.
 + constructor; inv H0.
   - eapply v_under_var_weaken. eapply has_vtype_is_under_ctx. eauto. omega.
   - rewrite slen, slen, (sctx A), (sctx B). eauto.
@@ -127,21 +124,20 @@ all: assert (forall x, S(i+tctx_len Z+x) = i+tctx_len Z+S x) as slen by
   - eapply v_under_var_weaken. eapply has_vtype_is_under_ctx. eauto. omega.
   - rewrite slen, (sctx A). auto. 
   - rewrite slen, (sctx B). auto. 
-+ inv H0. constructor. 2: constructor.
++ inv H0. constructor. 2: aconstructor.
   - eapply v_under_var_weaken. eapply has_vtype_is_under_ctx. eauto. omega.
-  - auto. 
   - rewrite slen, slen, (sctx A), (sctx (TyList A)). auto. 
 + destruct (get_case h o) eqn:finds; inv H0.
   - apply c_under_var_subs. apply c_under_var_subs. all: omega || simpl.
     * eapply get_case_under_var in finds; eauto.
-      assert (S(S(i+tctx_len Z+ctx_len Γ))=(ctx_len Γ+tctx_len Z)+(2+i)) by omega.
-      rewrite H0. apply c_under_var_shift. eauto. omega.
+      assert (S(S(i+tctx_len Z+ctx_len Γ))=(ctx_len Γ+tctx_len Z)+(2+i)).
+      omega. rewrite H0. apply c_under_var_shift; eaomega.
     * apply v_under_var_shift. eapply v_under_var_weaken.
-      eapply has_vtype_is_under_ctx. eauto. all: omega.
-    * rewrite slen, (sctx B_op). eauto.
+      eapply has_vtype_is_under_ctx. all: eaomega.
+    * rewrite slen, (sctx Bop). eauto.
   - simpl. constructor.
     * eapply v_under_var_weaken. eapply has_vtype_is_under_ctx. eauto. omega.
-    * rewrite slen, (sctx B_op). eauto.
+    * rewrite slen, (sctx Bop). eauto.
 Qed.
 
 (* ==================== Handling and Shifts. ==================== *)
@@ -149,7 +145,8 @@ Qed.
 Lemma handle_t_shift Γ' Γ Z h T Σ D i:
   wf_t Γ Z T Σ -> has_htype Γ' h Σ D -> 
     handle_t (ctx_len Γ) (tctx_len Z) (h_shift h 1 i) T
-  = c_shift (handle_t (ctx_len Γ) (tctx_len Z) h T) 
+  = c_shift 
+      (handle_t (ctx_len Γ) (tctx_len Z) h T) 
       1 (i + tctx_len Z + ctx_len Γ).
 Proof.
 revert Γ h i. induction T; intros Γ h i wf types; simpl; inv wf.
@@ -158,29 +155,29 @@ all: assert (forall A Γ, S(ctx_len Γ)=ctx_len (CtxU Γ A)) as sctx by
 all: assert (forall x, S(i+tctx_len Z+x) = i+tctx_len Z+S x) as slen by
   (intros; omega).
 + simpl. apply tctx_len_get_Some in H5 as zlen. 
-  destruct ((i + tctx_len Z + ctx_len Γ) <=? ctx_len Γ + v) eqn:cmp.
+  destruct ((i + tctx_len Z + ctx_len Γ) <=? ctx_len Γ + n) eqn:cmp.
   { apply leb_complete in cmp. omega. }
   f_equal. rewrite v_shift_too_high. auto.
   eapply has_vtype_is_under_ctx in H3.  
-  eapply v_under_var_weaken. eauto. omega.
+  eapply v_under_var_weaken; eaomega.
 + f_equal. rewrite v_shift_too_high. auto.
   apply has_vtype_is_under_ctx in H2.
-  eapply v_under_var_weaken. eauto. omega.
+  eapply v_under_var_weaken; eaomega.
 + f_equal.
   - rewrite v_shift_too_high. auto.
     apply has_vtype_is_under_ctx in H3.
-    eapply v_under_var_weaken. eauto. omega.
+    eapply v_under_var_weaken; eaomega.
   - rewrite slen, slen, (sctx A), (sctx B). auto.
 + f_equal.
   - rewrite v_shift_too_high. auto.
     apply has_vtype_is_under_ctx in H4.
-    eapply v_under_var_weaken. eauto. omega.
+    eapply v_under_var_weaken; eaomega.
   - rewrite slen, (sctx A). auto.
   - rewrite slen, (sctx B). auto.
   + f_equal.
   - rewrite v_shift_too_high. auto.
     apply has_vtype_is_under_ctx in H4.
-    eapply v_under_var_weaken. eauto. omega.
+    eapply v_under_var_weaken; eaomega.
   - auto.
   - rewrite slen, slen, (sctx A), (sctx (TyList A)). auto.
 + eapply h_has_case in H4 as find. 2: exact types.
@@ -194,15 +191,16 @@ all: assert (forall x, S(i+tctx_len Z+x) = i+tctx_len Z+S x) as slen by
     rewrite c_shift_comm. f_equal. omega. omega.
     rewrite (v_shift_too_high (v_shift v 1 0)). auto.
     apply v_under_var_shift. apply has_vtype_is_under_ctx in H6.
-    eapply v_under_var_weaken. eauto. omega. omega. 
-  * f_equal. rewrite slen, (sctx B_op). auto. 
+    eapply v_under_var_weaken. all: eaomega. 
+  * f_equal. rewrite slen, (sctx Bop). auto. 
 Qed.
 
 
 Lemma handle_t_negshift Γ' Γ Z h T Σ D i:
   h_no_var h i -> wf_t Γ Z T Σ -> has_htype Γ' h Σ D -> 
     handle_t (ctx_len Γ) (tctx_len Z) (h_negshift h 1 i) T
-  = c_negshift (handle_t (ctx_len Γ) (tctx_len Z) h T) 
+  = c_negshift 
+      (handle_t (ctx_len Γ) (tctx_len Z) h T) 
       1 (i + tctx_len Z + ctx_len Γ).
 Proof.
 revert Γ h i. induction T; intros Γ h i novar wf types; simpl; inv wf.
@@ -211,29 +209,29 @@ all: assert (forall A Γ, S(ctx_len Γ)=ctx_len (CtxU Γ A)) as sctx by
 all: assert (forall x, S(i+tctx_len Z+x) = i+tctx_len Z+S x) as slen by
   (intros; omega).
 + apply tctx_len_get_Some in H5 as zlen. simpl.
-  destruct ((i + tctx_len Z + ctx_len Γ) <=? ctx_len Γ + v) eqn:cmp.
+  destruct ((i + tctx_len Z + ctx_len Γ) <=? ctx_len Γ + n) eqn:cmp.
   - apply leb_complete in cmp. omega.
   - f_equal. rewrite v_negshift_too_high. auto.
     eapply has_vtype_is_under_ctx in H3.  
-    eapply v_under_var_weaken. eauto. omega.
+    eapply v_under_var_weaken; eaomega.
 + f_equal. rewrite v_negshift_too_high. auto.
   apply has_vtype_is_under_ctx in H2.
-  eapply v_under_var_weaken. eauto. omega.
+  eapply v_under_var_weaken; eaomega.
 + f_equal.
   - rewrite v_negshift_too_high. auto.
     apply has_vtype_is_under_ctx in H3.
-    eapply v_under_var_weaken. eauto. omega.
+    eapply v_under_var_weaken; eaomega.
   - rewrite slen, slen, (sctx A), (sctx B). auto.
 + f_equal.
   - rewrite v_negshift_too_high. auto.
     apply has_vtype_is_under_ctx in H4.
-    eapply v_under_var_weaken. eauto. omega.
+    eapply v_under_var_weaken; eaomega.
   - rewrite slen, (sctx A). auto.
   - rewrite slen, (sctx B). auto.
   + f_equal.
   - rewrite v_negshift_too_high. auto.
     apply has_vtype_is_under_ctx in H4.
-    eapply v_under_var_weaken. eauto. omega.
+    eapply v_under_var_weaken; eaomega.
   - auto.
   - rewrite slen, slen, (sctx A), (sctx (TyList A)). auto.
 + eapply h_has_case in H4 as find. 2: exact types.
@@ -248,23 +246,24 @@ all: assert (forall x, S(i+tctx_len Z+x) = i+tctx_len Z+S x) as slen by
     rewrite cext, c_shift_negshift_comm. f_equal. auto. omega.
     rewrite v_negshift_too_high. auto.
     - apply v_under_var_shift. apply has_vtype_is_under_ctx in H6.
-      eapply v_under_var_weaken. eauto. omega. omega. 
+      eapply v_under_var_weaken. all: eaomega. 
     - simpl. rewrite cext. apply c_no_var_shift. eauto. omega.
     - apply v_no_var_shift. apply has_vtype_is_under_ctx in H6.
-      eapply v_under_var_no_var. eauto. omega. omega. 
-  * f_equal. rewrite slen, (sctx B_op). auto.
+      eapply v_under_var_no_var. all: eaomega. 
+  * f_equal. rewrite slen, (sctx Bop). auto.
   * apply c_no_var_subs. simpl. rewrite cext.
-    apply c_no_var_shift. eauto. omega. 
+    apply c_no_var_shift; eaomega. 
     apply v_no_var_shift. apply has_vtype_is_under_ctx in H6.
-    eapply v_under_var_no_var. eauto. all: omega.
-  * simpl. rewrite slen, (sctx B_op). eapply handle_t_no_var; eauto.
+    eapply v_under_var_no_var. all: eaomega.
+  * simpl. rewrite slen, (sctx Bop). eapply handle_t_no_var; eauto.
 Qed.
 
 
 Lemma handle_t_sub Γ' Γ Z h T Σ D i v_s:
   wf_t Γ Z T Σ -> has_htype Γ' h Σ D ->
     handle_t (ctx_len Γ) (tctx_len Z) (h_sub h (i, v_s)) T
-  = c_sub (handle_t (ctx_len Γ) (tctx_len Z) h T)
+  = c_sub 
+      (handle_t (ctx_len Γ) (tctx_len Z) h T)
       (i+tctx_len Z+ctx_len Γ, v_shift v_s (tctx_len Z+ctx_len Γ) 0).
 Proof.
 revert Γ h i. induction T; intros Γ h i wf types; simpl; inv wf.
@@ -273,25 +272,25 @@ all: assert (forall A Γ, S(ctx_len Γ)=ctx_len (CtxU Γ A)) as sctx by
 all: assert (forall x, S(i+tctx_len Z+x) = i+tctx_len Z+S x) as slen by
   (intros; omega).
 + apply tctx_len_get_Some in H5 as zlen. simpl.
-  destruct (ctx_len Γ + v =? i + tctx_len Z + ctx_len Γ) eqn:cmp.
+  destruct (ctx_len Γ + n =? i + tctx_len Z + ctx_len Γ) eqn:cmp.
   - apply Nat.eqb_eq in cmp. omega.
   - f_equal. rewrite v_sub_too_high. auto.
     eapply has_vtype_is_under_ctx in H3. 
-    eapply v_under_var_weaken. eauto. omega.
+    eapply v_under_var_weaken; eaomega.
 + f_equal. rewrite v_sub_too_high. auto.
   apply has_vtype_is_under_ctx in H2.
-  eapply v_under_var_weaken. eauto. omega.
+  eapply v_under_var_weaken; eaomega.
 + f_equal.
   - rewrite v_sub_too_high. auto.
     apply has_vtype_is_under_ctx in H3.
-    eapply v_under_var_weaken. eauto. omega.
+    eapply v_under_var_weaken; eaomega.
   - assert (tctx_len Z + ctx_len Γ + 2 = tctx_len Z + S(S(ctx_len Γ))) as same.
     omega. rewrite v_shift_shift, same.
     rewrite slen, slen, (sctx A), (sctx B). auto.
 + f_equal.
   - rewrite v_sub_too_high. auto.
     apply has_vtype_is_under_ctx in H4.
-    eapply v_under_var_weaken. eauto. omega.
+    eapply v_under_var_weaken; eaomega.
   - assert (tctx_len Z + ctx_len Γ + 1 = tctx_len Z + S(ctx_len Γ)) as same.
     omega. rewrite v_shift_shift, same, slen, (sctx A). auto.
   - assert (tctx_len Z + ctx_len Γ + 1 = tctx_len Z + S(ctx_len Γ)) as same.
@@ -299,7 +298,7 @@ all: assert (forall x, S(i+tctx_len Z+x) = i+tctx_len Z+S x) as slen by
 + f_equal.
   - rewrite v_sub_too_high. auto.
     apply has_vtype_is_under_ctx in H4.
-    eapply v_under_var_weaken. eauto. omega.
+    eapply v_under_var_weaken; eaomega.
   - auto.
   - assert (tctx_len Z + ctx_len Γ + 2 = tctx_len Z + S(S(ctx_len Γ))) as same.
     omega. rewrite v_shift_shift, same.
@@ -316,9 +315,9 @@ all: assert (forall x, S(i+tctx_len Z+x) = i+tctx_len Z+S x) as slen by
     rewrite (v_shift_comm _ _ 0). f_equal. all: try omega.
     rewrite v_sub_too_high. auto.
     apply v_under_var_shift. apply has_vtype_is_under_ctx in H6.
-    eapply v_under_var_weaken. eauto. omega. omega. 
+    eapply v_under_var_weaken. all: eaomega. 
   * assert (tctx_len Z + ctx_len Γ + 1 = tctx_len Z + S(ctx_len Γ)) as same.
-    omega. f_equal. rewrite v_shift_shift, same, slen, (sctx B_op). auto.
+    omega. f_equal. rewrite v_shift_shift, same, slen, (sctx Bop). auto.
 Qed.
 
 
@@ -327,42 +326,42 @@ Qed.
 Fixpoint v_insert_typesafe 
   Γ v A (orig : has_vtype Γ v A) A_ins i {struct orig} :
   wf_vtype A_ins ->
-  has_vtype (ctx_insert Γ A_ins i) (v_shift v 1 i) A
+  has_vtype (ctx_insert Γ i A_ins) (v_shift v 1 i) A
 
 with c_insert_typesafe 
   Γ c C (orig : has_ctype Γ c C) A_ins i {struct orig} :
   wf_vtype A_ins ->
-  has_ctype (ctx_insert Γ A_ins i) (c_shift c 1 i) C
+  has_ctype (ctx_insert Γ i A_ins) (c_shift c 1 i) C
 
 with h_insert_typesafe 
   Γ h Σ D (orig : has_htype Γ h Σ D) A_ins i {struct orig} :
   wf_vtype A_ins ->
-  has_htype (ctx_insert Γ A_ins i) (h_shift h 1 i) Σ D
+  has_htype (ctx_insert Γ i A_ins) (h_shift h 1 i) Σ D
 
 with respects_insert_typesafe
   Γ h Σ D E (orig: respects Γ h Σ D E) A_ins i {struct orig} :
   has_htype Γ h Σ D -> wf_vtype A_ins ->
-  respects (ctx_insert Γ A_ins i) (h_shift h 1 i) Σ D E
+  respects (ctx_insert Γ i A_ins) (h_shift h 1 i) Σ D E
 
 with veq_insert_typesafe
   Γ A v1 v2 (orig: veq A Γ v1 v2) A_ins i {struct orig} :
   wf_vtype A_ins ->
-  veq A (ctx_insert Γ A_ins i) (v_shift v1 1 i) (v_shift v2 1 i)
+  veq A (ctx_insert Γ i A_ins) (v_shift v1 1 i) (v_shift v2 1 i)
 
 with ceq_insert_typesafe
   Γ C c1 c2 (orig: ceq C Γ c1 c2) A_ins i {struct orig} :
   wf_vtype A_ins ->
-  ceq C (ctx_insert Γ A_ins i) (c_shift c1 1 i) (c_shift c2 1 i)
+  ceq C (ctx_insert Γ i A_ins) (c_shift c1 1 i) (c_shift c2 1 i)
   
 with heq_insert_typesafe
   Γ Σ D h1 h2 (orig: heq Σ D Γ h1 h2) A_ins i {struct orig} :
   wf_vtype A_ins ->
-  heq Σ D (ctx_insert Γ A_ins i) (h_shift h1 1 i) (h_shift h2 1 i)
+  heq Σ D (ctx_insert Γ i A_ins) (h_shift h1 1 i) (h_shift h2 1 i)
 
 with wf_inst_insert_typesafe
   Γ Γ' I (orig: wf_inst Γ I Γ') A_ins i {struct orig} : 
   wf_vtype A_ins ->
-  wf_inst (ctx_insert Γ A_ins i) (inst_shift I 1 i) Γ'.
+  wf_inst (ctx_insert Γ i A_ins) (inst_shift I 1 i) Γ'.
 
 Proof.
 all: rename v_insert_typesafe into V; rename c_insert_typesafe into CI.
@@ -371,89 +370,115 @@ all: rename veq_insert_typesafe into VE; rename ceq_insert_typesafe into CE.
 all: rename heq_insert_typesafe into HE; rename wf_inst_insert_typesafe into WF.
 {
 intros wfins. apply TypeV.
-{ apply wf_ctx_insert. inv orig. assumption. assumption. }
-{ inv orig. assumption. }
+{ apply wf_ctx_insert. inv orig. all: auto. }
+{ inv orig. auto. }
 inv orig. destruct H1.
-+ clear V CI HC R VE CE HE WF. simpl. apply TypeUnit.
-+ clear V CI HC R VE CE HE WF. simpl. apply TypeInt.
++ clear V CI HC R VE CE HE WF.
+  simpl. apply TypeUnit.
++ clear V CI HC R VE CE HE WF.
+  simpl. apply TypeInt.
 + clear V CI HC R VE CE HE WF.
   simpl. destruct (i <=? n) eqn:cmp.
   - apply TypeVar. rewrite <-get_ctx_insert_changed.
-    assumption. apply leb_complete in cmp. omega.
+    auto. apply leb_complete in cmp. omega.
   - apply TypeVar. rewrite <-get_ctx_insert_unchanged.
-    assumption. apply leb_iff_conv in cmp. assumption.
+    auto. apply leb_iff_conv in cmp. auto.
 + specialize (V _ _ _ H1) as IHv1. specialize (V _ _ _ H2) as IHv2.
-  clear V CI HC R VE CE HE WF. simpl. apply TypePair; auto.
+  clear V CI HC R VE CE HE WF.
+  simpl. apply TypePair; auto.
 + specialize (V _ _ _ H1) as IHv.
-  clear V CI HC R VE CE HE WF. simpl. apply TypeInl. auto.
+  clear V CI HC R VE CE HE WF.
+  simpl. apply TypeInl. auto.
 + specialize (V _ _ _ H1) as IHv.
-  clear V CI HC R VE CE HE WF. simpl. apply TypeInr. auto.
-+ clear V CI HC R VE CE HE WF. simpl. apply TypeListNil.
-+ specialize (V _ _ _ H1) as IHv1. specialize (V _ _ _ H2) as IHv2.
-  clear V CI HC R VE CE HE WF. simpl. apply TypeListCons; auto.
+  clear V CI HC R VE CE HE WF.
+  simpl. apply TypeInr. auto.
++ clear V CI HC R VE CE HE WF.
+  simpl. apply TypeListNil.
++ specialize (V _ _ _ H1) as IHv1.
+  specialize (V _ _ _ H2) as IHv2.
+  clear V CI HC R VE CE HE WF.
+  simpl. apply TypeListCons; auto.
 + specialize (CI _ _ _ H1) as IHc.
   clear V CI HC R VE CE HE WF.
   simpl. apply TypeFun. rewrite ctx_insert_extend. auto.
-+ specialize (HC _ _ _ _ H2) as IHh. specialize (CI _ _ _ H1) as IHc.
++ specialize (HC _ _ _ _ H2) as IHh.
+  specialize (CI _ _ _ H1) as IHc.
   specialize (R _ _ _ _ _ H3) as IHres.
   clear V CI HC R VE CE HE WF.
   simpl. apply TypeHandler. rewrite ctx_insert_extend. all: auto. 
 + specialize (V _ _ _ H1) as IHv.
-  clear V CI HC R VE CE HE WF. eapply TypeVSubtype; auto.
+  clear V CI HC R VE CE HE WF.
+  eapply TypeVSubtype; auto.
 }{
 intros wfins. apply TypeC.
 { apply wf_ctx_insert. inv orig. all: assumption. }
 { inv orig. assumption. }
 inv orig. destruct H1.
 + specialize (V _ _ _ H1) as IHv.
-  clear V CI HC R VE CE HE WF. simpl. apply TypeRet. auto.
+  clear V CI HC R VE CE HE WF.
+  simpl. apply TypeRet. auto.
 + specialize (V _ _ _ H1) as IHv.
-  clear V CI HC R VE CE HE WF. simpl. apply TypeAbsurd. auto.
-+ specialize (V _ _ _ H1) as IHv. specialize (CI _ _ _ H2) as IHc.
-  clear V CI HC R VE CE HE WF. simpl. eapply TypeΠMatch. auto.
+  clear V CI HC R VE CE HE WF.
+  simpl. apply TypeAbsurd. auto.
++ specialize (V _ _ _ H1) as IHv.
+  specialize (CI _ _ _ H2) as IHc.
+  clear V CI HC R VE CE HE WF.
+  simpl. eapply TypeΠMatch. auto.
   rewrite ctx_insert_extend. rewrite ctx_insert_extend. auto.
-+ specialize (V _ _ _ H1) as IHv. specialize (CI _ _ _ H2) as IHc1.
++ specialize (V _ _ _ H1) as IHv.
+  specialize (CI _ _ _ H2) as IHc1.
   specialize (CI _ _ _ H3) as IHc2.
   clear V CI HC R VE CE HE WF.
-  simpl. eapply TypeΣMatch. auto. all: rewrite ctx_insert_extend; auto.
+  simpl. eapply TypeΣMatch. auto.
+  all: rewrite ctx_insert_extend; auto.
 + specialize (V _ _ _ H1) as IHv. 
   specialize (CI _ _ _ H2) as IHc1.
   specialize (CI _ _ _ H3) as IHc2.
-  clear V CI HC R VE CE HE WF. simpl. eapply TypeListMatch; auto.
-  rewrite ctx_insert_extend. rewrite ctx_insert_extend. auto.
-+ specialize (CI _ _ _ H1) as IHc1. specialize (CI _ _ _ H2) as IHc2.
   clear V CI HC R VE CE HE WF.
-  simpl. eapply TypeDoBind. auto. rewrite ctx_insert_extend. auto.
-+ specialize (V _ _ _ H1) as IHv. specialize (V _ _ _ H2) as IHv0.
-  clear V CI HC R VE CE HE WF. simpl. eapply TypeApp; auto.
-+ specialize (V _ _ _ H1) as IHv. specialize (CI _ _ _ H2) as IHc.
-  clear V CI HC R VE CE HE WF. simpl. eapply TypeHandle; auto.
+  simpl. eapply TypeListMatch; auto.
+  rewrite ctx_insert_extend. rewrite ctx_insert_extend. auto.
 + specialize (CI _ _ _ H1) as IHc1.
   specialize (CI _ _ _ H2) as IHc2.
-  clear V CI HC R VE CE HE WF. simpl. eapply TypeLetRec.
+  clear V CI HC R VE CE HE WF.
+  simpl. eapply TypeDoBind. auto. rewrite ctx_insert_extend. auto.
++ specialize (V _ _ _ H1) as IHv.
+  specialize (V _ _ _ H2) as IHv0.
+  clear V CI HC R VE CE HE WF.
+  simpl. eapply TypeApp; auto.
++ specialize (V _ _ _ H1) as IHv.
+  specialize (CI _ _ _ H2) as IHc.
+  clear V CI HC R VE CE HE WF.
+  simpl. eapply TypeHandle; auto.
++ specialize (CI _ _ _ H1) as IHc1.
+  specialize (CI _ _ _ H2) as IHc2.
+  clear V CI HC R VE CE HE WF.
+  simpl. eapply TypeLetRec.
   - do 2 rewrite ctx_insert_extend. auto.
   - rewrite ctx_insert_extend. auto.
-+ specialize (V _ _ _ H2) as IHv. specialize (CI _ _ _ H3) as IHc.
++ specialize (V _ _ _ H2) as IHv.
+  specialize (CI _ _ _ H3) as IHc.
   clear V CI HC R VE CE HE WF.
   simpl. eapply TypeOp. 3: rewrite ctx_insert_extend. all: eauto.
 + specialize (CI _ _ _ H1) as IHc.
-  clear V CI HC R VE CE HE WF. eapply TypeCSubtype; auto.
+  clear V CI HC R VE CE HE WF.
+  eapply TypeCSubtype; auto.
 }{
 intros wfins. apply TypeH.
 { apply wf_ctx_insert. inv orig. all: assumption. }
 all: try (inv orig; assumption).
 inv orig. destruct H2.
 + simpl. clear V CI HC R VE CE HE WF. apply TypeCasesØ.
-+ specialize (HC _ _ _ _ H3) as IHh. specialize (CI _ _ _ H4) as IHc.
++ specialize (HC _ _ _ _ H3) as IHh.
+  specialize (CI _ _ _ H4) as IHc.
   clear V CI HC R VE CE HE WF.
   simpl. apply TypeCasesU. 2: auto.
   - apply shift_get_case_None. assumption.
   - do 2 rewrite ctx_insert_extend. auto.
 }{
 intros types wfins. apply Respects.
-{ clear V CI HC R VE CE HE WF. apply wf_ctx_insert. inv orig. all: assumption. }
-all: try (inv orig; assumption).
-inv orig. destruct H3.
+{ clear V CI HC R VE CE HE WF. apply wf_ctx_insert. inv orig. all: auto. }
+all: inv orig; auto.
+destruct H3.
 + clear V CI HC R VE CE HE WF. apply RespectEqsØ.
 + specialize (R _ _ _ _ _ H3) as IHres. specialize (CE _ _ _ _ H4) as IHeq.
   clear V CI HC R VE CE HE WF. apply RespectEqsU. auto.
@@ -462,139 +487,176 @@ inv orig. destruct H3.
   rewrite <-len_tctx_to_ctx.
   assert (ctx_len Γ+(tctx_len Z+i) = i+tctx_len Z+ctx_len Γ) by omega.
   rewrite H5. apply IHeq.
-  all: inv H2. all: try eassumption.
+  all: inv H2. all: eauto.
 }{
 intros wfins. apply Veq.
 { inv orig; eauto. }
 { inv orig; eauto. }
 inv orig. destruct H1.
 + specialize (VE _ _ _ _ H1) as IH.
-  clear V CI HC R VE CE HE WF. apply VeqSym. auto.
+  clear V CI HC R VE CE HE WF.
+  apply VeqSym. auto.
 + specialize (VE _ _ _ _ H1) as IH1.
   specialize (VE _ _ _ _ H2) as IH2.
-  clear V CI HC R VE CE HE WF. eapply VeqTrans; eauto.
-+ clear V CI HC R VE CE HE WF. subst. simpl. rename i0 into j.
+  clear V CI HC R VE CE HE WF.
+  eapply VeqTrans; eauto.
++ clear V CI HC R VE CE HE WF.
+  subst. simpl. rename i0 into j.
   destruct (i <=? j) eqn:cmp; eapply VeqVar; eauto.
   - erewrite <-get_ctx_insert_changed. auto. apply leb_complete in cmp. auto.
-  - erewrite <-get_ctx_insert_unchanged. assumption. 
-    apply leb_complete_conv in cmp. assumption.
-+ clear V CI HC R VE CE HE WF. simpl. apply VeqUnit.
-+ clear V CI HC R VE CE HE WF. simpl. apply VeqInt.
+  - erewrite <-get_ctx_insert_unchanged. auto. 
+    apply leb_complete_conv in cmp. auto.
++ clear V CI HC R VE CE HE WF.
+  simpl. apply VeqUnit.
++ clear V CI HC R VE CE HE WF.
+  simpl. apply VeqInt.
 + specialize (VE _ _ _ _ H1) as IH1.
   specialize (VE _ _ _ _ H2) as IH2.
-  clear V CI HC R VE CE HE WF. simpl. apply VeqPair; auto.
+  clear V CI HC R VE CE HE WF.
+  simpl. apply VeqPair; auto.
 + specialize (VE _ _ _ _ H1) as IH.
-  clear V CI HC R VE CE HE WF. simpl. eapply VeqInl; eauto.
+  clear V CI HC R VE CE HE WF.
+  simpl. eapply VeqInl; eauto.
 + specialize (VE _ _ _ _ H1) as IH.
-  clear V CI HC R VE CE HE WF. simpl. eapply VeqInr; eauto.
-+ clear V CI HC R VE CE HE WF. simpl. eapply VeqListNil.
+  clear V CI HC R VE CE HE WF.
+  simpl. eapply VeqInr; eauto.
++ clear V CI HC R VE CE HE WF.
+simpl. eapply VeqListNil.
 + specialize (VE _ _ _ _ H1) as IH1.
   specialize (VE _ _ _ _ H2) as IH2.
-  clear V CI HC R VE CE HE WF. simpl. eapply VeqListCons; eauto.
+  clear V CI HC R VE CE HE WF.
+  simpl. eapply VeqListCons; eauto.
 + specialize (CE _ _ _ _ H1) as IH.
-  clear V CI HC R VE CE HE WF. simpl. eapply VeqFun.
+  clear V CI HC R VE CE HE WF.
+  simpl. eapply VeqFun.
   rewrite ctx_insert_extend. auto.
 + specialize (CE _ _ _ _ H1) as IHc.
   specialize (HE _ _ _ _ _ H2) as IHh.
-  clear V CI HC R VE CE HE WF. simpl. eapply VeqHandler; eauto.
+  clear V CI HC R VE CE HE WF.
+  simpl. eapply VeqHandler; eauto.
   rewrite ctx_insert_extend. auto.
-+ clear V CI HC R VE CE HE WF. simpl. apply ηUnit.
-+ clear V CI HC R VE CE HE WF. simpl. rewrite <-v_shift_comm. apply ηFun. omega.
++ clear V CI HC R VE CE HE WF.
+  simpl. apply ηUnit.
++ clear V CI HC R VE CE HE WF.
+  simpl. rewrite <-v_shift_comm. apply ηFun. omega.
 }{
 intros wfins. apply Ceq.
 { inv orig; eauto. }
 { inv orig; eauto. }
 inv orig. destruct H1.
 + specialize (CE _ _ _ _ H1) as IH.
-  clear V CI HC R VE CE HE WF. apply CeqSym. auto.
+  clear V CI HC R VE CE HE WF.
+  apply CeqSym. auto.
 + specialize (CE _ _ _ _ H1) as IH1.
   specialize (CE _ _ _ _ H2) as IH2.
-  clear V CI HC R VE CE HE WF. eapply CeqTrans; eauto.
+  clear V CI HC R VE CE HE WF.
+  eapply CeqTrans; eauto.
 + specialize (VE _ _ _ _ H1) as IH.
-  clear V CI HC R VE CE HE WF. simpl. apply CeqRet. auto.
+  clear V CI HC R VE CE HE WF.
+  simpl. apply CeqRet. auto.
 + specialize (VE _ _ _ _ H1) as IH.
-  clear V CI HC R VE CE HE WF. simpl. apply CeqAbsurd. auto.
+  clear V CI HC R VE CE HE WF.
+  simpl. apply CeqAbsurd. auto.
 + specialize (VE _ _ _ _ H1) as IHv.
   specialize (CE _ _ _ _ H2) as IHc.
-  clear V CI HC R VE CE HE WF. simpl. eapply CeqΠMatch. auto.
+  clear V CI HC R VE CE HE WF.
+  simpl. eapply CeqΠMatch. auto.
   do 2 rewrite ctx_insert_extend. auto.
 + specialize (VE _ _ _ _ H1) as IHv.
   specialize (CE _ _ _ _ H2) as IHc1.
   specialize (CE _ _ _ _ H3) as IHc2.
-  clear V CI HC R VE CE HE WF. simpl. eapply CeqΣMatch. auto.
+  clear V CI HC R VE CE HE WF.
+  simpl. eapply CeqΣMatch. auto.
   all: rewrite ctx_insert_extend; auto.
 + specialize (VE _ _ _ _ H1) as IHv.
   specialize (CE _ _ _ _ H2) as IHc1.
   specialize (CE _ _ _ _ H3) as IHc2.
-  clear V CI HC R VE CE HE WF. simpl. eapply CeqListMatch; eauto.
+  clear V CI HC R VE CE HE WF.
+  simpl. eapply CeqListMatch; eauto.
   do 2 rewrite ctx_insert_extend. auto.
 + specialize (CE _ _ _ _ H1) as IHc1.
   specialize (CE _ _ _ _ H2) as IHc2.
-  clear V CI HC R VE CE HE WF. simpl. eapply CeqDoBind. eauto.
+  clear V CI HC R VE CE HE WF.
+  simpl. eapply CeqDoBind. eauto.
   rewrite ctx_insert_extend; auto.
 + specialize (VE _ _ _ _ H1) as IHv1.
   specialize (VE _ _ _ _ H2) as IHv2.
-  clear V CI HC R VE CE HE WF. simpl. eapply CeqApp; eauto.
+  clear V CI HC R VE CE HE WF.
+  simpl. eapply CeqApp; eauto.
 + specialize (VE _ _ _ _ H1) as IHv.
   specialize (CE _ _ _ _ H2) as IHc.
-  clear V CI HC R VE CE HE WF. simpl. eapply CeqHandle; eauto.
+  clear V CI HC R VE CE HE WF.
+  simpl. eapply CeqHandle; eauto.
 + specialize (CE _ _ _ _ H1) as IHc1.
   specialize (CE _ _ _ _ H2) as IHc2.
-  clear V CI HC R VE CE HE WF. simpl. eapply CeqLetRec.
+  clear V CI HC R VE CE HE WF.
+  simpl. eapply CeqLetRec.
   do 2 rewrite ctx_insert_extend; auto.
   rewrite ctx_insert_extend; auto.
 + specialize (VE _ _ _ _ H2) as IHv.
   specialize (CE _ _ _ _ H3) as IHc.
-  clear V CI HC R VE CE HE WF. simpl. eapply CeqOp; eauto.
+  clear V CI HC R VE CE HE WF.
+  simpl. eapply CeqOp; eauto.
   rewrite ctx_insert_extend; auto.
 + specialize (WF _ _ _ H2) as IHwf.
-  clear V CI HC R VE CE HE WF. eapply OOTB; eauto.
+  clear V CI HC R VE CE HE WF.
+  eapply OOTB; eauto.
   rewrite <-c_shift_inst. rewrite H3. simpl. auto.
   rewrite <-c_shift_inst. rewrite H4. simpl. auto.
-+ clear V CI HC R VE CE HE WF. specialize βΠMatch as rule.
++ clear V CI HC R VE CE HE WF.
+  specialize βΠMatch as rule.
   unfold c_subs2_out in *. unfold c_subs_out in *. simpl.
   rewrite c_shift_subs, c_shift_subs, <-v_shift_comm.
   apply rule. all: omega.
-+ clear V CI HC R VE CE HE WF. specialize βΣMatch_Inl as rule.
++ clear V CI HC R VE CE HE WF.
+  specialize βΣMatch_Inl as rule.
   unfold c_subs_out in *. simpl. rewrite c_shift_subs.
   apply rule. all: omega.
-+ clear V CI HC R VE CE HE WF. specialize βΣMatch_Inr as rule.
++ clear V CI HC R VE CE HE WF.
+  specialize βΣMatch_Inr as rule.
   unfold c_subs_out in *. simpl. rewrite c_shift_subs.
   apply rule. all: omega.
-+ clear V CI HC R VE CE HE WF. specialize βListMatch_Nil as rule.
++ clear V CI HC R VE CE HE WF.
+  specialize βListMatch_Nil as rule.
   unfold c_subs_out in *. simpl. 
   apply rule. all: omega.
-+ clear V CI HC R VE CE HE WF. specialize βListMatch_Cons as rule.
++ clear V CI HC R VE CE HE WF.
+  specialize βListMatch_Cons as rule.
   unfold c_subs2_out in *. unfold c_subs_out in *. simpl.
   rewrite c_shift_subs, c_shift_subs, <-v_shift_comm.
   apply rule. all: omega.
-+ clear V CI HC R VE CE HE WF. specialize βApp as rule.
++ clear V CI HC R VE CE HE WF.
+  specialize βApp as rule.
   unfold c_subs_out in *. simpl. rewrite c_shift_subs.
   apply rule. all: omega.
-+ clear V CI HC R VE CE HE WF. specialize βLetRec as rule.
++ clear V CI HC R VE CE HE WF.
+  specialize βLetRec as rule.
   unfold c_subs_out in *. simpl. rewrite c_shift_subs.
   simpl. rewrite <-c_shift_comm. apply rule. all: omega.
-+ clear V CI HC R VE CE HE WF. specialize βDoBind_Ret as rule.
++ clear V CI HC R VE CE HE WF.
+  specialize βDoBind_Ret as rule.
   unfold c_subs_out in *. simpl. rewrite c_shift_subs.
   apply rule. all: omega.
 + clear V CI HC R VE CE HE WF. simpl. rewrite <-c_shift_comm. 
   eapply βDoBind_Op. omega.
-+ clear V CI HC R VE CE HE WF. specialize βHandle_Ret as rule.
++ clear V CI HC R VE CE HE WF.
+  specialize βHandle_Ret as rule.
   unfold c_subs_out in *. simpl. rewrite c_shift_subs.
   apply rule. all: omega.
-+ clear V CI HC R VE CE HE WF. specialize βHandle_Op as rule.
++ clear V CI HC R VE CE HE WF.
+  specialize βHandle_Op as rule.
   unfold c_subs2_out in *. unfold c_subs_out in *. simpl.
   rewrite c_shift_subs, c_shift_subs, <-v_shift_comm.
   simpl. rewrite <-c_shift_comm, <-h_shift_comm.
   eapply rule. apply shift_get_case_Some. eauto. all: omega.
 + specialize (CI _ _ _ H2) as IHc.
-  clear V CI HC R VE CE HE WF. simpl.
-  destruct (n<=?i) eqn:ni.
+  clear V CI HC R VE CE HE WF.
+  simpl. destruct (n<=?i) eqn:ni.
   - apply leb_complete in ni.
     rewrite c_shift_subs. rewrite c_shift_subs. simpl.
     assert (S(S(S i))=2+(S i)) as same by omega.
     rewrite same, <-c_shift_comm. all: try omega.
-    eapply ηPair. specialize (ctx_len_insert_trivial Γ A_ins i) as triv. omega.
+    eapply ηPair. specialize (ctx_len_insert_trivial Γ i A_ins) as triv. omega.
     rewrite <-ctx_insert_comm; try omega. auto.  
   - apply leb_complete_conv in ni.
     rewrite c_shift_subs_alt, c_shift_subs_alt.
@@ -604,31 +666,34 @@ inv orig. destruct H1.
     eapply ηPair. rewrite ctx_len_insert; omega.
     rewrite ctx_insert_comm; try omega. auto.
 + specialize (CI _ _ _ H2) as IHc.
-  clear V CI HC R VE CE HE WF. simpl.
-  destruct (n<=?i) eqn:ni.
+  clear V CI HC R VE CE HE WF.
+  simpl. destruct (n<=?i) eqn:ni.
   - apply leb_complete in ni.
     rewrite c_shift_subs, c_shift_subs, c_shift_subs. simpl.
     assert (S(S i)=1+(S i)) as same by omega.
-    rewrite same, <-c_shift_comm. all: try omega.
-    eapply ηSum. specialize (ctx_len_insert_trivial Γ A_ins i) as triv. omega.
-    rewrite <-ctx_insert_comm; try omega. auto.  
+    rewrite same, <-c_shift_comm. all: aomega.
+    eapply ηSum. specialize (ctx_len_insert_trivial Γ i A_ins) as triv. omega.
+    rewrite <-ctx_insert_comm; aomega.  
   - apply leb_complete_conv in ni.
     rewrite c_shift_subs_alt, c_shift_subs_alt, c_shift_subs_alt. simpl.
-    rewrite <-c_shift_comm. all: try omega.
+    rewrite <-c_shift_comm. all: aomega.
     eapply ηSum. rewrite ctx_len_insert; omega.
-    rewrite ctx_insert_comm; try omega. auto. 
-+ clear V CI HC R VE CE HE WF. simpl. apply ηDoBind.
+    rewrite ctx_insert_comm; aomega. 
++ clear V CI HC R VE CE HE WF.
+  simpl. apply ηDoBind.
 }{
 intros wfins. inv orig. destruct H4. 
 + specialize (HC _ _ _ _ H2) as IH1.
   specialize (HC _ _ _ _ H3) as IH2.
-  clear V CI HC R VE CE HE WF. eapply Heq. 
+  clear V CI HC R VE CE HE WF.
+  eapply Heq. 
   2: exact H0. all: eauto. apply HeqSigØ. 
 + specialize (HC _ _ _ _ H2) as IH1.
   specialize (HC _ _ _ _ H3) as IH2.
   specialize (CE _ _ _ _ H6) as IHc.
   specialize (HE _ _ _ _ _ H7) as IHh.
-  clear V CI HC R VE CE HE WF. eapply Heq.
+  clear V CI HC R VE CE HE WF.
+  eapply Heq.
   2: exact H0. all: eauto. eapply HeqSigU.
   - eapply shift_get_case_Some in H4. eauto.
   - eapply shift_get_case_Some in H5. eauto.
@@ -640,11 +705,12 @@ intros wfins. inv orig.
   apply wf_ctx_insert; auto.
 + specialize (V _ _ _ H) as IHv.
   specialize (WF _ _ _ H0) as IHwf.
-  clear V CI HC R VE CE HE WF. simpl.
-  apply WfInstU; auto.
+  clear V CI HC R VE CE HE WF.
+  simpl. apply WfInstU; auto.
 }
 Qed.
 
+(* ==================== Shorter definitions ==================== *)
 
 Fixpoint v_shift_typesafe v (Γ:ctx) A0 A :
   has_vtype Γ v A -> wf_vtype A0 ->
@@ -680,7 +746,7 @@ with wf_inst_shift_typesafe Γ Γ' I A0 :
 
 Proof.
 all: intros orig;
-assert (ctx_insert Γ A0 0 = CtxU Γ A0) by (destruct Γ; auto);
+assert (ctx_insert Γ 0 A0 = CtxU Γ A0) by (destruct Γ; auto);
 rewrite <-H.
 apply v_insert_typesafe. assumption.
 apply c_insert_typesafe. assumption.
@@ -720,8 +786,8 @@ Fixpoint v_join_ctxs_typesafe_right Γ Γ' v A {struct Γ'}:
   has_vtype (join_ctxs Γ' Γ) v A.
 Proof.
 intros; destruct Γ'; simpl.
-+ rewrite join_ctxs_left_unit. assumption.
-+ rewrite join_ctxs_left_step.
++ rewrite join_ctxs_CtxØ. assumption.
++ rewrite join_ctxs_CtxU.
   apply v_join_ctxs_typesafe_right. 
   rewrite <-(v_shift_too_high _ 1 (ctx_len Γ)).
   apply v_insert_typesafe. auto. inv H0. auto.
@@ -731,7 +797,8 @@ Qed.
 
 Lemma v_join_all_ctxs_typesafe Γ Γ' Z D v A :
   has_vtype Γ' v A -> wf_ctx Γ -> wf_tctx Z -> wf_ctype D ->
-  has_vtype (join_ctxs (join_ctxs Γ' (tctx_to_ctx Z D)) Γ)
+  has_vtype 
+    (join_ctxs (join_ctxs Γ' (tctx_to_ctx Z D)) Γ)
     (v_shift v (tctx_len Z+ctx_len Γ) 0) A.
 Proof.
 intros. 
@@ -744,7 +811,8 @@ Qed.
 
 Lemma c_join_all_ctxs_typesafe Γ Γ' Z D c C :
   has_ctype Γ' c C -> wf_ctx Γ -> wf_tctx Z -> wf_ctype D ->
-  has_ctype (join_ctxs (join_ctxs Γ' (tctx_to_ctx Z D)) Γ)
+  has_ctype 
+    (join_ctxs (join_ctxs Γ' (tctx_to_ctx Z D)) Γ)
     (c_shift c (tctx_len Z+ctx_len Γ) 0) C.
 Proof.
 intros. 
@@ -753,6 +821,9 @@ apply c_join_ctxs_typesafe_left; auto.
 erewrite len_tctx_to_ctx. apply c_join_ctxs_typesafe_left. auto.
 apply wf_tctx_to_ctx; auto.
 Qed.
+
+
+(* ==================== Safety and Sub. ==================== *)
 
 
 Fixpoint v_sub_typesafe 
@@ -814,90 +885,109 @@ assumption. assumption. destruct H1.
   - apply TypeVar. assumption.
 + specialize (V _ _ _ H1) as IHv1. 
   specialize (V _ _ _ H2) as IHv2.
-  clear V CI HC R VE CE HE WF. simpl. apply TypePair; eauto.
-+ specialize (V _ _ _ H1) as IHv. clear V CI HC R VE CE HE WF. apply TypeInl; eauto.
-+ specialize (V _ _ _ H1) as IHv. clear V CI HC R VE CE HE WF. apply TypeInr; eauto.
-+ clear V CI HC R VE CE HE WF. apply TypeListNil; eauto.
+  clear V CI HC R VE CE HE WF.
+  simpl. apply TypePair; eauto.
++ specialize (V _ _ _ H1) as IHv. 
+  clear V CI HC R VE CE HE WF.
+  apply TypeInl; eauto.
++ specialize (V _ _ _ H1) as IHv.
+  clear V CI HC R VE CE HE WF.
+  apply TypeInr; eauto.
++ clear V CI HC R VE CE HE WF.
+  apply TypeListNil; eauto.
 + specialize (V _ _ _ H1) as IHv1. 
   specialize (V _ _ _ H2) as IHv2.
-  clear V CI HC R VE CE HE WF. simpl. apply TypeListCons; eauto.
+  clear V CI HC R VE CE HE WF.
+  simpl. apply TypeListCons; eauto.
 + specialize (CI _ _ _ H1) as IHc. 
   specialize (V _ _ _ tyvs) as IHvs.
-  clear V CI HC R VE CE HE WF. simpl.
-  apply TypeFun. eapply IHc. eauto. inv H0. apply v_shift_typesafe; auto.
+  clear V CI HC R VE CE HE WF.
+  simpl. apply TypeFun. eapply IHc. eauto.
+  inv H0. apply v_shift_typesafe; auto.
 + specialize (HC _ _ _ _ H2) as IHh. 
   specialize (CI _ _ _ H1) as IHc.
   specialize (R _ _ _ _ _ H3) as IHr.
-  clear V CI HC R VE CE HE WF. simpl. apply TypeHandler; eauto. eapply IHc. 
-  exact gets. inv H0. inv H6. apply v_shift_typesafe; assumption.
+  clear V CI HC R VE CE HE WF.
+  simpl. apply TypeHandler; eauto. eapply IHc. 
+  exact gets. inv H0. inv H6. apply v_shift_typesafe; auto.
 + specialize (V _ _ _ H1) as IHv.
-  clear V CI HC R VE CE HE WF. eapply TypeVSubtype; eauto.
+  clear V CI HC R VE CE HE WF.
+  eapply TypeVSubtype; eauto.
 }{
-intros gets tyvs. apply TypeC; inv orig.
-assumption. assumption. destruct H1.
+intros gets tyvs. apply TypeC; inv orig. auto. auto. destruct H1.
 + specialize (V _ _ _ H1) as IHv. 
-  clear V CI HC R VE CE HE WF. apply TypeRet; eauto.
+  clear V CI HC R VE CE HE WF.
+  apply TypeRet; eauto.
 + specialize (V _ _ _ H1) as IHv. 
-  clear V CI HC R VE CE HE WF. apply TypeAbsurd; eauto.
+  clear V CI HC R VE CE HE WF.
+  apply TypeAbsurd; eauto.
 + specialize (V _ _ _ H1) as IHv. 
   specialize (CI _ _ _ H2) as IHc.
-  clear V CI HC R VE CE HE WF. simpl. eapply TypeΠMatch; eauto.
+  clear V CI HC R VE CE HE WF.
+  simpl. eapply TypeΠMatch; eauto.
   - eapply IHc. exact gets. rewrite <-(v_shift_shift 1 1 0).
     apply v_shift_typesafe. apply v_shift_typesafe. assumption.
     all: inv H1; inv H4; assumption.
 + specialize (V _ _ _ H1) as IHv. 
   specialize (CI _ _ _ H2) as IHc1.
   specialize (CI _ _ _ H3) as IHc2.
-  clear V CI HC R VE CE HE WF. simpl. eapply TypeΣMatch. eauto.
+  clear V CI HC R VE CE HE WF.
+  simpl. eapply TypeΣMatch. eauto.
   - eapply IHc1. exact gets. inv H1. inv H5. apply v_shift_typesafe; auto. 
   - eapply IHc2. exact gets. inv H1. inv H5. apply v_shift_typesafe; auto.
 + specialize (V _ _ _ H1) as IHv. 
   specialize (CI _ _ _ H2) as IHc1.
   specialize (CI _ _ _ H3) as IHc2.
-  clear V CI HC R VE CE HE WF. simpl. eapply TypeListMatch. eauto.
+  clear V CI HC R VE CE HE WF.
+  simpl. eapply TypeListMatch. eauto.
   - eapply IHc1. exact gets. auto.
   - eapply IHc2. exact gets. rewrite <-(v_shift_shift 1 1 0).
     apply v_shift_typesafe. apply v_shift_typesafe. assumption.
     all: inv H1. inv H5. all:auto.
 + specialize (CI _ _ _ H1) as IHc1. 
   specialize (CI _ _ _ H2) as IHc2.
-  clear V CI HC R VE CE HE WF. simpl. eapply TypeDoBind. eauto.
+  clear V CI HC R VE CE HE WF.
+  simpl. eapply TypeDoBind. eauto.
   eapply IHc2. exact gets. inv H1. inv H4. apply v_shift_typesafe; auto. 
 + specialize (V _ _ _ H1) as IHv. 
   specialize (V _ _ _ H2) as IHv0.
-  clear V CI HC R VE CE HE WF. simpl. eapply TypeApp; eauto.
+  clear V CI HC R VE CE HE WF.
+  simpl. eapply TypeApp; eauto.
 + specialize (V _ _ _ H1) as IHv. 
   specialize (CI _ _ _ H2) as IHc.
-  clear V CI HC R VE CE HE WF. simpl. eapply TypeHandle; eauto.
+  clear V CI HC R VE CE HE WF.
+  simpl. eapply TypeHandle; eauto.
 + specialize (CI _ _ _ H1) as IHc1. 
   specialize (CI _ _ _ H2) as IHc2.
-  clear V CI HC R VE CE HE WF. simpl. eapply TypeLetRec.
+  clear V CI HC R VE CE HE WF.
+  simpl. eapply TypeLetRec.
   - eapply IHc1. exact gets. rewrite <-(v_shift_shift 1 1 0).
     apply v_shift_typesafe. apply v_shift_typesafe. assumption.
     all: inv H1; inv H3. 2: assumption. inv H7. assumption. 
   - eapply IHc2. exact gets. inv H1. inv H3. apply v_shift_typesafe; auto.
 + specialize (V _ _ _ H2) as IHv. 
   specialize (CI _ _ _ H3) as IHc.
-  clear V CI HC R VE CE HE WF. simpl. eapply TypeOp; eauto.
+  clear V CI HC R VE CE HE WF.
+  simpl. eapply TypeOp; eauto.
   eapply IHc. exact gets. inv H3. inv H4. apply v_shift_typesafe; auto.
 + specialize (CI _ _ _ H1) as IHc.
-  clear V CI HC R VE CE HE WF. eapply TypeCSubtype; eauto.
+  clear V CI HC R VE CE HE WF.
+  eapply TypeCSubtype; eauto.
 }{
-intros gets tyvs; simpl; apply TypeH; inv orig.
-all: try assumption.
+intros gets tyvs; simpl; apply TypeH; inv orig. auto. auto. auto.
 destruct H2.
 + clear V CI HC R VE CE HE WF. 
   apply TypeCasesØ.
 + specialize (HC _ _ _ _ H3) as IHh. 
   specialize (CI _ _ _ H4) as IHc.
-  clear V CI HC R VE CE HE WF. simpl. apply TypeCasesU; eauto.
-  - rewrite sub_get_case_None; auto.
+  clear V CI HC R VE CE HE WF.
+  simpl. apply TypeCasesU; eauto.
+  - rewrite <-sub_get_case_None; eauto.
   - eapply IHc. exact gets. rewrite <-(v_shift_shift 1 1 0).
     apply v_shift_typesafe. apply v_shift_typesafe. assumption.
     all: inv H0. 2: assumption. apply WfTyFun; assumption.
 }{
-intros htys gets tyvs; simpl. apply Respects; inv orig.
-all: try assumption.
+intros htys gets tyvs; simpl. apply Respects; inv orig; auto.
 destruct H3.
 + clear V CI HC R VE CE HE WF. 
   apply RespectEqsØ.
@@ -916,156 +1006,192 @@ intros gets tyvs. apply Veq.
 { inv orig; eauto. }
 inv orig. destruct H1.
 + specialize (VE _ _ _ _ H1) as IH.
-  clear V CI HC R VE CE HE WF. apply VeqSym. eauto.
+  clear V CI HC R VE CE HE WF.
+  apply VeqSym. eauto.
 + specialize (VE _ _ _ _ H1) as IH1.
   specialize (VE _ _ _ _ H2) as IH2.
-  clear V CI HC R VE CE HE WF. eapply VeqTrans; eauto.
-+ clear V CI HC R VE CE HE WF. subst. simpl.
+  clear V CI HC R VE CE HE WF.
+  eapply VeqTrans; eauto.
++ clear V CI HC R VE CE HE WF.
+  subst. simpl.
   destruct (i0 =? i) eqn:cmp.
   - apply veq_refl in tyvs.
     inv H0. apply Nat.eqb_eq in cmp. subst. rewrite gets in H1.
     inv H1. eapply veq_subtype in tyvs; eauto. inv tyvs. assumption.
   - eapply VeqVar; eauto.
-+ clear V CI HC R VE CE HE WF. simpl. apply VeqUnit.
-+ clear V CI HC R VE CE HE WF. simpl. apply VeqInt.
++ clear V CI HC R VE CE HE WF.
+  simpl. apply VeqUnit.
++ clear V CI HC R VE CE HE WF.
+  simpl. apply VeqInt.
 + specialize (VE _ _ _ _ H1) as IH1.
   specialize (VE _ _ _ _ H2) as IH2.
-  clear V CI HC R VE CE HE WF. simpl. apply VeqPair; eauto.
+  clear V CI HC R VE CE HE WF.
+  simpl. apply VeqPair; eauto.
 + specialize (VE _ _ _ _ H1) as IH.
-  clear V CI HC R VE CE HE WF. simpl. eapply VeqInl; eauto.
+  clear V CI HC R VE CE HE WF.
+  simpl. eapply VeqInl; eauto.
 + specialize (VE _ _ _ _ H1) as IH.
-  clear V CI HC R VE CE HE WF. simpl. eapply VeqInr; eauto.
-+ clear V CI HC R VE CE HE WF. simpl. apply VeqListNil; eauto.
+  clear V CI HC R VE CE HE WF.
+  simpl. eapply VeqInr; eauto.
++ clear V CI HC R VE CE HE WF.
+  simpl. apply VeqListNil; eauto.
 + specialize (VE _ _ _ _ H1) as IH1.
   specialize (VE _ _ _ _ H2) as IH2.
-  clear V CI HC R VE CE HE WF. simpl. apply VeqListCons; eauto.
+  clear V CI HC R VE CE HE WF.
+    simpl. apply VeqListCons; eauto.
 + specialize (CE _ _ _ _ H1) as IH.
-  clear V CI HC R VE CE HE WF. simpl. eapply VeqFun. eapply IH.
+  clear V CI HC R VE CE HE WF.
+    simpl. eapply VeqFun. eapply IH.
   - simpl. eauto.
   - inv H. inv H3. apply v_shift_typesafe; auto.
 + specialize (CE _ _ _ _ H1) as IHc.
   specialize (HE _ _ _ _ _ H2) as IHh.
-  clear V CI HC R VE CE HE WF. simpl. eapply VeqHandler; eauto. eapply IHc.
+  clear V CI HC R VE CE HE WF.
+  simpl. eapply VeqHandler; eauto. eapply IHc.
   - simpl. eauto.
   - inv H. inv H5. inv H8. apply v_shift_typesafe; auto.
-+ clear V CI HC R VE CE HE WF. simpl. apply ηUnit.
-+ clear V CI HC R VE CE HE WF. simpl. rewrite <-v_shift_sub. apply ηFun. omega.
++ clear V CI HC R VE CE HE WF.
+  simpl. apply ηUnit.
++ clear V CI HC R VE CE HE WF.
+  simpl. rewrite <-v_shift_sub. apply ηFun. omega.
 }{
 intros gets vtys. apply Ceq.
 { inv orig; eauto. }
 { inv orig; eauto. }
 inv orig. destruct H1.
 + specialize (CE _ _ _ _ H1) as IH.
-  clear V CI HC R VE CE HE WF. apply CeqSym. eauto.
+  clear V CI HC R VE CE HE WF.
+  apply CeqSym. eauto.
 + specialize (CE _ _ _ _ H1) as IH1.
   specialize (CE _ _ _ _ H2) as IH2.
-  clear V CI HC R VE CE HE WF. eapply CeqTrans; eauto.
+  clear V CI HC R VE CE HE WF.
+  eapply CeqTrans; eauto.
 + specialize (VE _ _ _ _ H1) as IH.
-  clear V CI HC R VE CE HE WF. simpl. apply CeqRet. eauto.
+  clear V CI HC R VE CE HE WF.
+  simpl. apply CeqRet. eauto.
 + specialize (VE _ _ _ _ H1) as IH.
-  clear V CI HC R VE CE HE WF. simpl. apply CeqAbsurd. eauto.
+  clear V CI HC R VE CE HE WF.
+  simpl. apply CeqAbsurd. eauto.
 + specialize (VE _ _ _ _ H1) as IHv.
   specialize (CE _ _ _ _ H2) as IHc.
-  clear V CI HC R VE CE HE WF. simpl. eapply CeqΠMatch. eauto. eapply IHc.
+  clear V CI HC R VE CE HE WF.
+  simpl. eapply CeqΠMatch. eauto. eapply IHc.
   - simpl. eauto.
   - inv H1. inv H3. inv H6. rewrite <-(v_shift_shift 1 1).
     apply v_shift_typesafe; auto. apply v_shift_typesafe; auto.
 + specialize (VE _ _ _ _ H1) as IHv.
   specialize (CE _ _ _ _ H2) as IHc1.
   specialize (CE _ _ _ _ H3) as IHc2.
-  clear V CI HC R VE CE HE WF. simpl. eapply CeqΣMatch. eauto. all: inv H1; inv H4.
+  clear V CI HC R VE CE HE WF.
+  simpl. eapply CeqΣMatch. eauto. all: inv H1; inv H4.
   - eapply IHc1. simpl. eauto. inv H7. apply v_shift_typesafe; assumption.
   - eapply IHc2. simpl. eauto. inv H7. apply v_shift_typesafe; assumption.
 + specialize (VE _ _ _ _ H1) as IHv.
   specialize (CE _ _ _ _ H2) as IHc1.
   specialize (CE _ _ _ _ H3) as IHc2.
-  clear V CI HC R VE CE HE WF. simpl. eapply CeqListMatch. eauto.
+  clear V CI HC R VE CE HE WF.
+  simpl. eapply CeqListMatch. eauto.
   - eapply IHc1; eauto.
   - eapply IHc2. simpl. eauto. rewrite <-(v_shift_shift 1 1).
     apply v_shift_typesafe. apply v_shift_typesafe. auto.
     all: inv H1; inv H4. inv H7. auto. auto.
 + specialize (CE _ _ _ _ H1) as IHc1.
   specialize (CE _ _ _ _ H2) as IHc2.
-  clear V CI HC R VE CE HE WF. simpl. eapply CeqDoBind. eauto. eapply IHc2.
+  clear V CI HC R VE CE HE WF.
+  simpl. eapply CeqDoBind. eauto. eapply IHc2.
   - simpl. eauto.
   - inv H1. inv H3. inv H6. apply v_shift_typesafe; assumption.
 + specialize (VE _ _ _ _ H1) as IHv1.
   specialize (VE _ _ _ _ H2) as IHv2.
-  clear V CI HC R VE CE HE WF. simpl. eapply CeqApp; eauto.
+  clear V CI HC R VE CE HE WF.
+  simpl. eapply CeqApp; eauto.
 + specialize (VE _ _ _ _ H1) as IHv.
   specialize (CE _ _ _ _ H2) as IHc.
-  clear V CI HC R VE CE HE WF. simpl. eapply CeqHandle; eauto.
+  clear V CI HC R VE CE HE WF.
+  simpl. eapply CeqHandle; eauto.
 + specialize (CE _ _ _ _ H1) as IHc1.
   specialize (CE _ _ _ _ H2) as IHc2.
-  clear V CI HC R VE CE HE WF. simpl. inv H2. inv H4. eapply CeqLetRec.
+  clear V CI HC R VE CE HE WF.
+  simpl. inv H2. inv H4. eapply CeqLetRec.
   - eapply IHc1. simpl. eauto. rewrite <-(v_shift_shift 1 1).
     inv H2. apply v_shift_typesafe; auto. inv H10. apply v_shift_typesafe; auto.
   - eapply IHc2. simpl. eauto. inv H2. apply v_shift_typesafe; assumption.
 + specialize (VE _ _ _ _ H2) as IHv.
   specialize (CE _ _ _ _ H3) as IHc.
-  clear V CI HC R VE CE HE WF. simpl. eapply CeqOp; eauto.
+  clear V CI HC R VE CE HE WF.
+  simpl. eapply CeqOp; eauto.
   eapply IHc. simpl. eauto. apply v_shift_typesafe. assumption.
   apply get_op_type_wf in H1. destruct H1. assumption. inv H. inv H5. auto.
 + specialize (WF _ _ _ H2) as IHwf.
-  clear V CI HC R VE CE HE WF. clear H2. eapply OOTB; eauto.
+  clear V CI HC R VE CE HE WF.
+  clear H2. eapply OOTB; eauto.
   rewrite <-c_sub_inst. rewrite H3. simpl. auto.
   rewrite <-c_sub_inst. rewrite H4. simpl. auto.
-+ clear V CI HC R VE CE HE WF. specialize βΠMatch as rule.
++ clear V CI HC R VE CE HE WF.
+  specialize βΠMatch as rule.
   unfold c_subs2_out in *. unfold c_subs_out in *. simpl.
   rewrite c_sub_subs, c_sub_subs, <-v_shift_sub, v_shift_shift.
   apply rule. all: omega.
-+ clear V CI HC R VE CE HE WF. specialize βΣMatch_Inl as rule.
++ clear V CI HC R VE CE HE WF.
+  specialize βΣMatch_Inl as rule.
   unfold c_subs_out in *. simpl. rewrite c_sub_subs.
   apply rule. all: omega.
-+ clear V CI HC R VE CE HE WF. specialize βΣMatch_Inr as rule.
++ clear V CI HC R VE CE HE WF.
+  specialize βΣMatch_Inr as rule.
   unfold c_subs_out in *. simpl. rewrite c_sub_subs.
   apply rule. all: omega.
-+ clear V CI HC R VE CE HE WF. specialize βListMatch_Nil as rule.
++ clear V CI HC R VE CE HE WF.
+  specialize βListMatch_Nil as rule.
   unfold c_subs_out in *. simpl. apply rule. all: omega.
-+ clear V CI HC R VE CE HE WF. specialize βListMatch_Cons as rule.
++ clear V CI HC R VE CE HE WF.
+  specialize βListMatch_Cons as rule.
   unfold c_subs2_out in *. unfold c_subs_out in *. simpl.
   rewrite c_sub_subs, c_sub_subs, <-v_shift_sub, v_shift_shift.
   apply rule. all: omega.
-+ clear V CI HC R VE CE HE WF. specialize βApp as rule.
++ clear V CI HC R VE CE HE WF.
+  specialize βApp as rule.
   unfold c_subs_out in *. simpl. rewrite c_sub_subs.
   apply rule. all: omega.
-+ clear V CI HC R VE CE HE WF. specialize βLetRec as rule.
++ clear V CI HC R VE CE HE WF.
+  specialize βLetRec as rule.
   unfold c_subs_out in *. simpl. rewrite c_sub_subs.
   simpl. rewrite v_shift_comm, <-c_shift_sub, v_shift_shift. 
   apply rule. all: omega.
-+ clear V CI HC R VE CE HE WF. specialize βDoBind_Ret as rule.
++ clear V CI HC R VE CE HE WF.
+  specialize βDoBind_Ret as rule.
   unfold c_subs_out in *. simpl. rewrite c_sub_subs.
   apply rule. all: omega.
-+ clear V CI HC R VE CE HE WF. specialize βDoBind_Op as rule.
++ clear V CI HC R VE CE HE WF.
+  specialize βDoBind_Op as rule.
   simpl. rewrite v_shift_comm, <-c_shift_sub. 
   apply rule. all: omega.
-+ clear V CI HC R VE CE HE WF. specialize βHandle_Ret as rule.
++ clear V CI HC R VE CE HE WF.
+  specialize βHandle_Ret as rule.
   unfold c_subs_out in *. simpl. rewrite c_sub_subs.
   apply rule. all: omega.
-+ clear V CI HC R VE CE HE WF. specialize βHandle_Op as rule.
++ clear V CI HC R VE CE HE WF.
+  specialize βHandle_Op as rule.
   unfold c_subs2_out in *. unfold c_subs_out in *. simpl.
   rewrite c_sub_subs, c_sub_subs, <-v_shift_sub, v_shift_shift.
   simpl. rewrite v_shift_comm, <-c_shift_sub, <-h_shift_sub.
   simpl in rule. eapply rule. apply sub_get_case_Some. eauto. all: omega.
 + specialize (CI _ _ _ H2) as IHc.
-  clear V CI HC R VE CE HE WF. simpl.
-  destruct (n<=?i) eqn:ni.
+  clear V CI HC R VE CE HE WF.
+  simpl. destruct (n<=?i) eqn:ni.
   - apply leb_complete in ni.
     rewrite c_sub_subs, c_sub_subs. simpl.
     assert (S(S n)=2+n) as samen by omega.
     assert (S(S(S i))=2+(S i)) as samei by omega.
-    rewrite samei, samen, <-v_shift_comm.
-    rewrite <-c_shift_sub. all: try omega.
+    rewrite samei, samen, <-v_shift_comm, <-c_shift_sub. all: aomega.
     eapply ηPair. auto. eapply IHc.
     * erewrite <-get_ctx_insert_changed. eauto. omega.
     * apply v_insert_typesafe; auto. inv H2. 
       apply wf_ctx_insert_vtype in H3. auto. omega.
   - apply leb_complete_conv in ni.
-    rewrite c_sub_subs_alt, c_sub_subs_alt.
+    rewrite c_sub_subs_alt, c_sub_subs_alt; aomega.
     assert (S(S i)=2+i) as samei by omega.
     assert (S(S n)=2+n) as samen by omega.
-    simpl. rewrite samei, samen, <-v_shift_comm. 
-    rewrite <-c_shift_sub. all : try omega.
+    simpl. rewrite samei, samen, <-v_shift_comm, <-c_shift_sub; aomega.
     eapply ηPair. omega. eapply IHc.
     * erewrite <-get_ctx_insert_unchanged. eauto. omega.
     * apply v_insert_typesafe; auto. inv H2. 
@@ -1074,17 +1200,16 @@ inv orig. destruct H1.
   clear V CI HC R VE CE HE WF. simpl.
   destruct (n<=?i) eqn:ni.
   - apply leb_complete in ni.
-    rewrite c_sub_subs, c_sub_subs, c_sub_subs. simpl.
+    rewrite c_sub_subs, c_sub_subs, c_sub_subs; aomega. simpl.
     assert (S(S i)=1+(S i)) as samei by omega.
-    rewrite samei, <-v_shift_comm.
-    rewrite <-c_shift_sub. all: try omega.
+    rewrite samei, <-v_shift_comm, <-c_shift_sub; aomega.
     eapply ηSum. auto. eapply IHc.
     * erewrite <-get_ctx_insert_changed. eauto. omega.
     * apply v_insert_typesafe; auto. inv H2. 
       apply wf_ctx_insert_vtype in H3. auto. omega.
   - apply leb_complete_conv in ni.
     rewrite c_sub_subs_alt, c_sub_subs_alt, c_sub_subs_alt. simpl.
-    rewrite <-v_shift_comm, <-c_shift_sub. all: try omega.
+    rewrite <-v_shift_comm, <-c_shift_sub. all: aomega.
     eapply ηSum. omega. eapply IHc.
     * erewrite <-get_ctx_insert_unchanged. eauto. omega.
     * apply v_insert_typesafe; auto. inv H2. 
@@ -1095,70 +1220,74 @@ intros gets vtys.
 inv orig. destruct H4.
 + specialize (HC _ _ _ _ H2) as IH1.
   specialize (HC _ _ _ _ H3) as IH2.
-  clear V CI HC R VE CE HE WF. eapply Heq. 
-  2: exact H0. all: eauto. apply HeqSigØ. 
+  clear V CI HC R VE CE HE WF.
+  eapply Heq. 2: exact H0. all: eauto. apply HeqSigØ. 
 + specialize (HC _ _ _ _ H2) as IH1.
   specialize (HC _ _ _ _ H3) as IH2.
   specialize (CE _ _ _ _ H6) as IHc.
   specialize (HE _ _ _ _ _ H7) as IHh.
-  clear V CI HC R VE CE HE WF. eapply Heq.
-  2: exact H0. all: eauto. eapply HeqSigU.
+  clear V CI HC R VE CE HE WF.
+  eapply Heq. 2: exact H0. all: eauto. eapply HeqSigU.
   - eapply sub_get_case_Some in H4. eauto.
   - eapply sub_get_case_Some in H5. eauto.
   - eapply IHc. simpl. eauto. rewrite <-(v_shift_shift 1 1). 
     apply v_shift_typesafe. apply v_shift_typesafe; auto.
-    all: inv H6; inv H8; inv H6. inv H14. assumption. assumption.
+    all: inv H6; inv H8; inv H6. inv H14. all: auto.
   - eauto.
 }{
 intros gets vtys. destruct orig.
-+ clear V CI HC R VE CE HE WF. simpl. apply WfInstØ. auto.
++ clear V CI HC R VE CE HE WF.
+  simpl. apply WfInstØ. auto.
 + specialize (V _ _ _ H) as IHv.
   specialize (WF _ _ _ orig) as IHwf.
-  clear V CI HC R VE CE HE WF. simpl.
-  apply WfInstU; eauto.
+  clear V CI HC R VE CE HE WF. 
+  simpl. apply WfInstU; eauto.
 }
 Qed.
 
 
+(* ==================== Safety and Subs. ==================== *)
+
+
 Fixpoint v_subs_typesafe 
   Γ Γ' v A i v_s A_s (orig: has_vtype Γ' v A) {struct orig}:
-  has_vtype Γ v_s A_s -> Γ' = ctx_insert Γ A_s i -> ctx_len Γ >= i ->
+  has_vtype Γ v_s A_s -> Γ' = ctx_insert Γ i A_s -> ctx_len Γ >= i ->
   has_vtype Γ (v_subs v i v_s) A
 
 with c_subs_typesafe
   Γ Γ' c C i v_s A_s (orig: has_ctype Γ' c C) {struct orig}:
-  has_vtype Γ v_s A_s -> Γ' = ctx_insert Γ A_s i -> ctx_len Γ >= i ->
+  has_vtype Γ v_s A_s -> Γ' = ctx_insert Γ i A_s -> ctx_len Γ >= i ->
   has_ctype Γ (c_subs c i v_s) C
 
 with h_subs_typesafe
   Γ Γ' h Σ D i v_s A_s (orig: has_htype Γ' h Σ D) {struct orig}:
-  has_vtype Γ v_s A_s -> Γ' = ctx_insert Γ A_s i -> ctx_len Γ >= i ->
+  has_vtype Γ v_s A_s -> Γ' = ctx_insert Γ i A_s -> ctx_len Γ >= i ->
   has_htype Γ (h_subs h i v_s) Σ D
 
 with respects_subs_typesafe
   Γ Γ' h Σ D E i v_s A_s (orig: respects Γ' h Σ D E) {struct orig} :
-  has_htype Γ' h Σ D -> has_vtype Γ v_s A_s -> Γ' = ctx_insert Γ A_s i ->
+  has_htype Γ' h Σ D -> has_vtype Γ v_s A_s -> Γ' = ctx_insert Γ i A_s ->
   ctx_len Γ >= i ->
   respects Γ (h_subs h i v_s) Σ D E
 
 with veq_subs_typesafe
   Γ Γ' A v1 v2 i v_s A_s (orig: veq A Γ' v1 v2) {struct orig} :
-  has_vtype Γ v_s A_s -> Γ' = ctx_insert Γ A_s i -> ctx_len Γ >= i ->
+  has_vtype Γ v_s A_s -> Γ' = ctx_insert Γ i A_s -> ctx_len Γ >= i ->
   veq A Γ (v_subs v1 i v_s) (v_subs v2 i v_s)
 
 with ceq_subs_typesafe
   Γ Γ' C c1 c2 i v_s A_s (orig: ceq C Γ' c1 c2) {struct orig} :
-  has_vtype Γ v_s A_s -> Γ' = ctx_insert Γ A_s i -> ctx_len Γ >= i ->
+  has_vtype Γ v_s A_s -> Γ' = ctx_insert Γ i A_s -> ctx_len Γ >= i ->
   ceq C Γ (c_subs c1 i v_s) (c_subs c2 i v_s)
 
 with heq_subs_typesafe
   Γ Γ' Σ D h1 h2 i v_s A_s (orig: heq Σ D Γ' h1 h2) {struct orig} :
-  has_vtype Γ v_s A_s -> Γ' = ctx_insert Γ A_s i -> ctx_len Γ >= i ->
+  has_vtype Γ v_s A_s -> Γ' = ctx_insert Γ i A_s -> ctx_len Γ >= i ->
   heq Σ D Γ (h_subs h1 i v_s) (h_subs h2 i v_s)
 
 with wf_inst_subs_typesafe
   Γ Γ' I Γ0 i v_s A_s (orig: wf_inst Γ' I Γ0) {struct orig} :
-  has_vtype Γ v_s A_s -> Γ' = ctx_insert Γ A_s i -> ctx_len Γ >= i ->
+  has_vtype Γ v_s A_s -> Γ' = ctx_insert Γ i A_s -> ctx_len Γ >= i ->
   wf_inst Γ (inst_subs I i v_s) Γ0.
 
 Proof.
@@ -1171,15 +1300,19 @@ intros tyvs geq len.
 assert (wf_ctx Γ) as wfg by (inv tyvs; assumption).
 destruct orig. destruct H1.
 + clear V CI HC R VE CE HE WF. 
-  apply TypeV; auto; unfold v_subs; simpl. apply TypeUnit.
+  apply TypeV; auto; unfold v_subs; simpl.
+  apply TypeUnit.
 + clear V CI HC R VE CE HE WF. 
-  apply TypeV; auto; unfold v_subs; simpl. apply TypeInt.
+  apply TypeV; auto; unfold v_subs; simpl.
+  apply TypeInt.
 + clear V CI HC R VE CE HE WF. 
-  apply TypeV; auto; unfold v_subs; simpl. destruct (n=?i) eqn:ni.
+  apply TypeV; auto; unfold v_subs; simpl.
+  destruct (n=?i) eqn:ni.
   - apply Nat.eqb_eq in ni. subst.
     rewrite v_negshift_shift, v_shift_0. erewrite get_ctx_insert_new in H1.
     inv tyvs. inv H1. assumption. auto. omega.
-  - subst. simpl. destruct (i<=?n) eqn:cmp; apply TypeVar.
+  - subst. simpl. destruct (i<=?n) eqn:cmp;
+    apply TypeVar.
     * erewrite get_ctx_insert_changed.
       all: apply Nat.eqb_neq in ni; apply leb_complete in cmp.
       assert (1+(n-1)=n) by omega. rewrite H2. eauto. omega.
@@ -1188,36 +1321,42 @@ destruct orig. destruct H1.
 + specialize (V Γ Γ0 v1 _ i _ _ H1 tyvs geq) as IH1.
   specialize (V Γ Γ0 v2 _ i _ _ H2 tyvs geq) as IH2.
   clear V CI HC R VE CE HE WF.
-  apply TypeV; auto; unfold v_subs; simpl. apply TypePair; auto.  
+  apply TypeV; auto; unfold v_subs; simpl.
+  apply TypePair; auto.  
 + specialize (V Γ Γ0 v _ i _ _ H1 tyvs geq) as IH.
   clear V CI HC R VE CE HE WF.
-  apply TypeV; auto; unfold v_subs; simpl. apply TypeInl; auto.  
+  apply TypeV; auto; unfold v_subs; simpl.
+  apply TypeInl; auto.  
 + specialize (V Γ Γ0 v _ i _ _ H1 tyvs geq) as IH.
   clear V CI HC R VE CE HE WF.
-  apply TypeV; auto; unfold v_subs; simpl. apply TypeInr; auto.
+  apply TypeV; auto; unfold v_subs; simpl.
+  apply TypeInr; auto.
 + clear V CI HC R VE CE HE WF.
-  apply TypeV; auto; unfold v_subs; simpl. apply TypeListNil; auto.
+  apply TypeV; auto; unfold v_subs; simpl.
+  apply TypeListNil; auto.
 + specialize (V Γ Γ0 v _ i _ _ H1 tyvs geq) as IH1.
   specialize (V Γ Γ0 vs _ i _ _ H2 tyvs geq) as IH2.
   clear V CI HC R VE CE HE WF.
-  apply TypeV; auto; unfold v_subs; simpl. apply TypeListCons; auto.
-+ assert (CtxU Γ0 A = ctx_insert (CtxU Γ A) A_s (1+i)).
+  apply TypeV; auto; unfold v_subs; simpl.
+  apply TypeListCons; auto.
++ assert (CtxU Γ0 A = ctx_insert (CtxU Γ A) (1+i) A_s).
   { simpl. f_equal. auto. }
   inv H0. specialize (v_shift_typesafe _ Γ A _ tyvs H5) as tyvs'.
   specialize (CI _ _ c _ (1+i) _ _ H1 tyvs') as IH. 
   clear V CI HC R VE CE HE WF.
-  apply TypeV; auto; unfold v_subs; simpl. apply WfTyFun; auto. apply TypeFun. 
-  rewrite v_shift_comm. apply IH. simpl. f_equal. simpl. omega. omega.
-+ assert (CtxU Γ0 A = ctx_insert (CtxU Γ A) A_s (1+i)).
+  apply TypeV; auto; unfold v_subs; simpl. apply WfTyFun; auto.
+  apply TypeFun. rewrite v_shift_comm. apply IH.
+  simpl. f_equal. simpl. omega. omega.
++ assert (CtxU Γ0 A = ctx_insert (CtxU Γ A) (1+i) A_s).
   { simpl. f_equal. auto. }
   assert (wf_vtype A) as wfa by (inv H0; inv H7; assumption).
   specialize (v_shift_typesafe _ Γ A _ tyvs wfa) as tyvs'.
-  specialize (CI _ _ c_ret _ (1+i) _ _ H1 tyvs' H4) as IHc. 
+  specialize (CI _ _ cr _ (1+i) _ _ H1 tyvs' H4) as IHc. 
   specialize (HC _ _ h _ _ i _ _ H2 tyvs geq) as IHh. 
   specialize (R _ _ h _ _ _ i _ _ H3 H2 tyvs) as IHr.
   clear V CI HC R VE CE HE WF.
-  apply TypeV; auto; unfold v_subs; simpl. apply TypeHandler. 
-  rewrite v_shift_comm. apply IHc. simpl. omega. omega. auto. auto.
+  apply TypeV; auto; unfold v_subs; simpl.
+  apply TypeHandler. rewrite v_shift_comm. apply IHc. simpl. all: aomega.
 + specialize (V Γ Γ0 v _ i _ _ H1 tyvs geq) as IH.
   clear V CI HC R VE CE HE WF.
   apply TypeV; auto; unfold v_subs; simpl. 
@@ -1228,11 +1367,13 @@ assert (wf_ctx Γ) as wfg by (inv tyvs; assumption).
 destruct orig. destruct H1. 
 + specialize (V _ _ v _ i _ _ H1 tyvs) as IH.
   clear V CI HC R VE CE HE WF.
-  apply TypeC; auto; unfold c_subs; simpl. apply TypeRet. auto.
+  apply TypeC; auto; unfold c_subs; simpl.
+  apply TypeRet. auto.
 + specialize (V _ _ v _ i _ _ H1 tyvs) as IH.
   clear V CI HC R VE CE HE WF.
-  apply TypeC; auto; unfold c_subs; simpl. apply TypeAbsurd. auto.
-+ assert (CtxU (CtxU Γ0 A) B = ctx_insert (CtxU (CtxU Γ A) B) A_s (2+i)).
+  apply TypeC; auto; unfold c_subs; simpl.
+  apply TypeAbsurd. auto.
++ assert (CtxU (CtxU Γ0 A) B = ctx_insert (CtxU (CtxU Γ A) B) (2+i) A_s).
   { simpl. f_equal. f_equal. auto. }
   assert (wf_vtype A) as wfa by (inv H1; inv H5; auto).
   assert (wf_vtype B) as wfb by (inv H1; inv H5; auto).
@@ -1241,12 +1382,13 @@ destruct orig. destruct H1.
   specialize (v_shift_typesafe _ _ B _ tyvs' wfb) as tyvs''.
   specialize (CI _ _ c _ (2+i) _ _ H2 tyvs'' H3) as IHc.
   clear V CI HC R VE CE HE WF.
-  apply TypeC; auto; unfold c_subs; simpl. eapply TypeΠMatch. eauto. 
+  apply TypeC; auto; unfold c_subs; simpl.
+  eapply TypeΠMatch. eauto. 
   rewrite v_shift_shift in IHc. rewrite v_shift_comm. apply IHc.
   simpl. omega. omega.
-+ assert (CtxU Γ0 A = ctx_insert (CtxU Γ A) A_s (1+i)) as geqa.
++ assert (CtxU Γ0 A = ctx_insert (CtxU Γ A) (1+i) A_s) as geqa.
   { simpl. f_equal. auto. }
-  assert (CtxU Γ0 B = ctx_insert (CtxU Γ B) A_s (1+i)) as geqb.
+  assert (CtxU Γ0 B = ctx_insert (CtxU Γ B) (1+i) A_s) as geqb.
   { simpl. f_equal. auto. }
   assert (wf_vtype A) as wfa by (inv H1; inv H5; auto).
   assert (wf_vtype B) as wfb by (inv H1; inv H5; auto).
@@ -1256,11 +1398,12 @@ destruct orig. destruct H1.
   specialize (CI _ _ c1 _ (1+i) _ _ H2 tyvsa geqa) as IHc1.
   specialize (CI _ _ c2 _ (1+i) _ _ H3 tyvsb geqb) as IHc2.
   clear V CI HC R VE CE HE WF.
-  apply TypeC; auto; unfold c_subs; simpl. eapply TypeΣMatch. eauto. 
+  apply TypeC; auto; unfold c_subs; simpl.
+  eapply TypeΣMatch. eauto. 
   - rewrite v_shift_comm. apply IHc1. simpl. omega. omega.
   - rewrite v_shift_comm. apply IHc2. simpl. omega. omega.
 + assert (CtxU (CtxU Γ0 A) (TyList A) 
-    = ctx_insert (CtxU (CtxU Γ A) (TyList A)) A_s (2+i)).
+    = ctx_insert (CtxU (CtxU Γ A) (TyList A)) (2+i) A_s).
   { simpl. f_equal. f_equal. auto. }
   assert (wf_vtype A) as wfa by (inv H1; inv H6; auto).
   assert (wf_vtype (TyList A)) as wfla by (inv H1; auto).
@@ -1270,30 +1413,34 @@ destruct orig. destruct H1.
   specialize (CI _ _ c1 _ i _ _ H2 tyvs geq) as IHc1.
   specialize (CI _ _ c2 _ (2+i) _ _ H3 tyvs'' H4) as IHc2.
   clear V CI HC R VE CE HE WF.
-  apply TypeC; auto; unfold c_subs; simpl. eapply TypeListMatch; eauto. 
+  apply TypeC; auto; unfold c_subs; simpl.
+  eapply TypeListMatch; eauto. 
   rewrite v_shift_shift in IHc2. rewrite v_shift_comm. apply IHc2.
   simpl. omega. omega.
-+ assert (CtxU Γ0 A = ctx_insert (CtxU Γ A) A_s (1+i)) as geqa.
++ assert (CtxU Γ0 A = ctx_insert (CtxU Γ A) (1+i) A_s) as geqa.
   { simpl. f_equal. auto. }
   assert (wf_vtype A) as wfa by (inv H1; inv H4; auto).
   specialize (v_shift_typesafe _ _ A _ tyvs wfa) as tyvsa.
   specialize (CI _ _ c1 _ i _ _ H1 tyvs geq) as IHc1.
   specialize (CI _ _ c2 _ (1+i) _ _ H2 tyvsa geqa) as IHc2.
   clear V CI HC R VE CE HE WF.
-  apply TypeC; auto; unfold c_subs; simpl. eapply TypeDoBind. eauto. 
+  apply TypeC; auto; unfold c_subs; simpl.
+  eapply TypeDoBind. eauto. 
   rewrite v_shift_comm. apply IHc2. simpl. omega. omega.
 + specialize (V _ _ v1 _ i _ _ H1 tyvs) as IH1.
   specialize (V _ _ v2 _ i _ _ H2 tyvs) as IH2.
   clear V CI HC R VE CE HE WF.
-  apply TypeC; auto; unfold c_subs; simpl. eapply TypeApp. eauto. eauto.
+  apply TypeC; auto; unfold c_subs; simpl.
+  eapply TypeApp. eauto. eauto.
 + specialize (V _ _ v _ i _ _ H1 tyvs) as IHv.
   specialize (CI _ _ c _ i _ _ H2 tyvs) as IHc.
   clear V CI HC R VE CE HE WF.
-  apply TypeC; auto; unfold c_subs; simpl. eapply TypeHandle. eauto. eauto.
+  apply TypeC; auto; unfold c_subs; simpl.
+  eapply TypeHandle. eauto. eauto.
 + assert (CtxU (CtxU Γ0 A) (TyFun A C) 
-    = ctx_insert (CtxU (CtxU Γ A) (TyFun A C)) A_s (2+i)).
+    = ctx_insert (CtxU (CtxU Γ A) (TyFun A C)) (2+i) A_s).
   { simpl. f_equal. f_equal. auto. }
-  assert (CtxU Γ0 (TyFun A C) = ctx_insert (CtxU Γ (TyFun A C)) A_s (1+i)).
+  assert (CtxU Γ0 (TyFun A C) = ctx_insert (CtxU Γ (TyFun A C)) (1+i) A_s).
   { simpl. f_equal. auto. }
   assert (wf_vtype A) as wfa by (inv H1; inv H5; inv H10; auto).
   assert (wf_ctype C) as wfc by (inv H1; inv H5; inv H10; auto).
@@ -1305,18 +1452,20 @@ destruct orig. destruct H1.
   specialize (CI _ _ c1 _ (2+i) _ _ H1 tyvs'' H3) as IHc1.
   specialize (CI _ _ c2 _ (1+i) _ _ H2 tyvs''' H4) as IHc2.
   clear V CI HC R VE CE HE WF.
-  apply TypeC; auto; unfold c_subs; simpl. eapply TypeLetRec. 
+  apply TypeC; auto; unfold c_subs; simpl.
+  eapply TypeLetRec. 
   - rewrite v_shift_shift in IHc1. rewrite v_shift_comm. apply IHc1. 
     simpl. omega. omega.
   - rewrite v_shift_comm. apply IHc2. simpl. omega. omega.
-+ assert (CtxU Γ0 B_op = ctx_insert (CtxU Γ B_op) A_s (1+i)) as geqb.
++ assert (CtxU Γ0 Bop = ctx_insert (CtxU Γ Bop) (1+i) A_s) as geqb.
   { simpl. f_equal. auto. }
-  assert (wf_vtype B_op) as wfb by (inv H3; inv H4; auto).
-  specialize (v_shift_typesafe _ _ B_op _ tyvs wfb) as tyvsb.
+  assert (wf_vtype Bop) as wfb by (inv H3; inv H4; auto).
+  specialize (v_shift_typesafe _ _ Bop _ tyvs wfb) as tyvsb.
   specialize (V _ _ v _ i _ _ H2 tyvs geq) as IHv.
   specialize (CI _ _ c _ (1+i) _ _ H3 tyvsb geqb) as IHc.
   clear V CI HC R VE CE HE WF.
-  apply TypeC; auto; unfold c_subs; simpl. eapply TypeOp; eauto.
+  apply TypeC; auto; unfold c_subs; simpl.
+  eapply TypeOp; eauto.
   rewrite v_shift_comm. apply IHc. simpl. omega. omega.
 + specialize (CI Γ Γ0 c _ i _ _ H1 tyvs geq) as IH.
   clear V CI HC R VE CE HE WF.
@@ -1327,20 +1476,21 @@ intros tyvs geq len.
 assert (wf_ctx Γ) as wfg by (inv tyvs; assumption).
 destruct orig. destruct H2. 
 + clear V CI HC R VE CE HE WF.
-  apply TypeH; auto; unfold h_subs; simpl. apply TypeCasesØ.
-+ assert (CtxU (CtxU Γ0 (TyFun B_op D)) A_op 
-    = ctx_insert (CtxU (CtxU Γ (TyFun B_op D)) A_op) A_s (2+i)).
+  apply TypeH; auto; unfold h_subs; simpl.
+  apply TypeCasesØ.
++ assert (CtxU (CtxU Γ0 (TyFun Bop D)) Aop 
+    = ctx_insert (CtxU (CtxU Γ (TyFun Bop D)) Aop) (2+i) A_s).
   { simpl. f_equal. f_equal. auto. }
-  assert (wf_vtype A_op) as wfa by (inv H0; auto).
-  assert (wf_vtype (TyFun B_op D)) as wfb by (inv H0; apply WfTyFun; auto).
-  specialize (v_shift_typesafe _ _ (TyFun B_op D) _ tyvs wfb) as tyvs'.
-  specialize (v_shift_typesafe _ _ A_op _ tyvs' wfa) as tyvs''.
+  assert (wf_vtype Aop) as wfa by (inv H0; auto).
+  assert (wf_vtype (TyFun Bop D)) as wfb by (inv H0; apply WfTyFun; auto).
+  specialize (v_shift_typesafe _ _ (TyFun Bop D) _ tyvs wfb) as tyvs'.
+  specialize (v_shift_typesafe _ _ Aop _ tyvs' wfa) as tyvs''.
   specialize (HC _ _ h _ _ i _ _ H3 tyvs geq) as IHh.
-  specialize (CI _ _ c_op _ (2+i) _ _ H4 tyvs'' H5) as IHc.
+  specialize (CI _ _ cop _ (2+i) _ _ H4 tyvs'' H5) as IHc.
   clear V CI HC R VE CE HE WF.
-  apply TypeH; auto; unfold h_subs; simpl. eapply TypeCasesU.
-  - apply negshift_get_case_None. apply sub_get_case_None. assumption.
-  - auto. 
+  apply TypeH; auto; unfold h_subs; simpl.
+  eapply TypeCasesU; auto.
+  - apply negshift_get_case_None. apply sub_get_case_None. auto.
   - rewrite v_shift_shift in IHc. rewrite v_shift_comm. apply IHc. 
     simpl. omega. omega.
 }{
@@ -1358,7 +1508,8 @@ destruct orig. destruct H3.
     (i + tctx_len Z + ctx_len Γ0) 
     (v_shift v_s (tctx_len Z+ctx_len Γ0) 0) A_s H4) as IHc.
   all: clear V CI HC R VE CE HE WF.
-  apply Respects; auto; unfold h_subs; simpl. apply RespectEqsU. auto.
+  apply Respects; auto; unfold h_subs; simpl.
+  apply RespectEqsU. auto.
   erewrite handle_t_negshift, handle_t_sub, v_shift_comm.
   erewrite handle_t_negshift, handle_t_sub, (v_shift_comm 1 i).
   assert (tctx_len Z+ctx_len Γ0+i=i+tctx_len Z+ctx_len Γ0) as s by omega.
@@ -1381,76 +1532,94 @@ intros tyvs geq len. apply Veq.
 { inv orig; eauto. }
 destruct orig. destruct H1.
 + specialize (VE _ _ _ _ _ i _ _ H1 tyvs) as IH.
-  clear V CI HC R VE CE HE WF. apply VeqSym. apply IH; auto.
+  clear V CI HC R VE CE HE WF.
+  apply VeqSym. apply IH; auto.
 + specialize (VE _ _ _ _ _ i _ _ H1 tyvs) as IH1.
   specialize (VE _ _ _ _ _ i _ _ H2 tyvs) as IH2.
-  clear V CI HC R VE CE HE WF. eapply VeqTrans; eauto.
+  clear V CI HC R VE CE HE WF.
+  eapply VeqTrans; eauto.
 + clear V CI HC R VE CE HE WF. subst. unfold v_subs. simpl.
   rename i0 into j. destruct (j =? i) eqn:cmp. 
   - rewrite v_negshift_shift, v_shift_0. 
     apply veq_refl in tyvs. inv H0. apply Nat.eqb_eq in cmp. subst. 
     erewrite get_ctx_insert_new in H1. inv H1.
-    eapply veq_subtype in tyvs; eauto. inv tyvs. all: omega || auto.
-  - simpl. destruct (i<=?j) eqn:ilj; eapply VeqVar; omega || eauto.
+    eapply veq_subtype in tyvs; eauto. inv tyvs. all: eaomega.
+  - simpl. destruct (i<=?j) eqn:ilj;
+    eapply VeqVar; eaomega.
     * apply Nat.eqb_neq in cmp. apply leb_complete in ilj.
       erewrite get_ctx_insert_changed.
       assert (1+(j-1)=j) by omega. rewrite H3. eauto. omega. 
     * apply Nat.eqb_neq in cmp. apply leb_complete_conv in ilj.
-      erewrite get_ctx_insert_unchanged. eauto. omega.
-+ clear V CI HC R VE CE HE WF. simpl. apply VeqUnit.
-+ clear V CI HC R VE CE HE WF. simpl. apply VeqInt.
+      erewrite get_ctx_insert_unchanged; eaomega.
++ clear V CI HC R VE CE HE WF. simpl.
+  apply VeqUnit.
++ clear V CI HC R VE CE HE WF. simpl.
+  apply VeqInt.
 + specialize (VE _ _ _ _ _ i _ _ H1 tyvs) as IH1.
   specialize (VE _ _ _ _ _ i _ _ H2 tyvs) as IH2.
-  clear V CI HC R VE CE HE WF. unfold v_subs. simpl. apply VeqPair; auto.
+  clear V CI HC R VE CE HE WF.
+  unfold v_subs. simpl. apply VeqPair; auto.
 + specialize (VE _ _ _ _ _ i _ _ H1 tyvs) as IH.
-  clear V CI HC R VE CE HE WF. unfold v_subs. simpl. eapply VeqInl; eauto.
+  clear V CI HC R VE CE HE WF.
+  unfold v_subs. simpl. eapply VeqInl; eauto.
 + specialize (VE _ _ _ _ _ i _ _ H1 tyvs) as IH.
-  clear V CI HC R VE CE HE WF. unfold v_subs. simpl. eapply VeqInr; eauto.
-+ clear V CI HC R VE CE HE WF. unfold v_subs. simpl. apply VeqListNil; auto.
+  clear V CI HC R VE CE HE WF.
+  unfold v_subs. simpl. eapply VeqInr; eauto.
++ clear V CI HC R VE CE HE WF.
+unfold v_subs. simpl. apply VeqListNil; auto.
 + specialize (VE _ _ _ _ _ i _ _ H1 tyvs) as IH1.
   specialize (VE _ _ _ _ _ i _ _ H2 tyvs) as IH2.
-  clear V CI HC R VE CE HE WF. unfold v_subs. simpl. apply VeqListCons; auto.
+  clear V CI HC R VE CE HE WF.
+  unfold v_subs. simpl. apply VeqListCons; auto.
 + assert (wf_vtype A) as wfa by (inv H; inv H3; assumption).
   specialize (v_shift_typesafe _ _ A _ tyvs wfa) as tyvs'.
   specialize (CE _ _ _ _ _ (S i) _ _ H1 tyvs') as IH.
-  clear V CI HC R VE CE HE WF. unfold v_subs. simpl. eapply VeqFun.
-  rewrite v_shift_comm. apply IH. simpl. f_equal. assumption.
+  clear V CI HC R VE CE HE WF.
+  unfold v_subs. simpl. eapply VeqFun.
+  rewrite v_shift_comm. apply IH. simpl. f_equal. auto.
   all: simpl; omega.
-+ assert (wf_vtype A) as wfa by (inv H; inv H5; inv H8; assumption).
++ assert (wf_vtype A) as wfa by (inv H; inv H5; inv H8; auto).
   specialize (v_shift_typesafe _ _ A _ tyvs wfa) as tyvs'.
   specialize (CE _ _ _ _ _ (S i) _ _ H1 tyvs') as IHc.
   specialize (HE _ _ _ _ _ _ i _ _ H2 tyvs) as IHh.
-  clear V CI HC R VE CE HE WF. unfold v_subs. simpl. eapply VeqHandler; eauto.
-  rewrite v_shift_comm. apply IHc. simpl. f_equal. assumption.
+  clear V CI HC R VE CE HE WF.
+  unfold v_subs. simpl. eapply VeqHandler; eauto.
+  rewrite v_shift_comm. apply IHc. simpl. f_equal. auto.
   all: simpl; omega.
-+ clear V CI HC R VE CE HE WF. unfold v_subs. simpl. apply ηUnit.
-+ clear V CI HC R VE CE HE WF. unfold v_subs. simpl.
-  rewrite <-v_shift_sub, <-v_shift_negshift_comm. apply ηFun.
-  apply v_sub_makes_no_var. apply v_shift_makes_no_var. omega. omega. 
++ clear V CI HC R VE CE HE WF.
+  unfold v_subs. simpl. apply ηUnit.
++ clear V CI HC R VE CE HE WF.
+  unfold v_subs. simpl.
+  rewrite <-v_shift_sub, <-v_shift_negshift_comm; aomega. apply ηFun.
+  apply v_sub_makes_no_var. apply v_shift_makes_no_var. 
 }{
 intros tyvs geq len. apply Ceq.
 { inv orig; eauto. }
 { inv orig; eauto. }
 destruct orig. destruct H1.
 + specialize (CE _ _ _ _ _ i _ _ H1 tyvs) as IH.
-  clear V CI HC R VE CE HE WF. apply CeqSym. eauto.
+  clear V CI HC R VE CE HE WF.
+  apply CeqSym. eauto.
 + specialize (CE _ _ _ _ _ i _ _ H1 tyvs) as IH1.
   specialize (CE _ _ _ _ _ i _ _ H2 tyvs) as IH2.
-  clear V CI HC R VE CE HE WF. eapply CeqTrans; eauto.
+  clear V CI HC R VE CE HE WF.
+  eapply CeqTrans; eauto.
 + specialize (VE _ _ _ _ _ i _ _ H1 tyvs) as IH.
-  clear V CI HC R VE CE HE WF. simpl. apply CeqRet. auto.
+  clear V CI HC R VE CE HE WF.
+  simpl. apply CeqRet. auto.
 + specialize (VE _ _ _ _ _ i _ _ H1 tyvs) as IH.
-  clear V CI HC R VE CE HE WF. simpl. apply CeqAbsurd. auto.
+  clear V CI HC R VE CE HE WF.
+  simpl. apply CeqAbsurd. auto.
 + specialize (VE _ _ _ _ _ i _ _ H1 tyvs) as IHv.
   assert (wf_vtype A) as wfa by (inv H1; inv H4; inv H6; auto).
   assert (wf_vtype B) as wfb by (inv H1; inv H4; inv H6; auto).
   specialize (v_shift_typesafe _ _ A _ tyvs wfa) as tyvs'.
   specialize (v_shift_typesafe _ _ B _ tyvs' wfb) as tyvs''.
   specialize (CE _ _ _ _ _ (2+i) _ _ H2 tyvs'') as IHc.
-  clear V CI HC R VE CE HE WF. unfold c_subs. simpl. eapply CeqΠMatch. auto.
-  rewrite v_shift_comm, <-(v_shift_shift 1 1). apply IHc.
-  simpl. do 2 f_equal. assumption.
-  simpl. omega. omega.
+  clear V CI HC R VE CE HE WF.
+  unfold c_subs. simpl. eapply CeqΠMatch. auto.
+  rewrite v_shift_comm, <-(v_shift_shift 1 1); aomega.
+  apply IHc. simpl. do 2 f_equal. assumption. simpl. omega.
 + specialize (VE _ _ _ _ _ i _ _ H1 tyvs) as IHv.
   assert (wf_vtype A) as wfa by (inv H1; inv H5; inv H7; auto).
   assert (wf_vtype B) as wfb by (inv H1; inv H5; inv H7; auto).
@@ -1458,9 +1627,10 @@ destruct orig. destruct H1.
   specialize (v_shift_typesafe _ _ B _ tyvs wfb) as tyvsb.
   specialize (CE _ _ _ _ _ (S i) _ _ H2 tyvsa) as IHc1.
   specialize (CE _ _ _ _ _ (S i) _ _ H3 tyvsb) as IHc2.
-  clear V CI HC R VE CE HE WF. unfold c_subs. simpl. eapply CeqΣMatch. auto.
+  clear V CI HC R VE CE HE WF.
+  unfold c_subs. simpl. eapply CeqΣMatch. auto.
   all: rewrite v_shift_comm; omega || apply IHc1 || apply IHc2.
-  all: simpl; try omega; f_equal; assumption.
+  all: simpl; aomega; f_equal; auto.
 + specialize (VE _ _ _ _ _ i _ _ H1 tyvs) as IHv.
   assert (wf_vtype A) as wfa by (inv H1; inv H4; inv H7; auto).
   assert (wf_vtype (TyList A)) as wfla by (inv H1; inv H4; auto).
@@ -1468,22 +1638,26 @@ destruct orig. destruct H1.
   specialize (v_shift_typesafe _ _ (TyList A) _ tyvs' wfla) as tyvs''.
   specialize (CE _ _ _ _ _ i _ _ H2 tyvs) as IHc1.
   specialize (CE _ _ _ _ _ (2+i) _ _ H3 tyvs'') as IHc2.
-  clear V CI HC R VE CE HE WF. unfold c_subs. simpl. eapply CeqListMatch; eauto.
+  clear V CI HC R VE CE HE WF.
+  unfold c_subs. simpl. eapply CeqListMatch; eauto.
   rewrite v_shift_comm, <-(v_shift_shift 1 1). apply IHc2.
   simpl. do 2 f_equal. assumption. simpl. omega. omega.
 + assert (wf_vtype B) as wfb by (inv H1; inv H4; inv H6; auto).
   specialize (v_shift_typesafe _ _ B _ tyvs wfb) as tyvsb.
   specialize (CE _ _ _ _ _ i _ _ H1 tyvs) as IHc1.
   specialize (CE _ _ _ _ _ (S i) _ _ H2 tyvsb) as IHc2.
-  clear V CI HC R VE CE HE WF. unfold c_subs. simpl. eapply CeqDoBind. eauto.
+  clear V CI HC R VE CE HE WF.
+  unfold c_subs. simpl. eapply CeqDoBind. eauto.
   rewrite v_shift_comm. apply IHc2. simpl.  f_equal. assumption.
   simpl. omega. omega.
 + specialize (VE _ _ _ _ _ i _ _ H1 tyvs) as IHv1.
   specialize (VE _ _ _ _ _ i _ _ H2 tyvs) as IHv2.
-  clear V CI HC R VE CE HE WF. simpl. eapply CeqApp; eauto.
+  clear V CI HC R VE CE HE WF.
+  simpl. eapply CeqApp; eauto.
 + specialize (VE _ _ _ _ _ i _ _ H1 tyvs) as IHv.
   specialize (CE _ _ _ _ _ i _ _ H2 tyvs) as IHc.
-  clear V CI HC R VE CE HE WF. simpl. eapply CeqHandle; eauto.
+  clear V CI HC R VE CE HE WF.
+  simpl. eapply CeqHandle; eauto.
 + assert (wf_vtype A) as wfa by (inv H2; inv H3; inv H2; inv H10; auto).
   assert (wf_vtype (TyFun A C)) as wff by (inv H2; inv H3; inv H2; auto).
   specialize (v_shift_typesafe _ _ A _ tyvs wfa) as tyvs'.
@@ -1491,50 +1665,57 @@ destruct orig. destruct H1.
   specialize (v_shift_typesafe _ _ (TyFun A C) _ tyvs wff) as tyvs'''.
   specialize (CE _ _ _ _ _ (2+i) _ _ H1 tyvs'') as IHc1.
   specialize (CE _ _ _ _ _ (1+i) _ _ H2 tyvs''') as IHc2.
-  clear V CI HC R VE CE HE WF. unfold c_subs. simpl. eapply CeqLetRec.
-  all: rewrite v_shift_comm; omega || auto.
+  clear V CI HC R VE CE HE WF.
+  unfold c_subs. simpl. eapply CeqLetRec.
+  all: rewrite v_shift_comm; eaomega.
   - rewrite <-(v_shift_shift 1 1). eapply IHc1. simpl. do 2 f_equal. auto.
     simpl. omega.
   - apply IHc2. simpl. f_equal. auto. simpl. omega.
-+ assert (wf_vtype B_op) as wfb by (inv H3; inv H4; inv H3; auto).
-  specialize (v_shift_typesafe _ _ B_op _ tyvs wfb) as tyvsb.
++ assert (wf_vtype Bop) as wfb by (inv H3; inv H4; inv H3; auto).
+  specialize (v_shift_typesafe _ _ Bop _ tyvs wfb) as tyvsb.
   specialize (VE _ _ _ _ _ i _ _ H2 tyvs) as IHv.
   specialize (CE _ _ _ _ _ (S i) _ _ H3 tyvsb) as IHc.
-  clear V CI HC R VE CE HE WF. unfold c_subs. simpl. eapply CeqOp; eauto.
+  clear V CI HC R VE CE HE WF.
+  unfold c_subs. simpl. eapply CeqOp; eauto.
   rewrite v_shift_comm. apply IHc. simpl. f_equal. auto. simpl. omega. omega.
 + specialize (WF _ _ _ _ i _ _ H2 tyvs) as IHwf.
-  clear V CI HC R VE CE HE WF. eapply OOTB; eauto.
+  clear V CI HC R VE CE HE WF.
+  eapply OOTB; eauto.
   rewrite <-c_subs_inst. rewrite H3. simpl. auto.
   rewrite <-c_subs_inst. rewrite H4. simpl. auto.
-+ clear V CI HC R VE CE HE WF. specialize βΠMatch as rule.
++ clear V CI HC R VE CE HE WF.
+  specialize βΠMatch as rule.
   unfold c_subs2_out in *. unfold c_subs_out in *. simpl.
   rewrite c_subs_subs, (c_subs_subs _ 0). simpl.
   assert (c_subs (ΠMatch (Pair v1 v2) c) i v_s 
     = ΠMatch (Pair (v_subs v1 i v_s) (v_subs v2 i v_s)) 
         (c_subs c (2+i) (v_shift v_s 2 0))).
   { unfold c_subs. unfold v_subs. simpl. f_equal. f_equal. 
-    rewrite v_shift_comm. reflexivity. omega. }  
+    rewrite v_shift_comm; aomega. }  
   rewrite H1. rewrite v_shift_shift, <-v_shift_subs_alt.
   apply rule. all: omega.
-+ clear V CI HC R VE CE HE WF. specialize βΣMatch_Inl as rule.
++ clear V CI HC R VE CE HE WF.
+  specialize βΣMatch_Inl as rule.
   unfold c_subs_out in *. simpl. rewrite c_subs_subs. simpl.
   assert (c_subs (ΣMatch (Inl v) c1 c2) i v_s
     = ΣMatch (Inl (v_subs v i v_s)) 
         (c_subs c1 (1+i) (v_shift v_s 1 0))
         (c_subs c2 (1+i) (v_shift v_s 1 0))).
   { unfold c_subs. unfold v_subs. simpl. f_equal; f_equal; 
-    rewrite v_shift_comm; reflexivity || omega. }  
+    rewrite v_shift_comm; aomega. }  
   rewrite H1. apply rule. all: omega.
-+ clear V CI HC R VE CE HE WF. specialize βΣMatch_Inr as rule.
++ clear V CI HC R VE CE HE WF.
+  specialize βΣMatch_Inr as rule.
   unfold c_subs_out in *. simpl. rewrite c_subs_subs. simpl.
   assert (c_subs (ΣMatch (Inr v) c1 c2) i v_s
     = ΣMatch (Inr (v_subs v i v_s)) 
         (c_subs c1 (1+i) (v_shift v_s 1 0))
         (c_subs c2 (1+i) (v_shift v_s 1 0))).
   { unfold c_subs. unfold v_subs. simpl. f_equal; f_equal; 
-    rewrite v_shift_comm; reflexivity || omega. }  
+    rewrite v_shift_comm; aomega. }  
   rewrite H1. apply rule. all: omega.
-+ clear V CI HC R VE CE HE WF. specialize βListMatch_Nil as rule.
++ clear V CI HC R VE CE HE WF.
+  specialize βListMatch_Nil as rule.
   unfold c_subs_out in *. simpl.
   assert (c_subs (ListMatch ListNil c1 c2) i v_s 
     = ListMatch ListNil 
@@ -1543,7 +1724,8 @@ destruct orig. destruct H1.
   { unfold c_subs. unfold v_subs. simpl. f_equal; f_equal; 
     rewrite v_shift_comm; reflexivity || omega. }  
   rewrite H1. apply rule. all: omega.
-+ clear V CI HC R VE CE HE WF. specialize βListMatch_Cons as rule.
++ clear V CI HC R VE CE HE WF.
+  specialize βListMatch_Cons as rule.
   unfold c_subs2_out in *. unfold c_subs_out in *. simpl.
   rewrite c_subs_subs, (c_subs_subs _ 0). simpl.
   assert (c_subs (ListMatch (ListCons v vs) c1 c2) i v_s
@@ -1554,14 +1736,16 @@ destruct orig. destruct H1.
     rewrite v_shift_comm; reflexivity || omega. }  
   rewrite H1. rewrite v_shift_shift, <-v_shift_subs_alt.
   apply rule. all: omega.
-+ clear V CI HC R VE CE HE WF. specialize βApp as rule.
++ clear V CI HC R VE CE HE WF.
+  specialize βApp as rule.
   unfold c_subs_out in *. simpl. rewrite c_subs_subs. simpl.
   assert (c_subs (App (Fun c) v) i v_s 
     = App (Fun (c_subs c (1+i) (v_shift v_s 1 0))) (v_subs v i v_s)).
   { unfold c_subs. unfold v_subs. simpl. f_equal. f_equal. 
     rewrite v_shift_comm; reflexivity || omega. }  
   rewrite H1. apply rule. all: omega.
-+ clear V CI HC R VE CE HE WF. specialize βLetRec as rule.
++ clear V CI HC R VE CE HE WF.
+  specialize βLetRec as rule.
   unfold c_subs_out in *. simpl. rewrite c_subs_subs. simpl.
   assert (c_subs (LetRec c1 c2) i v_s
     = LetRec (c_subs c1 (2+i) (v_shift v_s 2 0))
@@ -1574,43 +1758,45 @@ destruct orig. destruct H1.
        (c_subs c1 (2+i) (v_shift v_s 2 0))) ).
   { unfold c_subs. unfold v_subs. simpl. do 2 f_equal.
     rewrite v_shift_comm, <-c_shift_sub, c_shift_negshift_comm.
-    do 2 f_equal. rewrite v_shift_comm. auto. omega.
-    apply c_sub_makes_no_var. apply v_shift_makes_no_var. all: try omega.
-    do 3 f_equal. rewrite v_shift_shift, v_shift_comm; auto || omega. }
+    do 2 f_equal. rewrite v_shift_comm. all: aomega.
+    apply c_sub_makes_no_var. apply v_shift_makes_no_var.
+    do 3 f_equal. rewrite v_shift_shift, v_shift_comm; aomega. }
   rewrite H1. clear H1. apply rule. omega.  
-+ clear V CI HC R VE CE HE WF. specialize βDoBind_Ret as rule.
++ clear V CI HC R VE CE HE WF.
+  specialize βDoBind_Ret as rule.
   unfold c_subs_out in *. simpl. rewrite c_subs_subs. simpl.
   assert (c_subs (DoBind (Ret v) c) i v_s 
     = DoBind (Ret (v_subs v i v_s)) (c_subs c (1+i) (v_shift v_s 1 0))).
   { unfold c_subs. unfold v_subs. simpl. f_equal. f_equal. 
-    rewrite v_shift_comm; reflexivity || omega. }  
+    rewrite v_shift_comm; aomega. }  
   rewrite H1. apply rule. all: omega.
-+ clear V CI HC R VE CE HE WF. specialize βDoBind_Op as rule.
++ clear V CI HC R VE CE HE WF.
+  specialize βDoBind_Op as rule.
   unfold c_subs_out in *. unfold c_subs. simpl. rewrite v_shift_comm. 
   specialize (rule op 
     (v_negshift (v_sub v (i, v_shift v_s 1 i)) 1 i)
     (c_negshift
-      (c_sub c1 (S i, v_shift (v_shift v_s 1 0) 1 (1 + i)))
-      1 (S i))
+      (c_sub c1 (S i, v_shift (v_shift v_s 1 0) 1 (1 + i))) 1 (S i))
     (c_negshift
-      (c_sub c2 (S i, v_shift (v_shift v_s 1 0) 1 (1 + i))) 1
-      (S i))).
+      (c_sub c2 (S i, v_shift (v_shift v_s 1 0) 1 (1 + i))) 1 (S i))).
   rewrite c_shift_negshift_comm, c_shift_sub in rule. simpl.
   assert (v_shift (v_shift (v_shift v_s 1 0) 1 (S i)) 1 0
     = v_shift (v_shift (v_shift v_s 1 0) 1 (S i)) 1 1).
-  { rewrite <-v_shift_comm, v_shift_comm. all: omega || auto. }
-  rewrite H1. apply rule. all: try omega. clear rule.
+  { rewrite <-v_shift_comm, v_shift_comm. all: aomega. }
+  rewrite H1. apply rule. all: aomega. clear rule.
   apply c_sub_makes_no_var. apply v_shift_makes_no_var.
-+ clear V CI HC R VE CE HE WF. specialize βHandle_Ret as rule.
++ clear V CI HC R VE CE HE WF.
+  specialize βHandle_Ret as rule.
   unfold c_subs_out in *. simpl. rewrite c_subs_subs. simpl.
   assert (c_subs (Handle (Handler c_r h) (Ret v)) i v_s
     = Handle (Handler 
       (c_subs c_r (1+i) (v_shift v_s 1 0)) (h_subs h i v_s)) 
       (Ret (v_subs v i v_s) ) ).
   { unfold c_subs. unfold v_subs. simpl. f_equal. f_equal. 
-    rewrite v_shift_comm; reflexivity || omega. }  
+    rewrite v_shift_comm; aomega. }  
   rewrite H1. apply rule. all: omega.
-+ clear V CI HC R VE CE HE WF. specialize βHandle_Op as rule.
++ clear V CI HC R VE CE HE WF.
+  specialize βHandle_Op as rule.
   unfold c_subs2_out in *. unfold c_subs_out in *. simpl.
   rewrite c_subs_subs, (c_subs_subs _ 0). simpl.
   assert (c_subs (Handle (Handler c_r h) (Op op v c_k)) i v_s =
@@ -1626,15 +1812,15 @@ destruct orig. destruct H1.
   { clear rule. unfold v_subs. unfold c_subs. unfold h_subs. 
     simpl. do 3 f_equal.
     rewrite c_shift_negshift_comm, c_shift_sub. do 3 f_equal.
-    rewrite v_shift_comm. f_equal. apply v_shift_comm. all: try omega.
+    rewrite v_shift_comm. f_equal. apply v_shift_comm. all: aomega.
     apply c_sub_makes_no_var. apply v_shift_makes_no_var.
-    rewrite h_shift_negshift_comm, h_shift_sub. f_equal. omega.
-    apply h_sub_makes_no_var. apply v_shift_makes_no_var. omega.
-    rewrite v_shift_comm. reflexivity. omega. }
+    rewrite h_shift_negshift_comm, h_shift_sub. all: aomega.
+    apply h_sub_makes_no_var. apply v_shift_makes_no_var.
+    rewrite v_shift_comm; aomega. }
   rewrite H2, v_shift_shift, <-v_shift_subs_alt. clear H2. simpl.
   eapply rule. unfold h_subs. 
   apply negshift_get_case_Some. rewrite <-(v_shift_comm 1 i 0). 
-  apply sub_get_case_Some. eauto. all: omega.
+  apply sub_get_case_Some. all:eaomega.
 + assert (wf_vtype (TyΠ A B)) as wfab.
   { inv H2. apply wf_ctx_insert_vtype in H3. auto. auto. }
   specialize (v_insert_typesafe _ _ _ tyvs (TyΠ A B) n wfab) as tyvsab.
@@ -1644,7 +1830,7 @@ destruct orig. destruct H1.
   clear V CI HC R VE CE HE WF. simpl.
   assert (forall c, c_subs (ΠMatch v c) i v_s 
     = ΠMatch (v_subs v i v_s) (c_subs c (2+i) (v_shift v_s 2 0))).
-  { intro c'. unfold c_subs. simpl. rewrite v_shift_comm. reflexivity. omega. }
+  { intro c'. unfold c_subs. simpl. rewrite v_shift_comm; aomega. }
   rewrite H3. clear H3.
   destruct (n<=?i) eqn:ni.
   - clear IHc.
@@ -1659,13 +1845,13 @@ destruct orig. destruct H1.
     assert (v_subs (Pair (Var 1) (Var 0)) (S(S i)) (v_shift v_s 2 0) 
       = (Pair (Var 1) (Var 0))).
     { unfold v_subs. simpl. reflexivity. }
-    rewrite H3. clear H3. eapply ηPair. all: omega || auto.
-    apply IHcp. subst. rewrite ctx_insert_comm. auto. omega. omega.
+    rewrite H3. clear H3. eapply ηPair. all: aomega.
+    apply IHcp. subst. rewrite ctx_insert_comm. all: aomega.
     rewrite ctx_len_insert; omega.
   - clear IHcp.
     apply leb_complete_conv in ni.
     destruct n. omega.
-    rewrite (c_subs_subs_alt _ n), (c_subs_subs_alt _ ). all: try omega. simpl.
+    rewrite (c_subs_subs_alt _ n), (c_subs_subs_alt _ ). all: aomega. simpl.
     specialize ηPair as rule.
     assert (v_subs (Pair (Var 1) (Var 0)) (S (S i)) (v_shift v_s 2 0)
       = (Pair (Var 1) (Var 0))).
@@ -1675,11 +1861,11 @@ destruct orig. destruct H1.
     rewrite samen, <-v_shift_comm.
     rewrite <-(v_shift_shift 1 1), <-(c_shift_shift 1 1).
     rewrite <-c_shift_subs_alt, <-c_shift_subs_alt, c_shift_shift.
-    eapply ηPair. all: omega || auto.
+    eapply ηPair. all: aomega.
     subst. rewrite ctx_len_insert in H1. omega. omega.
     assert (S n - 1 = n) as n0 by omega. rewrite n0 in *.
-    apply IHc. subst. rewrite ctx_insert_comm; omega || auto.
-    specialize (ctx_len_insert_trivial Γ (TyΠ A B) n) as triv. omega.
+    apply IHc. subst. rewrite ctx_insert_comm; aomega.
+    specialize (ctx_len_insert_trivial Γ n (TyΠ A B)) as triv. omega.
 + assert (wf_vtype (TyΣ A B)) as wfab.
   { inv H2. apply wf_ctx_insert_vtype in H3. auto. auto. }
   specialize (v_insert_typesafe _ _ _ tyvs (TyΣ A B) n wfab) as tyvsab.
@@ -1691,7 +1877,7 @@ destruct orig. destruct H1.
     = ΣMatch (v_subs v i v_s) 
         (c_subs c1 (1+i) (v_shift v_s 1 0))
         (c_subs c2 (1+i) (v_shift v_s 1 0))).
-  { intro c'. unfold c_subs. simpl. rewrite v_shift_comm. reflexivity. omega. }
+  { intro c'. unfold c_subs. simpl. rewrite v_shift_comm; aomega. }
   rewrite H3. clear H3.
   destruct (n<=?i) eqn:ni.
   - apply leb_complete in ni.
@@ -1699,17 +1885,17 @@ destruct orig. destruct H1.
     simpl. all: try omega.
     rewrite <-v_shift_comm, <-c_shift_subs_alt. all: try omega.
     eapply ηSum. omega. apply IHcp. 
-    subst. rewrite ctx_insert_comm; omega || auto.
+    subst. rewrite ctx_insert_comm; aomega.
     rewrite ctx_len_insert; omega.
   - apply leb_complete_conv in ni.
     rewrite (c_subs_subs_alt _ n), (c_subs_subs_alt _ n).
-    destruct n. all: try omega.
+    destruct n. all: aomega.
     rewrite (c_subs_subs_alt _ n). simpl.
-    rewrite <-v_shift_comm, <-c_shift_subs_alt. all: try omega.
+    rewrite <-v_shift_comm, <-c_shift_subs_alt. all: aomega.
     eapply ηSum. subst. rewrite ctx_len_insert in H1. omega. omega.
     assert (S n - 1 = n) as n0 by omega. rewrite n0 in *.
-    apply IHc. subst. rewrite ctx_insert_comm; omega || auto.
-    specialize (ctx_len_insert_trivial Γ (TyΣ A B) n) as triv. omega.
+    apply IHc. subst. rewrite ctx_insert_comm; aomega.
+    specialize (ctx_len_insert_trivial Γ n (TyΣ A B)) as triv. omega.
 + clear V CI HC R VE CE HE WF. simpl. apply ηDoBind.
 }{
 intros tyvs geq len.
@@ -1726,16 +1912,19 @@ destruct orig. destruct H4.
   specialize (v_shift_typesafe _ _ A _ tyvs' wfa) as tyvs''.
   specialize (CE _ _ _ _ _ (2+i) _ _ H6 tyvs'') as IH1.
   specialize (HE _ _ _ _ _ _ i _ _ H7 tyvs) as IH2.
-  clear V CI HC R VE CE HE WF. eapply Heq.
-  2: exact H0. all: eauto. eapply HeqSigU.
-  - unfold h_subs. eapply negshift_get_case_Some. eapply sub_get_case_Some. eauto.
-  - unfold h_subs. eapply negshift_get_case_Some. eapply sub_get_case_Some. eauto.
+  clear V CI HC R VE CE HE WF.
+  eapply Heq. 2: exact H0. all: eauto.
+  eapply HeqSigU; eauto.
+  - unfold h_subs. eapply negshift_get_case_Some.
+    eapply sub_get_case_Some. eauto.
+  - unfold h_subs. eapply negshift_get_case_Some.
+    eapply sub_get_case_Some. eauto.
   - rewrite v_shift_comm, <-(v_shift_shift 1 1). apply IH1.
-    simpl. do 2 f_equal. assumption. simpl. omega. omega.
-  - eauto.
+    simpl. do 2 f_equal. all: simpl; aomega.
 }{
 intros tyvs geq len. destruct orig.
-+ clear V CI HC R VE CE HE WF. simpl. apply WfInstØ. inv tyvs. auto.
++ clear V CI HC R VE CE HE WF.
+  simpl. apply WfInstØ. inv tyvs. auto.
 + specialize (V _ _ _ _ i _ _ H tyvs geq) as IHv.
   specialize (WF _ _ _ _ i _ _ orig tyvs geq) as IHwf.
   clear V CI HC R VE CE HE WF. simpl.
@@ -1743,6 +1932,8 @@ intros tyvs geq len. destruct orig.
 }
 Qed.
 
+
+(*
 (* ==================== Handling templates ==================== *)
 
 Fixpoint cop_insert_ctx Γ' Γ A B D c {struct Γ}:
@@ -2139,37 +2330,37 @@ destruct v; unfold v_subs in *; unfold c_subs in *; simpl; auto.
     rewrite inst_insert_same. simpl.
     assert (k=?k=true) as same by (apply Nat.eqb_eq; auto). rewrite same.
     rewrite v_negshift_shift, v_negshift_shift, v_shift_0, v_shift_0.
-    all: omega || auto. rewrite inst_len_shift. omega.
+    all: aomega. rewrite inst_len_shift. omega.
   - apply Nat.eqb_neq in dbin. apply leb_complete in cmp.
     destruct dbi. omega.
     rewrite inst_insert_above. simpl.
     assert (dbi-0=dbi) as same by omega. rewrite same, get_inst_val_shift. 
     destruct (get_inst_val I dbi) eqn:gets; simpl.
     rewrite v_sub_no_var_same, v_negshift_shift, v_shift_0.
-    all: omega || auto.
+    all: aomega.
     apply v_shift_makes_no_var. rewrite inst_len_shift. auto.
   - apply Nat.eqb_neq in dbin. apply leb_complete_conv in cmp.
     rewrite inst_insert_under. simpl.
     rewrite get_inst_val_shift.
     destruct (get_inst_val I dbi) eqn:gets; simpl.
     rewrite v_sub_no_var_same, v_negshift_shift, v_shift_0.
-    all: omega || auto.
+    all: aomega.
     apply v_shift_makes_no_var. rewrite inst_len_shift. auto. }
 all: f_equal; simpl in *; try destruct undv; eauto.
 all: rewrite inst_shift_insert, inst_shift_comm, v_shift_comm; try omega; simpl.
 all: erewrite (c_inst_subs (S k)); simpl.
-all: try rewrite inst_len_shift; omega || auto.
+all: try rewrite inst_len_shift; aomega.
 + do 3 f_equal. do 2 f_equal. omega. rewrite v_shift_inst, v_shift_comm.
   simpl. rewrite instU_is_insert, v_inst_no_var_same.
   rewrite v_negshift_shift, v_shift_0, v_shift_inst, v_shift_inst. 
-  all: omega || auto. apply v_shift_makes_no_var.
+  all: aomega. apply v_shift_makes_no_var.
   apply v_under_var_shift; try omega.
   rewrite inst_len_shift, inst_len_shift. auto.
 + apply v_under_var_shift; try omega. auto.
 + do 3 f_equal. do 2 f_equal. omega. rewrite v_shift_inst, v_shift_comm.
   simpl. rewrite instU_is_insert, v_inst_no_var_same.
   rewrite v_negshift_shift, v_shift_0, v_shift_inst, v_shift_inst. 
-  all: omega || auto. apply v_shift_makes_no_var.
+  all: aomega. apply v_shift_makes_no_var.
   apply v_under_var_shift; try omega.
   rewrite inst_len_shift, inst_len_shift. auto.
 + apply v_under_var_shift; try omega. auto.
@@ -2184,103 +2375,103 @@ all: simpl in *; try destruct undv; try destruct H0; omega || eauto.
 
 all: assert (forall n, S(S n)=2+n) as ssn by (intros; omega).
 + rewrite (c_inst_subs (S(S k))). clear c_inst_subs. simpl. do 3 f_equal.
-  all: simpl; (try rewrite inst_len_shift); omega || auto.
+  all: simpl; (try rewrite inst_len_shift); aomega.
   - do 2 f_equal. rewrite inst_shift_insert. simpl. f_equal.
     rewrite (inst_shift_comm 1). f_equal. all: omega.
   - rewrite v_shift_comm. f_equal. rewrite v_shift_inst.
     rewrite instU_is_insert, v_inst_no_var_same. all: try omega.
     rewrite instU_is_insert, v_inst_no_var_same. all: try omega.
-    * rewrite v_negshift_shift, v_negshift_shift, v_shift_0; omega || auto.
+    * rewrite v_negshift_shift, v_negshift_shift, v_shift_0; aomega.
     * rewrite v_negshift_shift. apply v_shift_makes_no_var. omega.
     * rewrite v_negshift_shift. apply v_under_var_shift; simpl. 3: omega.
-      all: rewrite inst_len_shift; omega || auto.
+      all: rewrite inst_len_shift; aomega.
     * rewrite <-(v_shift_shift 1). apply v_shift_makes_no_var.
     * rewrite <-(v_shift_shift 1). apply v_under_var_shift; simpl.
       apply v_under_var_shift; simpl.
-      all: rewrite inst_len_shift; omega || auto.
+      all: rewrite inst_len_shift; aomega.
   - rewrite (ssn (inst_len I)). apply v_under_var_shift. auto. omega.
 + rewrite (c_inst_subs (S k)). clear c_inst_subs. simpl. do 3 f_equal.
-  all: simpl; (try rewrite inst_len_shift); omega || auto.
+  all: simpl; (try rewrite inst_len_shift); aomega.
   - do 2 f_equal. rewrite inst_shift_insert. simpl. f_equal.
-    rewrite <-inst_shift_comm. all: omega || auto.
+    rewrite <-inst_shift_comm. all: aomega.
   - rewrite v_shift_comm. f_equal. rewrite v_shift_inst.
     rewrite instU_is_insert, v_inst_no_var_same. all: try omega.
-    * rewrite v_negshift_shift, v_shift_0; omega || auto.
+    * rewrite v_negshift_shift, v_shift_0; aomega.
     * apply v_shift_makes_no_var.
-    * apply v_under_var_shift; rewrite inst_len_shift; omega || auto.
-  - apply v_under_var_shift; omega || auto.
+    * apply v_under_var_shift; rewrite inst_len_shift; aomega.
+  - apply v_under_var_shift; aomega.
 + rewrite (c_inst_subs (S k)). clear c_inst_subs. simpl. do 3 f_equal.
-  all: simpl; (try rewrite inst_len_shift); omega || auto.
+  all: simpl; (try rewrite inst_len_shift); aomega.
   - do 2 f_equal. rewrite inst_shift_insert. simpl. f_equal.
-    rewrite <-inst_shift_comm. all: omega || auto.
+    rewrite <-inst_shift_comm. all: aomega.
   - rewrite v_shift_comm. f_equal. rewrite v_shift_inst.
     rewrite instU_is_insert, v_inst_no_var_same. all: try omega.
-    * rewrite v_negshift_shift, v_shift_0; omega || auto.
+    * rewrite v_negshift_shift, v_shift_0; aomega.
     * apply v_shift_makes_no_var.
-    * apply v_under_var_shift; rewrite inst_len_shift; omega || auto.
-  - apply v_under_var_shift; omega || auto.
+    * apply v_under_var_shift; rewrite inst_len_shift; aomega.
+  - apply v_under_var_shift; aomega.
 + rewrite (c_inst_subs (S(S k))). clear c_inst_subs. simpl. do 3 f_equal.
-  all: simpl; (try rewrite inst_len_shift); omega || auto.
+  all: simpl; (try rewrite inst_len_shift); aomega.
   - do 2 f_equal. rewrite inst_shift_insert. simpl. f_equal.
     rewrite (inst_shift_comm 1). f_equal. all: omega.
   - rewrite v_shift_comm. f_equal. rewrite v_shift_inst.
     rewrite instU_is_insert, v_inst_no_var_same. all: try omega.
     rewrite instU_is_insert, v_inst_no_var_same. all: try omega.
-    * rewrite v_negshift_shift, v_negshift_shift, v_shift_0; omega || auto.
+    * rewrite v_negshift_shift, v_negshift_shift, v_shift_0; aomega.
     * rewrite v_negshift_shift. apply v_shift_makes_no_var. omega.
     * rewrite v_negshift_shift. apply v_under_var_shift; simpl. 3: omega.
-      all: rewrite inst_len_shift; omega || auto.
+      all: rewrite inst_len_shift; aomega.
     * rewrite <-(v_shift_shift 1). apply v_shift_makes_no_var.
     * rewrite <-(v_shift_shift 1). apply v_under_var_shift; simpl.
       apply v_under_var_shift; simpl.
-      all: rewrite inst_len_shift; omega || auto.
+      all: rewrite inst_len_shift; aomega.
   - rewrite (ssn (inst_len I)). apply v_under_var_shift. auto. omega.
 + rewrite (c_inst_subs (S k)). clear c_inst_subs. simpl. do 3 f_equal.
-  all: simpl; (try rewrite inst_len_shift); omega || auto.
+  all: simpl; (try rewrite inst_len_shift); aomega.
   - do 2 f_equal. rewrite inst_shift_insert. simpl. f_equal.
-    rewrite <-inst_shift_comm. all: omega || auto.
+    rewrite <-inst_shift_comm. all: aomega.
   - rewrite v_shift_comm. f_equal. rewrite v_shift_inst.
     rewrite instU_is_insert, v_inst_no_var_same. all: try omega.
-    * rewrite v_negshift_shift, v_shift_0; omega || auto.
+    * rewrite v_negshift_shift, v_shift_0; aomega.
     * apply v_shift_makes_no_var.
-    * apply v_under_var_shift; rewrite inst_len_shift; omega || auto.
-  - apply v_under_var_shift; omega || auto.
+    * apply v_under_var_shift; rewrite inst_len_shift; aomega.
+  - apply v_under_var_shift; aomega.
 + rewrite (c_inst_subs (S(S k))). clear c_inst_subs. simpl. do 3 f_equal.
-  all: simpl; (try rewrite inst_len_shift); omega || auto.
+  all: simpl; (try rewrite inst_len_shift); aomega.
   - do 2 f_equal. rewrite inst_shift_insert. simpl. f_equal.
     rewrite (inst_shift_comm 1). f_equal. all: omega.
   - rewrite v_shift_comm. f_equal. rewrite v_shift_inst.
     rewrite instU_is_insert, v_inst_no_var_same. all: try omega.
     rewrite instU_is_insert, v_inst_no_var_same. all: try omega.
-    * rewrite v_negshift_shift, v_negshift_shift, v_shift_0; omega || auto.
+    * rewrite v_negshift_shift, v_negshift_shift, v_shift_0; aomega.
     * rewrite v_negshift_shift. apply v_shift_makes_no_var. omega.
     * rewrite v_negshift_shift. apply v_under_var_shift; simpl. 3: omega.
-      all: rewrite inst_len_shift; omega || auto.
+      all: rewrite inst_len_shift; aomega.
     * rewrite <-(v_shift_shift 1). apply v_shift_makes_no_var.
     * rewrite <-(v_shift_shift 1). apply v_under_var_shift; simpl.
       apply v_under_var_shift; simpl.
-      all: rewrite inst_len_shift; omega || auto.
+      all: rewrite inst_len_shift; aomega.
   - rewrite (ssn (inst_len I)). apply v_under_var_shift. auto. omega.
 + rewrite (c_inst_subs (S k)). clear c_inst_subs. simpl. do 3 f_equal.
-  all: simpl; (try rewrite inst_len_shift); omega || auto.
+  all: simpl; (try rewrite inst_len_shift); aomega.
   - do 2 f_equal. rewrite inst_shift_insert. simpl. f_equal.
-    rewrite <-inst_shift_comm. all: omega || auto.
+    rewrite <-inst_shift_comm. all: aomega.
   - rewrite v_shift_comm. f_equal. rewrite v_shift_inst.
     rewrite instU_is_insert, v_inst_no_var_same. all: try omega.
-    * rewrite v_negshift_shift, v_shift_0; omega || auto.
+    * rewrite v_negshift_shift, v_shift_0; aomega.
     * apply v_shift_makes_no_var.
-    * apply v_under_var_shift; rewrite inst_len_shift; omega || auto.
-  - apply v_under_var_shift; omega || auto.
+    * apply v_under_var_shift; rewrite inst_len_shift; aomega.
+  - apply v_under_var_shift; aomega.
 + rewrite (c_inst_subs (S k)). clear c_inst_subs. simpl. do 3 f_equal.
-  all: simpl; (try rewrite inst_len_shift); omega || auto.
+  all: simpl; (try rewrite inst_len_shift); aomega.
   - do 2 f_equal. rewrite inst_shift_insert. simpl. f_equal.
-    rewrite <-inst_shift_comm. all: omega || auto.
+    rewrite <-inst_shift_comm. all: aomega.
   - rewrite v_shift_comm. f_equal. rewrite v_shift_inst.
     rewrite instU_is_insert, v_inst_no_var_same. all: try omega.
-    * rewrite v_negshift_shift, v_shift_0; omega || auto.
+    * rewrite v_negshift_shift, v_shift_0; aomega.
     * apply v_shift_makes_no_var.
-    * apply v_under_var_shift; rewrite inst_len_shift; omega || auto.
-  - apply v_under_var_shift; omega || auto.
+    * apply v_under_var_shift; rewrite inst_len_shift; aomega.
+  - apply v_under_var_shift; aomega.
 }{
 intros safe undv undvs. 
 destruct h; unfold h_subs in *; unfold c_subs in *; simpl; auto; f_equal.
@@ -2294,14 +2485,14 @@ all: clear c_inst_subs h_inst_subs.
   - rewrite v_shift_comm. f_equal. rewrite v_shift_inst.
     rewrite instU_is_insert, v_inst_no_var_same. all: try omega.
     rewrite instU_is_insert, v_inst_no_var_same. all: try omega.
-    * rewrite v_negshift_shift, v_negshift_shift, v_shift_0; omega || auto.
+    * rewrite v_negshift_shift, v_negshift_shift, v_shift_0; aomega.
     * rewrite v_negshift_shift. apply v_shift_makes_no_var. omega.
     * rewrite v_negshift_shift. apply v_under_var_shift; simpl. 3: omega.
-      all: rewrite inst_len_shift; omega || auto.
+      all: rewrite inst_len_shift; aomega.
     * rewrite <-(v_shift_shift 1). apply v_shift_makes_no_var.
     * rewrite <-(v_shift_shift 1). apply v_under_var_shift; simpl.
       apply v_under_var_shift; simpl.
-      all: rewrite inst_len_shift; omega || auto.
+      all: rewrite inst_len_shift; aomega.
 + assert (S(S(inst_len I)) = 2+(inst_len I)) as same by omega.
   rewrite same. apply v_under_var_shift. auto. omega.
 }
@@ -2318,7 +2509,7 @@ Proof.
 intros. unfold c_subs_out. unfold c_subs_out.
 rewrite (c_inst_subs 0). do 2 f_equal.
 rewrite instU_is_insert.
-all: simpl; omega || auto.
+all: simpl; aomega.
 Qed.
 
 
@@ -2334,7 +2525,7 @@ intros. unfold c_subs2_out.
 rewrite c_inst_subs_out, c_inst_subs_out. simpl.
 rewrite inst_shift_shift. f_equal. f_equal.
 rewrite instU_is_insert, v_inst_no_var_same, v_negshift_shift, v_shift_0.
-all: simpl; omega || auto.
+all: simpl; aomega.
 + apply v_shift_makes_no_var.
 + apply v_under_var_shift. rewrite inst_len_shift. auto. omega.
 + rewrite inst_len_shift. auto.
@@ -2364,7 +2555,7 @@ destruct I; simpl.
     specialize (ggaux (InstU I v0) n k v). simpl in ggaux.
     rewrite ggaux. rewrite get_inst_shift.
     destruct (get_inst_val (inst_extend_by_n (InstU I v0) k) v); simpl.
-    rewrite v_shift_shift, v_shift_shift. do 2 f_equal. all: omega || auto.
+    rewrite v_shift_shift, v_shift_shift. do 2 f_equal. all: aomega.
 Qed.
 
 Fixpoint gaux I k n v {struct k}:
@@ -2380,7 +2571,7 @@ destruct k; simpl.
 - destruct v. omega.
   rewrite get_inst_shift, get_inst_shift, ggaux.
   destruct (get_inst_val (inst_extend_by_n I k) v); simpl.
-  rewrite v_shift_shift, v_shift_shift. do 2 f_equal. all: omega || auto.
+  rewrite v_shift_shift, v_shift_shift. do 2 f_equal. all: aomega.
 Qed.
 
 Fixpoint vaux k n v I: 
@@ -2406,7 +2597,7 @@ destruct v; simpl; auto; try f_equal; auto.
     rewrite get_inst_extend_same.
     rewrite gaux. auto. apply leb_complete. auto.
   - apply leb_complete_conv in kv. rewrite get_inst_extend_var. 
-    simpl. rewrite get_inst_extend_var. all: omega || auto.
+    simpl. rewrite get_inst_extend_var. all: aomega.
 + specialize (caux (S k) n c I). simpl in caux. rewrite caux. auto.
 + specialize (caux (S k) n c I). simpl in caux. rewrite caux. auto.
 }{
@@ -2449,15 +2640,15 @@ all: assert (forall x y, x+(S y) = S (x+y)) as comm by (intros; omega).
 + erewrite v_inst_extend_same; eauto. omega.
 + erewrite v_inst_extend_same; eauto.
   eapply inst_handle_t in H5. simpl in H5. rewrite <-H5.
-  rewrite comm, comm. simpl. rewrite inst_shift_shift. all: omega || auto.
+  rewrite comm, comm. simpl. rewrite inst_shift_shift. all: aomega.
 + erewrite v_inst_extend_same; eauto.
   eapply inst_handle_t in H6. simpl in H6. rewrite <-H6.
   eapply inst_handle_t in H7. simpl in H7. rewrite <-H7.
-  rewrite comm. simpl. all: omega || auto.
+  rewrite comm. simpl. all: aomega.
 + erewrite v_inst_extend_same; eauto.
   eapply inst_handle_t in H6. simpl in H6. rewrite <-H6.
   eapply inst_handle_t in H7. simpl in H7. rewrite <-H7.
-  rewrite comm, comm. simpl. rewrite inst_shift_shift. all: omega || auto.
+  rewrite comm, comm. simpl. rewrite inst_shift_shift. all: aomega.
 + destruct (get_case h o) eqn: finds.
   - eapply find_inst_Some in finds as findss. rewrite findss. 2: reflexivity.
     rewrite c_inst_subs2_out. unfold c_subs2_out. unfold c_subs_out. simpl.
@@ -2477,7 +2668,7 @@ all: assert (forall x y, x+(S y) = S (x+y)) as comm by (intros; omega).
       rewrite <-caux. do 2 f_equal. omega.
     * erewrite v_inst_shift_extend; eauto. omega.
     * f_equal. eapply inst_handle_t in H7. simpl in H7. rewrite <-H7.
-      f_equal. rewrite comm. all: omega || auto.
+      f_equal. rewrite comm. all: aomega.
     * rewrite inst_len_extend_by_n. simpl.
       assert (S (S (inst_len I + (tctx_len Z + ctx_len Γ))) 
         = (ctx_len Γ + tctx_len Z) + (S (S (inst_len I)))) by omega.
@@ -2894,7 +3085,7 @@ destruct orig. destruct H2; simpl.
   apply Veq; auto. rewrite instU_is_insert.
   rewrite v_inst_no_var_same, v_negshift_shift, v_shift_0. 
   rewrite <-v_shift_inst. apply ηFun.
-  all: omega || auto.
+  all: aomega.
   apply v_shift_makes_no_var.
   apply v_under_var_shift. erewrite inst_len_shift, wf_inst_len_same.
   eapply has_vtype_is_under_ctx. all: omega || eauto.
@@ -3032,7 +3223,7 @@ destruct orig. destruct H2; simpl.
   unfold c_subs_out in rule. rewrite c_inst_subs_out.
   apply rule. all: try clear rule; try rewrite same_len.
   - apply has_ctype_is_under_ctx in tyc1. auto.
-  - apply shape_sum_inl in tyv. eapply has_vtype_is_under_ctx. eauto.
+  - apply shape_inl in tyv. eapply has_vtype_is_under_ctx. eauto.
 + eapply CL in H0 as tys1; eauto.
   eapply CL in H1 as tys2; eauto.
   clear VL CL HL RL VEL CEL HEL WS.
@@ -3047,7 +3238,7 @@ destruct orig. destruct H2; simpl.
   unfold c_subs_out in rule. rewrite c_inst_subs_out.
   apply rule. all: try clear rule; try rewrite same_len.
   - apply has_ctype_is_under_ctx in tyc2. auto.
-  - apply shape_sum_inr in tyv. eapply has_vtype_is_under_ctx. eauto.
+  - apply shape_inr in tyv. eapply has_vtype_is_under_ctx. eauto.
 + eapply CL in H0 as tys1; eauto.
   eapply CL in H1 as tys2; eauto.
   clear VL CL HL RL VEL CEL HEL WS.
@@ -3072,9 +3263,9 @@ destruct orig. destruct H2; simpl.
   rewrite c_inst_subs2_out. rewrite v_shift_inst in rule. 
   apply rule. all: try clear rule; try rewrite same_len.
   - apply has_ctype_is_under_ctx in tyc2. auto.
-  - apply shape_list_cons in tyv. destruct tyv.
+  - apply shape_cons in tyv. destruct tyv.
     eapply has_vtype_is_under_ctx. eauto.
-  - apply shape_list_cons in tyv. destruct tyv.
+  - apply shape_cons in tyv. destruct tyv.
     eapply has_vtype_is_under_ctx. eauto.
 + eapply CL in H0 as tys1; eauto.
   eapply CL in H1 as tys2; eauto.
@@ -3109,7 +3300,7 @@ destruct orig. destruct H2; simpl.
       (Var 1)) (Var 0)) 2 (Var 2)) as same.
   {simpl. destruct I; auto. }
   rewrite same, c_inst_no_var_same, c_negshift_shift, c_shift_0. apply rule.
-  all: simpl; omega || auto.
+  all: simpl; aomega.
   all: clear rule; try clear same.
   - apply c_shift_makes_no_var.
   - rewrite inst_len_shift, inst_len_shift, same_len. apply c_under_var_shift.
@@ -3152,7 +3343,7 @@ destruct orig. destruct H2; simpl.
      1 (Var 1)) as same.
   { simpl. destruct I; auto. }
   rewrite same, c_inst_no_var_same, c_negshift_shift, c_shift_0. apply rule.
-  all: simpl; omega || auto.
+  all: simpl; aomega.
   - apply c_shift_makes_no_var.
   - rewrite inst_len_shift, inst_len_shift, same_len.
     apply c_under_var_shift. apply has_ctype_is_under_ctx in tyc2.
@@ -3203,7 +3394,7 @@ destruct orig. destruct H2; simpl.
   rewrite c_negshift_shift, c_shift_0, h_negshift_shift, h_shift_0. simpl.
   rewrite inst_shift_comm. rewrite v_shift_inst, h_shift_inst in rule.
   apply rule. 
-  all: simpl; omega || auto; try clear rule; clear tys1 tys2.
+  all: simpl; aomega; try clear rule; clear tys1 tys2.
   all: try rewrite inst_len_shift; try rewrite inst_len_shift.
   all: try rewrite same_len.
   all: destruct C' as [A Σ E]; apply shape_handler in tyh;
@@ -3241,7 +3432,7 @@ destruct orig. destruct H2; simpl.
   { rewrite <-(c_shift_shift 1), instU_is_insert, c_inst_no_var_same.
     rewrite c_negshift_shift, c_shift_0, instU_is_insert, c_inst_no_var_same.
     rewrite c_negshift_shift, c_shift_0. do 2 f_equal.
-    rewrite (inst_shift_comm 1). all: omega || auto.
+    rewrite (inst_shift_comm 1). all: aomega.
     + apply c_shift_makes_no_var.
     + apply c_under_var_shift; omega || simpl.
       rewrite inst_len_insert, inst_len_shift, inst_len_shift, same_len.
@@ -3256,7 +3447,7 @@ destruct orig. destruct H2; simpl.
       all: try omega. rewrite inst_len_shift, inst_len_shift, same_len. omega.
   }
   rewrite H4. eapply rule. omega. exact tys3.
-  all: try clear rule; simpl; omega || auto.
+  all: try clear rule; simpl; aomega.
   all: try rewrite inst_len_shift; try rewrite same_len. omega.
   - assert (S (S (S (ctx_len Γ0))) = 2+S (ctx_len Γ0)) as same by omega.
     rewrite same. apply c_under_var_shift.
@@ -3268,7 +3459,7 @@ destruct orig. destruct H2; simpl.
   - assert (ctx_insert Γ (TyΠ A B) 0 = CtxU Γ (TyΠ A B)) as same.
     { destruct Γ; simpl; auto. }
     rewrite same. apply wf_inst_extend_n. 
-    inv H3. apply wf_ctx_insert_vtype in H4. all: omega || auto.
+    inv H3. apply wf_ctx_insert_vtype in H4. all: aomega.
 + eapply CL in H0 as tys1; eauto.
   eapply CL in H1 as tys2; eauto.
   eapply CL in H3 as tys3; eauto.
@@ -3287,7 +3478,7 @@ destruct orig. destruct H2; simpl.
     = (c_inst c (inst_insert (inst_shift (inst_shift I 1 0) 1 0) n (Var 1)))).
   { rewrite instU_is_insert, c_inst_no_var_same.
     rewrite c_negshift_shift, c_shift_0. do 2 f_equal.
-    rewrite <-(inst_shift_comm). all: omega || auto.
+    rewrite <-(inst_shift_comm). all: aomega.
     + apply c_shift_makes_no_var.
     + simpl. apply c_under_var_shift.
       rewrite inst_len_insert, inst_len_shift, inst_len_shift, same_len.
@@ -3296,8 +3487,8 @@ destruct orig. destruct H2; simpl.
       all: try omega. rewrite inst_len_shift, inst_len_shift, same_len. omega.
   }
   rewrite H4. eapply rule. omega. exact tys3.
-  all: try clear rule; simpl; omega || auto.
-  all: try rewrite inst_len_shift; try rewrite same_len; omega || auto.
+  all: try clear rule; simpl; aomega.
+  all: try rewrite inst_len_shift; try rewrite same_len; aomega.
   - apply c_under_var_shift. apply has_ctype_is_under_ctx in H3.
     rewrite ctx_len_insert in H3. simpl in H3. auto. all: omega.
   - apply c_under_var_shift. apply has_ctype_is_under_ctx in H3.
@@ -3308,7 +3499,7 @@ destruct orig. destruct H2; simpl.
   - assert (ctx_insert Γ (TyΣ A B) 0 = CtxU Γ (TyΣ A B)) as same.
     { destruct Γ; simpl; auto. }
     rewrite same. apply wf_inst_extend_n. 
-    inv H3. apply wf_ctx_insert_vtype in H4. all: omega || auto.
+    inv H3. apply wf_ctx_insert_vtype in H4. all: aomega.
 + eapply CL in H0 as tys1; eauto.
   eapply CL in H1 as tys2; eauto.
   clear VL CL HL RL VEL CEL HEL WS.
@@ -3343,4 +3534,4 @@ destruct orig; simpl.
   apply WfInstU; auto.
 }
 Qed.
-
+ *)
